@base <https://w3id.org/lbd/c3po/> .
@prefix c3po: <> .
@prefix owl: <http://www.w3.org/2002/07/owl#> .
@prefix rdf: <http://www.w3.org/1999/02/22-rdf-syntax-ns#> .
@prefix xml: <http://www.w3.org/XML/1998/namespace> .
@prefix xsd: <http://www.w3.org/2001/XMLSchema#> .
@prefix rdfs: <http://www.w3.org/2000/01/rdf-schema#> .
@prefix cc: <http://creativecommons.org/ns#> .
@prefix vann: <http://purl.org/vocab/vann/> .
@prefix voaf: <http://purl.org/vocommons/voaf#> .
@prefix foaf: <http://xmlns.com/foaf/0.1/>.
@prefix schema: <http://schema.org/>.
@prefix dct: <http://purl.org/dc/terms/>.
@prefix skos: <http://www.w3.org/2004/02/skos/core#>.
@prefix dul: <http://www.ontologydesignpatterns.org/ont/dul/DUL.owl#>.
@prefix eli: <http://data.europa.eu/eli/ontology#> .
@prefix rdac: <http://www.rdaregistry.info/Elements/c/> .
@prefix quantitykind: <http://qudt.org/vocab/quantitykind/> .
@prefix prov: <http://www.w3.org/ns/prov#>.

c3po:core a owl:Ontology ;
    dct:title "Construction Compliance Checking and Permitting Ontology"@en ;
    dct:description  "An ontology for Construction Compliance Checking and Permitting, based on the statements on building compliance-related document and design codes."@en ;
    skos:note """Main classes and properties in the C3PO ontology are aligned to higher level ontologies, such as DUL."""@en ;
    dct:modified "2023-05-14"^^xsd:date ;
    dct:contributor <edlira> ; 
    dct:contributor <pan> ;
    dct:contributor <http://maxime-lefrancois.info/me#> ; 
    dct:contributor <thomas> ;
	 dct:contributor <etc> ;
    cc:license <https://creativecommons.org/licenses/by/4.0/> ;
    vann:preferredNamespacePrefix "c3po" ;
    vann:preferredNamespaceUri <> .

skos:Concept a owl:Class .
skos:inScheme a owl:ObjectProperty .
skos:ConceptScheme a owl:Class .

#################################################################
#    Document
#################################################################
c3po:Document a owl:Class ;
  rdfs:label "Document"@en ;
  rdfs:comment """A document representing AEC regulations, guidelines, building codes etc."""@en ;
  skos:example """Approved Document A, Eurocode, Finish Regulations..."""@en ;

c3po:DocumentSubdivision a owl:Class
rdfs:subClassOf c3po:Document ;
rdfs:label "Document Subdivision"@en ;
skos:example """Paragraph, section, definition..."""@en

dct:hasPart a owl:ObjectProperty ;
  rdfs:label "has Part"@en ;
  rdfs:comment """A related resource that is included either physically or logically in the described resource."""@en ;
  skos:example """A document has as part of it paragraphs, sections, RASE tags etc. """@en ;
  rdfs:domain c3po:Document ;
  rdfs:range c3po:DocumentSubdivision ;
  owl:inverseOf dct:isPartOf .
  
dct:identifier a owl:ObjectProperty ;
  rdfs:label "Identifier"@en ;
  rdfs:comment """An unambiguous reference to the resource within a given context. """@en ;
  skos:example """To identify the document or a section within the document. Examples include International Standard Book Number (ISBN), Digital Object Identifier (DOI), and Uniform Resource Name (URN). Persistent identifiers should be provided as HTTP URIs. """@en ;
  rdfs:domain [ a owl:Class ; owl:unionOf ( c3po:Document c3po:DocumentSubdivision c3po:Statement ) ] ;
  rdfs:range rdfs:Literal .
  
dct:references a owl:ObjectProperty ;
  rdfs:label "References"@en ;
  rdfs:comment """A related resource that is referenced, cited, or otherwise pointed to by the described resource."""@en ;
  skos:example """Ensure that the measured ceiling height is at least 2.4 meters (7.9 feet) in all habitable rooms. Refer to the Building Code Standards, Section 3.2.1, to verify the requirement for minimum ceiling heights. """@en ;
  rdfs:domain c3po:Document ;
  rdfs:range rdfs:Literal ;
  owl:inverseOf dct:isReferencedBy .

#################################################################
#    Statement
#################################################################
c3po:Statement a owl:Class ;
rdfs:subClassOf c3po:DocumentSubdivision ;
  rdfs:label "Statement"@en ;
  rdfs:comment """Something said in a building compliance-related document"""@en ;
  skos:example """Any  solar protection  solutions  in  the  building  shall  be  taken  into  account  in  the  calculation  of  solar energy gains for the building."""@en ;

dct:source a owl:ObjectProperty ;
  rdfs:label "Source"@en ;
  rdfs:comment """A related resource from which the described statement is derived. """@en ;
  skos:example """Recommended best practice is to identify the related resource by means of a string conforming to a formal identification system."""@en ;
  rdfs:domain c3po:Statement ;
  rdfs:range rdfs:Literal .

c3po:asText a owl:DatatypeProperty ;
  rdfs:label "as text"@en ;
  rdfs:comment """The text as written in a compliance related document or the content of a declarative or procedural check, that verifiers can use."""@en ;
  rdfs:domain [ a owl:Class ; owl:unionOf ( c3po:DeclarativeCheck c3po:ProceduralCheck c3po:Statement) ] .



#################################################################
#    Statement type
#################################################################
c3po:CheckStatement rdf:type owl:Class ;
            rdfs:subClassOf c3po:Statement .

c3po:CategoryCheckStatement rdf:type owl:Class ;
                    rdfs:subClassOf c3po:CheckCheckStatement .


c3po:CertificateCheckStatement rdf:type owl:Class ;
                       rdfs:subClassOf c3po:CheckCheckStatement .


c3po:ChecklistStatement rdf:type owl:Class ;
                         rdfs:subClassOf c3po:Statement .
						 
c3po:DefinitionStatement rdf:type owl:Class ;
    rdfs:subClassOf c3po:Statement .

c3po:HumanEvaluatedStatement rdf:type owl:Class ;
    rdfs:subClassOf c3po:Statement . 
rdfs: comment"""A type of check that is evaluated by a human. Those are primarily for issues of perception, e.g. "is aesthetically appropriate".""" .	
 
c3po:AndCheck a owl:Class ;
    rdfs:label "And Check"@en ;
    rdfs:comment """Check verified if and only if all of its sub-checks are verified."""@en ;
    rdfs:subClassOf c3po:ChecklistStatement ;
    rdfs:subClassOf [ a owl:Restriction ; owl:onProperty c3po:hasSubCheck ; owl:minCardinality 1 ] .
    
c3po:OrCheck a owl:Class ;
    rdfs:label "Or Check"@en ;
    rdfs:comment """Check verified if and only if at least one of its sub-checks is verified."""@en ;
    rdfs:subClassOf c3po:ChecklistStatement ;
    rdfs:subClassOf [ a owl:Restriction ; owl:onProperty c3po:hasSubCheck ; owl:minCardinality 1 ] .

c3po:NumericalCheck rdf:type owl:Class ;
                     rdfs:subClassOf c3po:Check ;
                     rdfs:comment "A check that involves checking one numerical property against another, i.e. x < y or similar." .

#################################################################
#    Features of Interest
#################################################################

c3po:FeatureOfInterest a owl:Class ;
  rdfs:subClassOf dul:Object ;
  rdfs:label "Feature Of Interest"@en ;
  rdfs:comment """The object whose conformance against checks is verified."""@en ;
  skos:example """A building, a building space, a building element, the set of columns in a building, ..."""@en ;
  skos:note """It is expected that classes in other ontologies are used to multi-type instances of FeatureOfInterest.
  For example a feature of interest may also be:
  - a bot:Zone or a bot:Element
  - a ifc:IfcRamp, a ifc:IfcSurfaceFeature"""@en .


#################################################################
#    Properties of features of interest
#################################################################

c3po:Property a owl:Class ;
  rdfs:subClassOf dul:Quality ;
  rdfs:label "Property"@en ;
  rdfs:comment """An aspect of a feature of interest that is intrinsic to and cannot exist without the feature of interest."""@en ;
  skos:example """The height of a building, the area of a space, the U-value of a wall"""@en .

c3po:hasProperty a owl:ObjectProperty ;
  rdfs:label "has Property"@en ;
  rdfs:comment """Links a feature of interest to one of its aspect that is intrinsic to and cannot exist without it."""@en ;
  skos:example """Links a space to the area property of that space, a wall to the U-value property of that wall..."""@en ;
  rdfs:domain c3po:FeatureOfInterest ;
  rdfs:range c3po:Property .


#################################################################
#    Kinds of properties
#################################################################

c3po:PropertyKind a owl:Class ;
  rdfs:subClassOf dul:Region ;
  rdfs:label "Property Kind"@en ;
  rdfs:comment """Any region in a dimensional space, which can be used as a value for a quality of an entity.
  It is expected that the property kinds are organized in a hierarchy of concepts using skos:broader/skos:narrower.
  Property kinds may be taken from the QUDT Quantity Kind vocabulary http://qudt.org/2.1/vocab/quantitykind  """@en ;
  skos:example """Length, Area, U-Value."""@en ;
  skos:note """Both PropertyKind and QuantityValue are aligned to dul:Region. A dimensional space such as "Length" or "Thermal Transmittance" is a maximal Region, and a specific quantity value such as "13 m" or "3.5 W/(m^2.K)" is a minimal Region."""@en .

c3po:hasPropertyKind a owl:ObjectProperty ;
    rdfs:label "has property kind"@en ;
    rdfs:comment """Links a property of a feature of interest to its kind"""@en ;
    skos:example """A space area property to the property kind "area"."""@en ;
    rdfs:domain c3po:Property ;
    rdfs:range c3po:PropertyKind .

c3po:forPropertyKind a owl:ObjectProperty ;
    rdfs:label "for property kind"@en ;
    rdfs:comment """Links any entity (check, verification, procedure execution) to some property kind it is """@en ;
    rdfs:range c3po:PropertyKind .

# some examples

c3po:CompressiveForce a c3po:PropertyKind , skos:Concept ;
  skos:broader quantitykind:Force .
c3po:CrossSection a c3po:PropertyKind, skos:Concept ;
  skos:broader quantitykind:CrossSection .
c3po:GammaM  a c3po:PropertyKind, skos:Concept .
c3po:SystemStrength a c3po:PropertyKind, skos:Concept .
c3po:hasRequiredfc0k a c3po:PropertyKind, skos:Concept .
c3po:kmod a c3po:PropertyKind, skos:Concept .



#################################################################
#   RASE (Requirement, Applicability, Selection, Exclusion)
#################################################################




#################################################################
#    Design
#################################################################

c3po:Design a owl:Class ;
    rdfs:subClassOf dul:Design ;
    rdfs:label "Design"@en ;
    rdfs:comment """A Description of some design of a feature of interest, in terms of structure, geometry, and function. 
    May be linked to a feature of interest to describe the design it has, for example using the ClassificationDesign subclass.
    May be linked to a check, verifier, or check result, to describe the kind of design it is for."""@en ;
    skos:example """Example: 
- the type of use of a building (Residential / Commercial)
- the type of structural material (steel/ RC / timber)
- the designed height of a building (High-rise, Mid-rise, Low-rise)
- the area of space abc in IFC model xyz is 14 m2"""@en .

c3po:hasDesign a owl:ObjectProperty ;
    rdfs:label "has design"@en ;
    rdfs:comment """Links a feature of interest or a property to a description of its design."""@en ;
    rdfs:domain [ a owl:Class ; owl:unionOf ( c3po:FeatureOfInterest c3po:Property ) ] ;
    rdfs:range c3po:Design .

# usure we need this inverse
# c3po:isDesignOf a owl:ObjectProperty ;
#     rdfs:label "is design of"@en ;
#     rdfs:comment """Links a design to the feature of interest or to the property it describes."""@en ;
#     rdfs:domain c3po:Design ;
#     rdfs:range [ a owl:Class ; owl:unionOf ( c3po:FeatureOfInterest c3po:Property ) ] ;
#     owl:inverseOf c3po:hasDesign .

c3po:forDesign a owl:ObjectProperty ;
    rdfs:label "for design"@en ;
    rdfs:comment """Links a check, verifier, or checking act, to the type of design it applies."""@en ;
    rdfs:domain [ a owl:Class ; owl:unionOf ( c3po:Check c3po:Verifier c3po:Checking ) ] ;
    rdfs:range c3po:Design .

# usure we need this inverse
# c3po:isDesignFor a owl:ObjectProperty ;
#     rdfs:label "is design for"@en ;
#     rdfs:comment """Links a design to the check, verifier, or checking act, is applies."""@en ;
#     rdfs:domain c3po:Design ;
#     rdfs:range [ a owl:Class ; owl:unionOf ( c3po:Check c3po:Verifier c3po:Checking ) ] ;
#     owl:inverseOf c3po:forDesign .


#################################################################
#    Classification Design
#################################################################

c3po:ClassificationDesign a owl:Class ;
  rdfs:label "classification design"@en ;
  rdfs:comment "Designs that take values in classification schemes, described using SKOS"@en ;
  skos:note """classification design are expected to be taken in existing concept schemes.
  C3PO defines some concept schemes such as c3po:building_structure
  Existing concept schemes may also be used such as Ifc classes, or bSDD."""@en ;
  owl:equivalentClass [
    owl:intersectionOf (
     skos:Concept
     [  a owl:Restriction ;
        owl:onProperty skos:inScheme ;
        owl:someValuesFrom skos:ConceptScheme .
     ]
   )
  ] .

#################################################################
#    Property Design
#################################################################

c3po:PropertyDesign a owl:Class ;
  rdfs:subClassOf c3po:Design ;
  rdfs:label "property design"@en ;
  rdfs:comment "Designs that assign a value expressed as a literal to some property of a feature of interest."@en ;
  skos:note "The value of the literal may be a XSD literal (boolean, integer, decimal, string), it may also use custom datatypes such as cdt:ucum"@en ;
  rdfs:subClassOf 
    [ a owl:Restriction ;
      owl:onProperty [ owl:inverseOf c3po:hasDesign ] ;
      owl:allValuesFrom c3po:Property ;
    ] ,
    [  a owl:Restriction ;
      owl:onProperty c3po:hasValue ;
      owl:cardinality 1 .
    ] .
    

c3po:hasValue a owl:DatatypeProperty , owl:FunctionalProperty ;
  rdfs:label "has value"@en ;
  rdfs:comment """links a property design to the value of that property, expressed as a literal."""@en ;
  skos:note """The value of the literal may be a XSD literal (boolean, integer, decimal, string), it may also use custom datatypes such as cdt:ucum"""@en ;
  rdfs:domain c3po:PropertyDesign .


#################################################################
#    Property Kind Design
#################################################################

c3po:PropertyKindDesign a owl:Class ;
  rdfs:subClassOf c3po:Design ;
  rdfs:label "property kind design"@en ;
  rdfs:comment "Designs that constrain the value for some property kind."@en ;
  skos:note """The comparisonOperator must be taken from the c3po:ComparisonOperatorTable concept scheme defined in module c3po:comparisonOperators"""@en ;
  rdfs:subClassOf 
    [  a owl:Restriction ;
      owl:onProperty [ owl:inverseOf c3po:hasDesign ] ;
      owl:allValuesFrom c3po:PropertyKind 
    ] ,
    [  a owl:Restriction ;
      owl:onProperty c3po:hasValue ;
      owl:cardinality 1 
    ] ,
    [  a owl:Restriction ;
      owl:onProperty c3po:hasComparisonOperator ;
      owl:cardinality 1 
    ] ;
  rdfs:seeAlso c3po:comparisonOperators .

c3po:hasComparisonOperator a owl:ObjectProperty, owl:FunctionalProperty ;
  rdfs:subPropertyOf c3po:hasDesign ;
  rdfs:range c3po:ComparisonOperator ;
  rdfs:label "has comparisonOperator"@en ;
  rdfs:comment """The comparisonOperator of a property kind design;
  A set of values is defined by C3PO in the corresponding concept scheme."""@en .



c3po:ComparisonOperator a owl:Class ;
  rdfs:subClassOf skos:Concept ;
  rdfs:label "comparisonComparisonOperator"@en ;
  rdfs:comment "Formally defined as the set of skos:Concept in concept scheme c3po:ComparisonOperatorTable"@en ;
  owl:equivalentClass [
    owl:intersectionOf (
     skos:Concept
     [  a owl:Restriction ;
        owl:onProperty skos:inScheme ;
        owl:hasValue eli:ComparisonOperatorTable .
     ]
   )
  ] .

c3po:ComparisonOperatorTable a skos:ConceptScheme ;
  skos:hasTopConcept c3po:ComparisonOperator-lt, c3po:ComparisonOperator-le, c3po:ComparisonOperator-eq, c3po:ComparisonOperator-ge, c3po:ComparisonOperator-gt ;
  rdfs:label "Opeator table"@en ;
  skos:definition """A set of values for the comparisonComparisonOperator.
  C3PO includes a set of values for this table.
  These values are :
  - lt : lower than;
  - le : lower or equal;
  - eq : equals;
  - ge : greater or equal;
  - gt : greater than."""@en .

c3po:ComparisonOperator-lt a c3po:ComparisonOperator, skos:Concept ;
  skos:inScheme c3po:ComparisonOperatorTable ;
  skos:topConceptOf c3po:ComparisonOperatorTable ;
  skos:definition "Less than comparisonComparisonOperator."@en ;
  skos:prefLabel "less than"@en .

c3po:ComparisonOperator-le a c3po:ComparisonOperator, skos:Concept ;
  skos:inScheme c3po:ComparisonOperatorTable ;
  skos:topConceptOf c3po:ComparisonOperatorTable ;
  skos:definition "Less or equal comparisonComparisonOperator."@en ;
  skos:prefLabel "less or equal"@en .

c3po:ComparisonOperator-eq a c3po:ComparisonOperator, skos:Concept ;
  skos:inScheme c3po:ComparisonOperatorTable ;
  skos:topConceptOf c3po:ComparisonOperatorTable ;
  skos:definition "Equals comparisonComparisonOperator."@en ;
  skos:prefLabel "equals"@en .

c3po:ComparisonOperator-ge a c3po:ComparisonOperator, skos:Concept ;
  skos:inScheme c3po:ComparisonOperatorTable ;
  skos:topConceptOf c3po:ComparisonOperatorTable ;
  skos:definition "Greater or equal comparisonComparisonOperator."@en ;
  skos:prefLabel "greater or equal"@en .
  
c3po:ComparisonOperator-gt a c3po:ComparisonOperator, skos:Concept ;
  skos:inScheme c3po:ComparisonOperatorTable ;
  skos:topConceptOf c3po:ComparisonOperatorTable ;
  skos:definition "Greater than comparisonComparisonOperator."@en ;
  skos:prefLabel "greater than"@en .



#################################################################
#     Checks as operationalization of document subdivisions 
#################################################################


c3po:Check a owl:Class ;
    rdfs:subClassOf dul:Method ;
    rdfs:label "Check"@en ;
    rdfs:comment """A piece of information that operationalizes a clause, usually executed in order to control the conformance of some entity against a design. A Check is re-usable, and may be executed several times."""@en ;
    skos:note """A Check may be linked to some Design through the `forDesign` property.
    A Check may be linked to some Property Kind through the `forPropertyKind` property."""@en .

c3po:isOperationalizedBy a owl:ObjectProperty ;
  rdfs:domain eli:DocumentSubdivision ; # encompasses c3po:Statement
  rdfs:range c3po:Check ;
  owl:inverseOf c3po:operationalizes .

c3po:operationalizes a owl:ObjectProperty ;
  rdfs:domain c3po:Check ;
  rdfs:range eli:DocumentSubdivision ;
  owl:inverseOf c3po:isOperationalizedBy .

c3po:hasSubCheck a owl:ObjectProperty ;
  rdfs:label "has sub check"@en ;
  rdfs:comment """Links a AndCheck to the set of checks that all need to be verified.
Links a OrCheck to the set of checks that at least one must verify."""@en ;
  rdfs:domain c3po:Check ;
  rdfs:range c3po:Check .
 


c3po:ComponentCheck  a owl:Class ;
  rdfs:subClassOf c3po:Check ;
  rdfs:label "Component Check"@en ;
  rdfs:comment """Formally defined as checks for some feature of interest"""@en ;
  owl:equivalentClass [
    a owl:Class ;
    owl:intersectionOf (
      c3po:Check 
      [
        a owl:Restriction ; 
        owl:onProperty c3po:forDesign ;
        owl:allValuesFrom [
            a owl:Restriction ;
            owl:onProperty [ owl:inverseOf c3po:forDesign ] ;
            owl:allValuesFrom c3po:FeatureOfInterest
        ]
      ]
    )
  ] .

c3po:DeclarativeCheck a owl:Class ;
    rdfs:subClassOf c3po:Check ;
    rdfs:label "Declarative Check"@en ;
    rdfs:comment """Declarative check, expressed in IDS, SPARQL, BimSPARQL (SPARQL with eg HDF5 for geometry access, with extra SPARQL functions), or any other declarative language. 

The identifier of a Declarative Check is expected to be dereferenceable, potentially with mediatype-based content negotiation. The content type of the retrieved representation indicates which type of declaration language it uses. Alternatively, the check expression may be given using a property such as c3po:asText."""@en .

c3po:IDSCheck a owl:Class ;
    rdfs:subClassOf c3po:DeclarativeCheck ;
    skos:note "must be refined" .

c3po:ProceduralCheck a owl:Class ;
    rdfs:subClassOf c3po:Check ;
    rdfs:label "Procedural Check"@en ;
    rdfs:comment """Procedural checks are semantically described but opaque modules, implemented in any language or as REST API, invoked by micro-services.
Alternatively, the check procedure may be given using a property such as c3po:asText."""@en .


#################################################################
#     Execution of checks
#################################################################

c3po:Checking a owl:Class ;
    rdfs:subClassOf dul:Event ;
    rdfs:label "Checking"@en ;
    rdfs:comment """Act of verifying a check to determine the conformance of some design. 
    Links to Verifier that made the checking act ;
    Links to the checks that were verified, either satified, or unsatisfied;
    Links to the designs that were satisfied, or unsatisfied."""@en ;
    rdfs:subClassOf [ 
      a owl:Restriction ;
      owl:onProperty c3po:madeBy ;
      owl:someValuesFrom c3po:Verifier
    ] , [ 
      a owl:Restriction ;
      owl:onProperty c3po:checked ;
      owl:minCardinality 1
    ] .

c3po:madeBy a owl:ObjectProperty ;
  rdfs:label "made by"@en ;
  rdfs:comment """Links a checking act to the verifier that made it."""@en ;
  rdfs:domain c3po:Checking ;
  rdfs:range c3po:Verifier .

c3po:checked a owl:ObjectProperty ;
  rdfs:label "checked"@en ;
  rdfs:comment """Links a checking act to the feature of interest, property, design, check, or legal resource, it verified."""@en ;
  rdfs:domain c3po:Checking ;
  rdfs:range c3po:Check .

c3po:satisfied a owl:ObjectProperty ;
  rdfs:subPropertyOf c3po:checked ;
  rdfs:label "satisfied"@en ;
  rdfs:comment """Links a checking act to a satisfied feature of interest, property, design, check, or legal resource."""@en ;
  rdfs:domain c3po:Checking ;
  rdfs:range [ 
    a owl:Class ; 
    owl:unionOf ( 
      c3po:FeatureOfInterest 
      c3po:Property 
      c3po:Design 
      c3po:Check
      eli:LegalResource 
      )
    ] .

c3po:unsatisfied a owl:ObjectProperty ;
  rdfs:subPropertyOf c3po:checked ;
  rdfs:label "unsatisfied check"@en ;
  rdfs:comment """Links a checking act to an unsatisfied  feature of interest, property, design, check, or legal resource."""@en .

c3po:hasEvidence a owl:ObjectProperty ;
    rdfs:domain c3po:Checking ;
    rdfs:label "has evidence"@en ;
    rdfs:comment """Links a checking act to some evidence that demonstrates that this checking act is satisfied or unsatisfied."""@en .

#################################################################
#     Verifier 
#################################################################

c3po:LegalVerifier a owl:Class ;
 rdfs:label "Legal Verifier"@en ;
  rdfs:comment """ """@en .

c3po:StateVerifier a owl:Clas ;
	rdfs:subClassOf c3po:LegalVerifier.
 	rdfs:label "State Verifier"@en ;
	rdfs:comment """ """@en .

c3po:PrivateVerifier a owl:Clas ;
	rdfs:subClassOf c3po:LegalVerifier.
 	rdfs:label "Provate Verifier"@en ;
	rdfs:comment """ """@en .


#################################################################
#     General axioms
#################################################################


[ a owl:AllDisjointClasses ;
  owl:members ( c3po:FeatureOfInterest
    c3po:Property
    c3po:PropertyKind
    c3po:Design
    eli:LegalResource
    c3po:Check
    c3po:Verifier
    c3po:Checking
    )
] .

