@base <https://w3id.org/lbd/aec3po/> .
@prefix aec3po: <https://w3id.org/lbd/aec3po/> .
@prefix cc: <http://creativecommons.org/ns#> .
@prefix dct: <http://purl.org/dc/terms/> .
@prefix dul: <http://www.ontologydesignpatterns.org/ont/dul/DUL.owl#> .
@prefix ns1: <https://w3id.org/profile/ontdoc/> .
@prefix owl: <http://www.w3.org/2002/07/owl#> .
@prefix prov: <http://www.w3.org/ns/prov#> .
@prefix rdfs: <http://www.w3.org/2000/01/rdf-schema#> .
@prefix vann: <http://purl.org/vocab/vann/> .
@prefix xsd: <http://www.w3.org/2001/XMLSchema#> .

<CheckingAct> a rdfs:Class,
        owl:Class ;
    rdfs:label "Checking Act"@en ;
    dct:description """Act of checking some entities for something and generating a compliance verification report. 
    
- Links to the check method that was used, which operationalizes a statement in a document;
- Links to the process verifier that made the checking act;
- Links to the entities that are checked;
- Links to compliance verification report that resulted.

"""@en ;
    dct:title "Checking Act"@en ;
    rdfs:comment """Act of checking some entities for something and generating a compliance verification report. 
    
- Links to the check method that was used, which operationalizes a statement in a document;
- Links to the process verifier that made the checking act;
- Links to the entities that are checked;
- Links to compliance verification report that resulted.

"""@en ;
    rdfs:isDefinedBy <checking_act> ;
    rdfs:subClassOf _:n91d995ee228547bba028da91f80be7dab1,
        _:n91d995ee228547bba028da91f80be7dab2,
        _:n91d995ee228547bba028da91f80be7dab3,
        _:n91d995ee228547bba028da91f80be7dab4,
        dul:Event ;
    ns1:inDomainOf <checked>,
        <endTime>,
        <hasReport>,
        <madeBy>,
        <startTime>,
        <usedMethod> .

<http://maxime-lefrancois.info/me#> a prov:Agent .

dul:Event ns1:superClassOf <CheckingAct> .

rdfs:Class ns1:hasMember <CheckingAct> .

owl:Class ns1:hasMember <CheckingAct> .

owl:Ontology ns1:hasMember <checking_act> .

xsd:dateTime ns1:inRangeOf <endTime>,
        <startTime> .

owl:DatatypeProperty ns1:hasMember <endTime>,
        <startTime> .

<CheckMethod> ns1:inRangeOf <usedMethod> .

<ComplianceVerificationReport> ns1:inRangeOf <hasReport> .

<ProcessVerifier> ns1:inRangeOf <madeBy> .

<checked> a owl:ObjectProperty ;
    rdfs:label "checked"@en ;
    dct:description "Links a checking act to some entity (ex. statement, feature of interest, property) it checked."@en ;
    dct:title "checked"@en ;
    rdfs:comment "Links a checking act to some entity (ex. statement, feature of interest, property) it checked."@en ;
    rdfs:domain <CheckingAct> ;
    rdfs:isDefinedBy <checking_act> .

<endTime> a owl:DatatypeProperty ;
    rdfs:label "end time"@en ;
    dct:description "the end time of the checking act"@en ;
    dct:title "end time"@en ;
    rdfs:comment "the end time of the checking act"@en ;
    rdfs:domain <CheckingAct> ;
    rdfs:isDefinedBy <checking_act> ;
    rdfs:range xsd:dateTime .

<startTime> a owl:DatatypeProperty ;
    rdfs:label "start time"@en ;
    dct:description "the start time of the checking act"@en ;
    dct:title "start time"@en ;
    rdfs:comment "the start time of the checking act"@en ;
    rdfs:domain <CheckingAct> ;
    rdfs:isDefinedBy <checking_act> ;
    rdfs:range xsd:dateTime .

owl:ObjectProperty ns1:hasMember <checked>,
        <hasReport>,
        <madeBy>,
        <usedMethod> .

owl:Restriction ns1:hasMember _:n91d995ee228547bba028da91f80be7dab1,
        _:n91d995ee228547bba028da91f80be7dab2,
        _:n91d995ee228547bba028da91f80be7dab3,
        _:n91d995ee228547bba028da91f80be7dab4 .

<hasReport> a owl:ObjectProperty ;
    rdfs:label "has report"@en ;
    dct:description "Links a checking act to the resulting compliance verification report."@en ;
    dct:title "has report"@en ;
    rdfs:comment "Links a checking act to the resulting compliance verification report."@en ;
    rdfs:domain <CheckingAct> ;
    rdfs:isDefinedBy <checking_act> ;
    rdfs:range <ComplianceVerificationReport> .

<madeBy> a owl:ObjectProperty ;
    rdfs:label "made by"@en ;
    dct:description "Links a checking act to the process verifier that made it (a aec3po:ProcessVerifier)."@en ;
    dct:title "made by"@en ;
    rdfs:comment "Links a checking act to the process verifier that made it (a aec3po:ProcessVerifier)."@en ;
    rdfs:domain <CheckingAct> ;
    rdfs:isDefinedBy <checking_act> ;
    rdfs:range <ProcessVerifier> .

<usedMethod> a owl:ObjectProperty ;
    rdfs:label "used method"@en ;
    dct:description "Links a checking act to the method it used (a aec3po:CheckMethod)."@en ;
    dct:title "used method"@en ;
    rdfs:comment "Links a checking act to the method it used (a aec3po:CheckMethod)."@en ;
    rdfs:domain <CheckingAct> ;
    rdfs:isDefinedBy <checking_act> ;
    rdfs:range <CheckMethod> .

<checking_act> a owl:Ontology ;
    cc:license <https://creativecommons.org/licenses/by/4.0/> ;
    dct:contributor <http://maxime-lefrancois.info/me#> ;
    dct:created "2023-05-26"^^xsd:date ;
    dct:description "The AEC3PO Checking Act module describes the act of checking some entities for something and generating a compliance verification report."@en ;
    dct:modified "2023-05-26"^^xsd:date,
        "2024-02-28"^^xsd:date ;
    dct:title "AEC3PO: Checking Act"@en ;
    vann:preferredNamespacePrefix "aec3po" ;
    vann:preferredNamespaceUri "https://w3id.org/lbd/aec3po/" ;
    owl:imports <check_method>,
        <compliance_verification_report> .

_:n91d995ee228547bba028da91f80be7dab1 a owl:Restriction ;
    owl:onProperty <usedMethod> ;
    owl:someValuesFrom <CheckMethod> ;
    ns1:superClassOf <CheckingAct> .

_:n91d995ee228547bba028da91f80be7dab2 a owl:Restriction ;
    owl:onProperty <madeBy> ;
    owl:someValuesFrom <ProcessVerifier> ;
    ns1:superClassOf <CheckingAct> .

_:n91d995ee228547bba028da91f80be7dab3 a owl:Restriction ;
    owl:onProperty <checked> ;
    owl:someValuesFrom owl:Thing ;
    ns1:superClassOf <CheckingAct> .

_:n91d995ee228547bba028da91f80be7dab4 a owl:Restriction ;
    owl:onProperty <hasReport> ;
    owl:someValuesFrom <ComplianceVerificationReport> ;
    ns1:superClassOf <CheckingAct> .

