<?xml version="1.0" encoding="utf-8"?>
<rdf:RDF xml:base="https://w3id.org/lbd/aec3po/"
  xmlns:owl="http://www.w3.org/2002/07/owl#"
  xmlns:vann="http://purl.org/vocab/vann/"
  xmlns:rdfs="http://www.w3.org/2000/01/rdf-schema#"
  xmlns:dct="http://purl.org/dc/terms/"
  xmlns:aec3po="https://w3id.org/lbd/aec3po/"
  xmlns:rdf="http://www.w3.org/1999/02/22-rdf-syntax-ns#"
  xmlns:cc="http://creativecommons.org/ns#"
>
  <owl:DatatypeProperty rdf:about="resultMessage">
    <rdfs:label xml:lang="en">result message</rdfs:label>
    <rdfs:comment>Verification results may have values for the property aec3po:resultMessage, for example to communicate additional textual details to humans. While aec3po:resultMessage may have multiple values, there should not be two values with the same language tag. These values may be produced based on the statements in the AEC3PO graph.</rdfs:comment>
    <rdfs:domain rdf:resource="VerificationResult"/>
    <rdfs:isDefinedBy>
      <owl:Ontology rdf:about="compliance_verification_report">
        <cc:license rdf:resource="https://creativecommons.org/licenses/by/4.0/"/>
        <dct:contributor rdf:resource="http://maxime-lefrancois.info/me#"/>
        <dct:description xml:lang="en">The AEC3PO Compliance Verification Report module describes results of some `aec3po:ProcessVerifier` checking some entity via a `aec3po:CheckingAct`. Entities may be validated or repudiated.</dct:description>
        <dct:title xml:lang="en">AEC3PO: Compliance Verification Report</dct:title>
        <owl:imports rdf:resource="check_method"/>
        <owl:imports rdf:resource="compliance_verification_report"/>
        <vann:preferredNamespacePrefix>aec3po</vann:preferredNamespacePrefix>
        <vann:preferredNamespaceUri>https://w3id.org/lbd/aec3po/</vann:preferredNamespaceUri>
        <dct:created rdf:datatype="http://www.w3.org/2001/XMLSchema#date">2023-10-30</dct:created>
        <dct:modified rdf:datatype="http://www.w3.org/2001/XMLSchema#date">2025-04-22</dct:modified>
      </owl:Ontology>
    </rdfs:isDefinedBy>
  </owl:DatatypeProperty>
  <owl:NamedIndividual rdf:about="Info">
    <rdf:type rdf:resource="Severity"/>
    <rdfs:label xml:lang="en">Info</rdfs:label>
    <rdfs:comment xml:lang="en">The severity for an informational validation result.</rdfs:comment>
    <rdfs:isDefinedBy rdf:resource="compliance_verification_report"/>
  </owl:NamedIndividual>
  <owl:ObjectProperty rdf:about="hasResult">
    <rdfs:label xml:lang="en">has result</rdfs:label>
    <rdfs:comment xml:lang="en">Links a compliance verification report to some verification result.</rdfs:comment>
    <rdfs:isDefinedBy rdf:resource="compliance_verification_report"/>
    <rdfs:domain rdf:resource="ComplianceVerificationReport"/>
    <rdfs:range rdf:resource="VerificationResult"/>
  </owl:ObjectProperty>
  <owl:NamedIndividual rdf:about="Violation">
    <rdf:type rdf:resource="Severity"/>
    <rdfs:label xml:lang="en">Violation</rdfs:label>
    <rdfs:comment xml:lang="en">The severity for a violation validation result.</rdfs:comment>
    <rdfs:isDefinedBy rdf:resource="compliance_verification_report"/>
  </owl:NamedIndividual>
  <owl:ObjectProperty rdf:about="verificationStatement">
    <rdfs:label xml:lang="en">verification statement</rdfs:label>
    <rdfs:comment>Statement that was validated when the verification result was produced.</rdfs:comment>
    <rdfs:domain rdf:resource="VerificationResult"/>
    <rdfs:range rdf:resource="CheckStatement"/>
    <rdfs:isDefinedBy rdf:resource="compliance_verification_report"/>
  </owl:ObjectProperty>
  <owl:ObjectProperty rdf:about="verificationPlanZone">
    <rdfs:label xml:lang="en">verification plan zone</rdfs:label>
    <rdfs:comment>Planning (urban regulation) zone where the verificationFocus entity (building or building component) is located, and that defines the regulation (verificationStatement) that was validated when the verification result was produced.</rdfs:comment>
    <rdfs:domain rdf:resource="VerificationResult"/>
    <rdfs:isDefinedBy rdf:resource="compliance_verification_report"/>
  </owl:ObjectProperty>
  <owl:NamedIndividual rdf:about="Warning">
    <rdf:type rdf:resource="Severity"/>
    <rdfs:label xml:lang="en">Warning</rdfs:label>
    <rdfs:comment xml:lang="en">The severity for a warning validation result.</rdfs:comment>
    <rdfs:isDefinedBy rdf:resource="compliance_verification_report"/>
  </owl:NamedIndividual>
  <owl:DatatypeProperty rdf:about="conforms">
    <rdfs:label xml:lang="en">conforms</rdfs:label>
    <rdfs:comment xml:lang="en">True if the Checking act confirms the check was validated, and false otherwise.</rdfs:comment>
    <rdfs:domain rdf:resource="ComplianceVerificationReport"/>
    <rdfs:isDefinedBy rdf:resource="compliance_verification_report"/>
    <rdfs:range rdf:resource="http://www.w3.org/2001/XMLSchema#boolean"/>
  </owl:DatatypeProperty>
  <owl:Class rdf:about="VerificationResult">
    <rdfs:label xml:lang="en">Verification Result</rdfs:label>
    <rdfs:comment xml:lang="en">Individual verification result of a Compliance Verification Report.</rdfs:comment>
    <rdfs:isDefinedBy rdf:resource="compliance_verification_report"/>
    <rdfs:subClassOf>
      <owl:Restriction rdf:nodeID="nd7cc22cd62e14854b47c852263b35d28b2">
        <owl:onProperty rdf:resource="verificationFocus"/>
        <owl:cardinality rdf:datatype="http://www.w3.org/2001/XMLSchema#integer">1</owl:cardinality>
      </owl:Restriction>
    </rdfs:subClassOf>
    <rdfs:subClassOf>
      <owl:Restriction rdf:nodeID="nd7cc22cd62e14854b47c852263b35d28b3">
        <owl:onProperty rdf:resource="hasSeverity"/>
        <owl:cardinality rdf:datatype="http://www.w3.org/2001/XMLSchema#integer">1</owl:cardinality>
      </owl:Restriction>
    </rdfs:subClassOf>
  </owl:Class>
  <owl:Class rdf:about="Severity">
    <rdfs:label xml:lang="en">Severity</rdfs:label>
    <rdfs:comment xml:lang="en">The class of validation result severity levels, including violation and warning levels.</rdfs:comment>
    <rdfs:isDefinedBy rdf:resource="compliance_verification_report"/>
  </owl:Class>
  <owl:ObjectProperty rdf:about="verificationFocus">
    <rdfs:label xml:lang="en">verification focus</rdfs:label>
    <rdfs:comment>Each verification result has exactly one value for the property aec3po:verificationFocus that is equal to the focus entity that has caused the result. This is the focus entity that was validated when the verification result was produced.</rdfs:comment>
    <rdfs:domain rdf:resource="VerificationResult"/>
    <rdfs:isDefinedBy rdf:resource="compliance_verification_report"/>
  </owl:ObjectProperty>
  <owl:ObjectProperty rdf:about="hasSeverity">
    <rdfs:label xml:lang="en">has severity</rdfs:label>
    <rdfs:comment>Each verification result has exactly one value for the property aec3po:resultSeverity, and this value is an IRI. The value is equal to the value of aec3po:hasSeverity of the statement in the AEC3PO graph that caused the result, defaulting to aec3po:Violation if no aec3po:hasSeverity has been specified for the statement.</rdfs:comment>
    <rdfs:domain rdf:resource="VerificationResult"/>
    <rdfs:range rdf:resource="Severity"/>
    <rdfs:isDefinedBy rdf:resource="compliance_verification_report"/>
  </owl:ObjectProperty>
  <owl:Class rdf:about="ComplianceVerificationReport">
    <rdfs:label xml:lang="en">Compliance Verification Report</rdfs:label>
    <rdfs:comment xml:lang="en">Result of a checking act. May be compliant or not.</rdfs:comment>
    <rdfs:isDefinedBy rdf:resource="compliance_verification_report"/>
    <rdfs:subClassOf>
      <owl:Restriction rdf:nodeID="nd7cc22cd62e14854b47c852263b35d28b1">
        <owl:onProperty rdf:resource="conforms"/>
        <owl:cardinality rdf:datatype="http://www.w3.org/2001/XMLSchema#integer">1</owl:cardinality>
      </owl:Restriction>
    </rdfs:subClassOf>
  </owl:Class>
</rdf:RDF>
