<?xml version="1.0" encoding="utf-8"?>
<rdf:RDF xml:base="https://w3id.org/lbd/aec3po/"
  xmlns:rdfs="http://www.w3.org/2000/01/rdf-schema#"
  xmlns:dct="http://purl.org/dc/terms/"
  xmlns:prov="http://www.w3.org/ns/prov#"
  xmlns:ns1="https://w3id.org/profile/ontdoc/"
  xmlns:skos="http://www.w3.org/2004/02/skos/core#"
  xmlns:owl="http://www.w3.org/2002/07/owl#"
  xmlns:vann="http://purl.org/vocab/vann/"
  xmlns:rdf="http://www.w3.org/1999/02/22-rdf-syntax-ns#"
  xmlns:cc="http://creativecommons.org/ns#"
>
  <owl:Class rdf:about="DataRequirement">
    <rdf:type>
      <rdf:Description rdf:about="http://www.w3.org/2000/01/rdf-schema#Class">
        <ns1:hasMember rdf:resource="hasRequiredData"/>
        <ns1:hasMember rdf:resource="DataRequirement"/>
        <ns1:hasMember rdf:resource="IDS"/>
      </rdf:Description>
    </rdf:type>
    <rdfs:label xml:lang="en">Data Requirement</rdfs:label>
    <rdfs:comment xml:lang="en">Data-informed by a Statement which is required in order to perform a check to demonstrate compliance checking.</rdfs:comment>
    <skos:example xml:lang="en">The minimum width of a door can be a data requirement.</skos:example>
    <rdfs:isDefinedBy>
      <owl:Ontology rdf:about="data_requirement">
        <cc:license rdf:resource="https://creativecommons.org/licenses/by/4.0/"/>
        <dct:contributor rdf:resource="http://maxime-lefrancois.info/me#"/>
        <dct:description xml:lang="en">The AEC3PO DataRequirement module describes the data requirements that derive from a statement. These can describe any aspect of the building model or any type of property, physical or conceptual, associated with it.</dct:description>
        <dct:description rdf:resource="file:///home/runner/work/aec3po/aec3po/src/diagrams/data_requirement.png"/>
        <dct:title xml:lang="en">AEC3PO: Data Requirement</dct:title>
        <vann:preferredNamespacePrefix>aec3po</vann:preferredNamespacePrefix>
        <vann:preferredNamespaceUri>https://w3id.org/lbd/aec3po/</vann:preferredNamespaceUri>
        <owl:imports rdf:resource="statement"/>
        <dct:created rdf:datatype="http://www.w3.org/2001/XMLSchema#date">2023-10-01</dct:created>
        <dct:modified rdf:datatype="http://www.w3.org/2001/XMLSchema#date">2025-04-22</dct:modified>
      </owl:Ontology>
    </rdfs:isDefinedBy>
    <dct:title xml:lang="en">Data Requirement</dct:title>
    <dct:description xml:lang="en">Data-informed by a Statement which is required in order to perform a check to demonstrate compliance checking.</dct:description>
    <ns1:superClassOf rdf:resource="IDS"/>
    <ns1:inRangeOf rdf:resource="hasRequiredData"/>
  </owl:Class>
  <rdf:Description rdf:about="http://www.w3.org/2002/07/owl#Class">
    <ns1:hasMember rdf:resource="hasRequiredData"/>
    <ns1:hasMember rdf:resource="DataRequirement"/>
    <ns1:hasMember rdf:resource="IDS"/>
  </rdf:Description>
  <owl:Class rdf:about="hasRequiredData">
    <rdf:type rdf:resource="http://www.w3.org/2000/01/rdf-schema#Class"/>
    <rdfs:label xml:lang="en">has required data</rdfs:label>
    <rdfs:comment xml:lang="en">Links a statement to some data that is required in order to perform a check to demonstrate compliance checking.</rdfs:comment>
    <rdfs:domain>
      <rdf:Description rdf:about="Statement">
        <ns1:inDomainOf rdf:resource="hasRequiredData"/>
      </rdf:Description>
    </rdfs:domain>
    <rdfs:range rdf:resource="DataRequirement"/>
    <rdfs:isDefinedBy rdf:resource="data_requirement"/>
    <dct:title xml:lang="en">has required data</dct:title>
    <dct:description xml:lang="en">Links a statement to some data that is required in order to perform a check to demonstrate compliance checking.</dct:description>
  </owl:Class>
  <prov:Agent rdf:about="http://maxime-lefrancois.info/me#"/>
  <owl:Class rdf:about="IDS">
    <rdf:type rdf:resource="http://www.w3.org/2000/01/rdf-schema#Class"/>
    <rdfs:label xml:lang="en">IDS</rdfs:label>
    <rdfs:comment xml:lang="en">Required data defined in an Information Delivery Format (IDS).</rdfs:comment>
    <rdfs:subClassOf rdf:resource="DataRequirement"/>
    <rdfs:isDefinedBy rdf:resource="data_requirement"/>
    <dct:title xml:lang="en">IDS</dct:title>
    <dct:description xml:lang="en">Required data defined in an Information Delivery Format (IDS).</dct:description>
  </owl:Class>
  <rdf:Description rdf:about="http://www.w3.org/2002/07/owl#Ontology">
    <ns1:hasMember rdf:resource="data_requirement"/>
  </rdf:Description>
</rdf:RDF>
