@base <https://w3id.org/lbd/aec3po/> .
@prefix aec3po: <https://w3id.org/lbd/aec3po/> .
@prefix cc: <http://creativecommons.org/ns#> .
@prefix dct: <http://purl.org/dc/terms/> .
@prefix owl: <http://www.w3.org/2002/07/owl#> .
@prefix rdfs: <http://www.w3.org/2000/01/rdf-schema#> .
@prefix skos: <http://www.w3.org/2004/02/skos/core#> .
@prefix vann: <http://purl.org/vocab/vann/> .
@prefix xsd: <http://www.w3.org/2001/XMLSchema#> .

<IDS> a owl:Class ;
    rdfs:label "IDS"@en ;
    rdfs:comment "Required data defined in an Information Delivery Format (IDS)."@en ;
    rdfs:isDefinedBy <data_requirement> ;
    rdfs:subClassOf <DataRequirement> .

<hasRequiredData> a owl:Class ;
    rdfs:label "has required data"@en ;
    rdfs:comment "Links a statement to some data that is required in order to perform a check to demonstrate compliance checking."@en ;
    rdfs:domain <Statement> ;
    rdfs:isDefinedBy <data_requirement> ;
    rdfs:range <DataRequirement> .

<DataRequirement> a owl:Class ;
    rdfs:label "Data Requirement"@en ;
    rdfs:comment "Data-informed by a Statement which is required in order to perform a check to demonstrate compliance checking."@en ;
    rdfs:isDefinedBy <data_requirement> ;
    skos:example "The minimum width of a door can be a data requirement."@en .

<data_requirement> a owl:Ontology ;
    cc:license <https://creativecommons.org/licenses/by/4.0/> ;
    dct:contributor <http://maxime-lefrancois.info/me#> ;
    dct:created "2023-10-01"^^xsd:date ;
    dct:description <file:///home/runner/work/aec3po/aec3po/src/DataRequirement.png>,
        "The AEC3PO DataRequirement module describes the data requirements that derive from a statement. These can describe any aspect of the building model or any type of property, physical or conceptual, associated with it."@en ;
    dct:modified "2024-02-28"^^xsd:date ;
    dct:title "AEC3PO: Data Requirement"@en ;
    vann:preferredNamespacePrefix "aec3po" ;
    vann:preferredNamespaceUri "https://w3id.org/lbd/aec3po/" ;
    owl:imports <statement> .

