<?xml version="1.0" encoding="utf-8"?>
<rdf:RDF xml:base="https://w3id.org/lbd/aec3po/"
  xmlns:owl="http://www.w3.org/2002/07/owl#"
  xmlns:skos="http://www.w3.org/2004/02/skos/core#"
  xmlns:rdfs="http://www.w3.org/2000/01/rdf-schema#"
  xmlns:dct="http://purl.org/dc/terms/"
  xmlns:rdf="http://www.w3.org/1999/02/22-rdf-syntax-ns#"
  xmlns:prov="http://www.w3.org/ns/prov#"
  xmlns:ns1="https://w3id.org/profile/ontdoc/"
  xmlns:vann="http://purl.org/vocab/vann/"
  xmlns:cc="http://creativecommons.org/ns#"
>
  <owl:Class rdf:about="Document">
    <rdf:type>
      <rdf:Description rdf:about="http://www.w3.org/2000/01/rdf-schema#Class">
        <ns1:hasMember rdf:resource="Document"/>
        <ns1:hasMember rdf:resource="DocumentSubdivision"/>
        <ns1:hasMember rdf:resource="Drawing"/>
        <ns1:hasMember rdf:resource="Image"/>
      </rdf:Description>
    </rdf:type>
    <rdfs:label xml:lang="en">Document</rdfs:label>
    <rdfs:comment xml:lang="en">A document representing AEC regulations, guidelines, building codes etc.</rdfs:comment>
    <skos:note xml:lang="en">a Document is expected to be annotated using properties from the Dublin Core Terms vocabulary.</skos:note>
    <skos:example xml:lang="en">Approved Document A, Eurocode, Finish Regulations, etc.</skos:example>
    <rdfs:isDefinedBy>
      <owl:Ontology rdf:about="document">
        <cc:license rdf:resource="https://creativecommons.org/licenses/by/4.0/"/>
        <dct:contributor rdf:resource="http://maxime-lefrancois.info/me#"/>
        <dct:description xml:lang="en">The AEC3PO Document module describes a document, of any kind, typically related to compliance and permitting. Documents are split into division and subdivisions, down to individual statements.

Document subdivisions can be described as literals, link to their first part, and to their immediate following subdivision. This enables roundtripping from a document to its AEC3PO description, and back.</dct:description>
        <dct:description rdf:resource="file:///home/runner/work/aec3po/aec3po/src/diagrams/document.png"/>
        <dct:modified rdf:datatype="http://www.w3.org/2001/XMLSchema#date">2023-05-25</dct:modified>
        <dct:modified rdf:datatype="http://www.w3.org/2001/XMLSchema#date">2025-04-22</dct:modified>
        <dct:title xml:lang="en">AEC3PO: document</dct:title>
        <vann:preferredNamespacePrefix>aec3po</vann:preferredNamespacePrefix>
        <vann:preferredNamespaceUri>https://w3id.org/lbd/aec3po/</vann:preferredNamespaceUri>
        <dct:created rdf:datatype="http://www.w3.org/2001/XMLSchema#date">2023-05-25</dct:created>
      </owl:Ontology>
    </rdfs:isDefinedBy>
    <dct:title xml:lang="en">Document</dct:title>
    <dct:description xml:lang="en">A document representing AEC regulations, guidelines, building codes etc.</dct:description>
    <ns1:superClassOf rdf:resource="Drawing"/>
    <ns1:superClassOf rdf:resource="Image"/>
    <ns1:inRangeOf>
      <owl:ObjectProperty rdf:about="forDocument">
        <rdfs:label xml:lang="en">for document</rdfs:label>
        <rdfs:comment xml:lang="en">links an entity such as a legal verifier to the document it is for.</rdfs:comment>
        <rdfs:range rdf:resource="Document"/>
        <rdfs:isDefinedBy rdf:resource="document"/>
        <dct:title xml:lang="en">for document</dct:title>
        <dct:description xml:lang="en">links an entity such as a legal verifier to the document it is for.</dct:description>
      </owl:ObjectProperty>
    </ns1:inRangeOf>
    <ns1:inRangeOf>
      <owl:ObjectProperty rdf:about="usesDocument">
        <rdfs:label xml:lang="en">uses document</rdfs:label>
        <rdfs:comment xml:lang="en">Links an entity (procedure, statement, verifier, ...) to the document it uses.</rdfs:comment>
        <rdfs:isDefinedBy rdf:resource="document"/>
        <rdfs:range rdf:resource="Document"/>
        <dct:title xml:lang="en">uses document</dct:title>
        <dct:description xml:lang="en">Links an entity (procedure, statement, verifier, ...) to the document it uses.</dct:description>
        <ns1:superPropertyOf rdf:resource="requiresDocument"/>
      </owl:ObjectProperty>
    </ns1:inRangeOf>
    <ns1:inRangeOf>
      <owl:ObjectProperty rdf:about="requiresDocument">
        <rdfs:label xml:lang="en">requires document</rdfs:label>
        <rdfs:comment xml:lang="en">Links an entity (procedure, statement, verifier, ...) to the document it requires.</rdfs:comment>
        <rdfs:isDefinedBy rdf:resource="document"/>
        <rdfs:subPropertyOf rdf:resource="usesDocument"/>
        <rdfs:range rdf:resource="Document"/>
        <dct:title xml:lang="en">requires document</dct:title>
        <dct:description xml:lang="en">Links an entity (procedure, statement, verifier, ...) to the document it requires.</dct:description>
      </owl:ObjectProperty>
    </ns1:inRangeOf>
  </owl:Class>
  <owl:Class rdf:about="DocumentSubdivision">
    <rdf:type rdf:resource="http://www.w3.org/2000/01/rdf-schema#Class"/>
    <rdfs:label xml:lang="en">Document Subdivision</rdfs:label>
    <rdfs:comment xml:lang="en">Any subdivision of a document, including sections, paragraphs, definitions, words, etc.</rdfs:comment>
    <rdfs:isDefinedBy rdf:resource="document"/>
    <rdfs:subClassOf>
      <owl:Restriction rdf:nodeID="nde74e8929339460ea8a8f35a2483d7f5b1">
        <owl:onProperty rdf:resource="hasSubdivision"/>
        <owl:allValuesFrom rdf:resource="DocumentSubdivision"/>
        <ns1:superClassOf rdf:resource="DocumentSubdivision"/>
      </owl:Restriction>
    </rdfs:subClassOf>
    <skos:example xml:lang="en">Paragraph, section, definition...</skos:example>
    <dct:title xml:lang="en">Document Subdivision</dct:title>
    <dct:description xml:lang="en">Any subdivision of a document, including sections, paragraphs, definitions, words, etc.</dct:description>
    <ns1:inDomainOf>
      <owl:DatatypeProperty rdf:about="DocumentSubdivision_asLiteral">
        <rdfs:label xml:lang="en">as literal</rdfs:label>
        <rdfs:comment xml:lang="en">Links a document subdivision to its literal representation. The literal datatype may be xsd:string, rdf:HTMLLiteral, xsd:base64Binary, or any other relevant datatype.</rdfs:comment>
        <skos:hiddenLabel>text</skos:hiddenLabel>
        <rdfs:isDefinedBy rdf:resource="document"/>
        <rdfs:domain rdf:resource="DocumentSubdivision"/>
        <rdfs:range rdf:resource="http://www.w3.org/2000/01/rdf-schema#Literal"/>
        <dct:title xml:lang="en">as literal</dct:title>
        <dct:description xml:lang="en">Links a document subdivision to its literal representation. The literal datatype may be xsd:string, rdf:HTMLLiteral, xsd:base64Binary, or any other relevant datatype.</dct:description>
      </owl:DatatypeProperty>
    </ns1:inDomainOf>
    <ns1:inDomainOf>
      <owl:ObjectProperty rdf:about="hasNextSubdivision">
        <rdf:type rdf:resource="http://www.w3.org/2002/07/owl#FunctionalProperty"/>
        <rdfs:label xml:lang="en">has next subdivision</rdfs:label>
        <rdfs:comment xml:lang="en">Links a document subdivision to the document subdivision that immediately follows it, if it exists</rdfs:comment>
        <rdfs:domain rdf:resource="DocumentSubdivision"/>
        <rdfs:range rdf:resource="DocumentSubdivision"/>
        <rdfs:isDefinedBy rdf:resource="document"/>
        <dct:title xml:lang="en">has next subdivision</dct:title>
        <dct:description xml:lang="en">Links a document subdivision to the document subdivision that immediately follows it, if it exists</dct:description>
      </owl:ObjectProperty>
    </ns1:inDomainOf>
    <ns1:inRangeOf>
      <owl:ObjectProperty rdf:about="hasSubdivision">
        <rdfs:label xml:lang="en">has subdivision</rdfs:label>
        <rdfs:comment xml:lang="en">links a document part to some of its subdivision</rdfs:comment>
        <rdfs:domain rdf:nodeID="nde74e8929339460ea8a8f35a2483d7f5b2"/>
        <rdfs:range rdf:resource="DocumentSubdivision"/>
        <rdfs:subPropertyOf rdf:resource="http://purl.org/dc/terms/hasPart"/>
        <rdfs:isDefinedBy rdf:resource="document"/>
        <dct:title xml:lang="en">has subdivision</dct:title>
        <dct:description xml:lang="en">links a document part to some of its subdivision</dct:description>
        <ns1:superPropertyOf rdf:resource="hasFirstSubdivision"/>
      </owl:ObjectProperty>
    </ns1:inRangeOf>
    <ns1:inRangeOf rdf:resource="hasNextSubdivision"/>
    <ns1:inRangeOf>
      <owl:ObjectProperty rdf:about="hasFirstSubdivision">
        <rdf:type rdf:resource="http://www.w3.org/2002/07/owl#FunctionalProperty"/>
        <rdfs:label xml:lang="en">has first subdivision</rdfs:label>
        <rdfs:comment xml:lang="en">Links a document part to the first of its subdivision</rdfs:comment>
        <rdfs:domain rdf:nodeID="nde74e8929339460ea8a8f35a2483d7f5b5"/>
        <rdfs:range rdf:resource="DocumentSubdivision"/>
        <rdfs:subPropertyOf rdf:resource="hasSubdivision"/>
        <rdfs:isDefinedBy rdf:resource="document"/>
        <dct:title xml:lang="en">has first subdivision</dct:title>
        <dct:description xml:lang="en">Links a document part to the first of its subdivision</dct:description>
      </owl:ObjectProperty>
    </ns1:inRangeOf>
  </owl:Class>
  <rdf:Description rdf:about="http://www.w3.org/2002/07/owl#ObjectProperty">
    <ns1:hasMember rdf:resource="forDocument"/>
    <ns1:hasMember rdf:resource="usesDocument"/>
    <ns1:hasMember rdf:resource="requiresDocument"/>
    <ns1:hasMember rdf:resource="hasSubdivision"/>
    <ns1:hasMember rdf:resource="hasNextSubdivision"/>
    <ns1:hasMember rdf:resource="hasFirstSubdivision"/>
  </rdf:Description>
  <owl:Class rdf:about="Drawing">
    <rdf:type rdf:resource="http://www.w3.org/2000/01/rdf-schema#Class"/>
    <rdfs:label xml:lang="en">Drawing</rdfs:label>
    <rdfs:comment xml:lang="en">Drawing is a form of visual art in which an artist uses instruments to mark paper or other two-dimensional surface. (Source: Wikipedia)</rdfs:comment>
    <rdfs:subClassOf rdf:resource="Document"/>
    <rdfs:isDefinedBy rdf:resource="document"/>
    <dct:title xml:lang="en">Drawing</dct:title>
    <dct:description xml:lang="en">Drawing is a form of visual art in which an artist uses instruments to mark paper or other two-dimensional surface. (Source: Wikipedia)</dct:description>
  </owl:Class>
  <owl:Class rdf:about="Image">
    <rdf:type rdf:resource="http://www.w3.org/2000/01/rdf-schema#Class"/>
    <rdfs:label xml:lang="en">Image</rdfs:label>
    <rdfs:comment xml:lang="en">An image is a visual representation of something. It can be two-dimensional, three-dimensional, or somehow otherwise feed into the visual system to convey information. (Source: Wikipedia)</rdfs:comment>
    <rdfs:subClassOf rdf:resource="Document"/>
    <rdfs:isDefinedBy rdf:resource="document"/>
    <dct:title xml:lang="en">Image</dct:title>
    <dct:description xml:lang="en">An image is a visual representation of something. It can be two-dimensional, three-dimensional, or somehow otherwise feed into the visual system to convey information. (Source: Wikipedia)</dct:description>
  </owl:Class>
  <rdf:Description rdf:about="http://www.w3.org/2002/07/owl#Restriction">
    <ns1:hasMember rdf:nodeID="nde74e8929339460ea8a8f35a2483d7f5b1"/>
  </rdf:Description>
  <rdf:Description rdf:about="http://www.w3.org/2002/07/owl#Class">
    <ns1:hasMember rdf:resource="Document"/>
    <ns1:hasMember rdf:resource="DocumentSubdivision"/>
    <ns1:hasMember rdf:resource="Drawing"/>
    <ns1:hasMember rdf:resource="Image"/>
    <ns1:hasMember>
      <owl:Class rdf:nodeID="nde74e8929339460ea8a8f35a2483d7f5b2">
        <owl:unionOf rdf:parseType="Collection">
          <rdf:Description rdf:about="Document"/>
          <rdf:Description rdf:about="DocumentSubdivision"/>
        </owl:unionOf>
        <ns1:inDomainOf rdf:resource="hasSubdivision"/>
      </owl:Class>
    </ns1:hasMember>
    <ns1:hasMember>
      <owl:Class rdf:nodeID="nde74e8929339460ea8a8f35a2483d7f5b5">
        <owl:unionOf rdf:parseType="Collection">
          <rdf:Description rdf:about="Document"/>
          <rdf:Description rdf:about="DocumentSubdivision"/>
        </owl:unionOf>
        <ns1:inDomainOf rdf:resource="hasFirstSubdivision"/>
      </owl:Class>
    </ns1:hasMember>
  </rdf:Description>
  <rdf:Description rdf:about="http://www.w3.org/2002/07/owl#FunctionalProperty">
    <ns1:hasMember rdf:resource="hasNextSubdivision"/>
    <ns1:hasMember rdf:resource="hasFirstSubdivision"/>
  </rdf:Description>
  <rdf:Description rdf:about="http://www.w3.org/2002/07/owl#DatatypeProperty">
    <ns1:hasMember rdf:resource="DocumentSubdivision_asLiteral"/>
  </rdf:Description>
  <prov:Agent rdf:about="http://maxime-lefrancois.info/me#"/>
  <rdf:Description rdf:about="http://www.w3.org/2002/07/owl#Ontology">
    <ns1:hasMember rdf:resource="document"/>
  </rdf:Description>
  <rdf:Description rdf:about="http://purl.org/dc/terms/hasPart">
    <ns1:superPropertyOf rdf:resource="hasSubdivision"/>
  </rdf:Description>
  <rdf:Description rdf:about="http://www.w3.org/2000/01/rdf-schema#Literal">
    <ns1:inRangeOf rdf:resource="DocumentSubdivision_asLiteral"/>
  </rdf:Description>
</rdf:RDF>
