@base <https://w3id.org/lbd/aec3po/> .
@prefix aec3po: <https://w3id.org/lbd/aec3po/> .
@prefix cc: <http://creativecommons.org/ns#> .
@prefix dct: <http://purl.org/dc/terms/> .
@prefix ns1: <https://w3id.org/profile/ontdoc/> .
@prefix owl: <http://www.w3.org/2002/07/owl#> .
@prefix prov: <http://www.w3.org/ns/prov#> .
@prefix rdfs: <http://www.w3.org/2000/01/rdf-schema#> .
@prefix skos: <http://www.w3.org/2004/02/skos/core#> .
@prefix vann: <http://purl.org/vocab/vann/> .
@prefix xsd: <http://www.w3.org/2001/XMLSchema#> .

<Evidence> a rdfs:Class,
        owl:Class ;
    rdfs:label "Evidence"@en ;
    dct:description "A resource used as an evidence for a statement"@en ;
    dct:title "Evidence"@en ;
    rdfs:comment "A resource used as an evidence for a statement"@en ;
    rdfs:isDefinedBy <evidence> ;
    skos:example "A drawing can be an evidence."@en .

<http://maxime-lefrancois.info/me#> a prov:Agent .

dct:format ns1:superPropertyOf <hasFormat> .

rdfs:Class ns1:hasMember <Evidence> .

owl:Class ns1:hasMember <Evidence> .

owl:Ontology ns1:hasMember <evidence> .

owl:ObjectProperty ns1:hasMember <hasEvidence>,
        <hasFormat> .

<Statement> ns1:inDomainOf <hasEvidence>,
        <hasFormat> .

<hasEvidence> a owl:ObjectProperty ;
    dct:description "Links a statement to a piece of evidence for that statement (assertion, statement, or claim)."@en ;
    rdfs:comment "Links a statement to a piece of evidence for that statement (assertion, statement, or claim)."@en ;
    rdfs:domain <Statement> ;
    rdfs:isDefinedBy <statement> ;
    skos:note "Unstable. Need evidence of how this property is intended to be used"@en .

<evidence> a owl:Ontology ;
    cc:license <https://creativecommons.org/licenses/by/4.0/> ;
    dct:contributor <http://maxime-lefrancois.info/me#> ;
    dct:created "2023-09-23"^^xsd:date ;
    dct:description <file:///home/runner/work/aec3po/aec3po/src/diagrams/evidence.png>,
        "The AEC3PO Evidence module describes the evidence that an actor in the compliance and permitting process needs to provide in order to prove that the requirements derived from a Statement have been met."@en ;
    dct:modified "2025-04-22"^^xsd:date ;
    dct:title "AEC3PO: evidence"@en ;
    vann:preferredNamespacePrefix "aec3po" ;
    vann:preferredNamespaceUri "https://w3id.org/lbd/aec3po/" ;
    owl:imports <statement> .

<hasFormat> a owl:ObjectProperty ;
    dct:description "Defines the format of an evidence. A sub-property of dct:format"@en ;
    rdfs:comment "Defines the format of an evidence. A sub-property of dct:format"@en ;
    rdfs:domain <Statement> ;
    rdfs:isDefinedBy <evidence> ;
    rdfs:subPropertyOf dct:format ;
    skos:example "an image, a drawing or a model can be an evidence."@en .

