<?xml version="1.0" encoding="utf-8"?>
<rdf:RDF xml:base="https://w3id.org/lbd/aec3po/"
  xmlns:rdfs="http://www.w3.org/2000/01/rdf-schema#"
  xmlns:dct="http://purl.org/dc/terms/"
  xmlns:cc="http://creativecommons.org/ns#"
  xmlns:rdf="http://www.w3.org/1999/02/22-rdf-syntax-ns#"
  xmlns:owl="http://www.w3.org/2002/07/owl#"
  xmlns:skos="http://www.w3.org/2004/02/skos/core#"
  xmlns:prov="http://www.w3.org/ns/prov#"
  xmlns:ns1="https://w3id.org/profile/ontdoc/"
  xmlns:vann="http://purl.org/vocab/vann/"
>
  <owl:ObjectProperty rdf:about="hasEvidence">
    <rdfs:comment xml:lang="en">Links a statement to a piece of evidence for that statement (assertion, statement, or claim).</rdfs:comment>
    <skos:note xml:lang="en">Unstable. Need evidence of how this property is intended to be used</skos:note>
    <rdfs:domain>
      <rdf:Description rdf:about="Statement">
        <ns1:inDomainOf rdf:resource="hasEvidence"/>
        <ns1:inDomainOf rdf:resource="hasFormat"/>
      </rdf:Description>
    </rdfs:domain>
    <rdfs:isDefinedBy rdf:resource="statement"/>
    <dct:description xml:lang="en">Links a statement to a piece of evidence for that statement (assertion, statement, or claim).</dct:description>
  </owl:ObjectProperty>
  <owl:ObjectProperty rdf:about="hasFormat">
    <rdfs:comment xml:lang="en">Defines the format of an evidence. A sub-property of dct:format</rdfs:comment>
    <skos:example xml:lang="en">an image, a drawing or a model can be an evidence.</skos:example>
    <rdfs:domain rdf:resource="Statement"/>
    <rdfs:subPropertyOf>
      <rdf:Description rdf:about="http://purl.org/dc/terms/format">
        <ns1:superPropertyOf rdf:resource="hasFormat"/>
      </rdf:Description>
    </rdfs:subPropertyOf>
    <rdfs:isDefinedBy>
      <owl:Ontology rdf:about="evidence">
        <cc:license rdf:resource="https://creativecommons.org/licenses/by/4.0/"/>
        <dct:contributor rdf:resource="http://maxime-lefrancois.info/me#"/>
        <dct:description xml:lang="en">The AEC3PO Evidence module describes the evidence that an actor in the compliance and permitting process needs to provide in order to prove that the requirements derived from a Statement have been met.</dct:description>
        <dct:description rdf:resource="file:///home/runner/work/aec3po/aec3po/src/diagrams/evidence.png"/>
        <dct:title xml:lang="en">AEC3PO: evidence</dct:title>
        <vann:preferredNamespacePrefix>aec3po</vann:preferredNamespacePrefix>
        <vann:preferredNamespaceUri>https://w3id.org/lbd/aec3po/</vann:preferredNamespaceUri>
        <owl:imports rdf:resource="statement"/>
        <dct:created rdf:datatype="http://www.w3.org/2001/XMLSchema#date">2023-09-23</dct:created>
        <dct:modified rdf:datatype="http://www.w3.org/2001/XMLSchema#date">2025-04-22</dct:modified>
      </owl:Ontology>
    </rdfs:isDefinedBy>
    <dct:description xml:lang="en">Defines the format of an evidence. A sub-property of dct:format</dct:description>
  </owl:ObjectProperty>
  <rdf:Description rdf:about="http://www.w3.org/2002/07/owl#Ontology">
    <ns1:hasMember rdf:resource="evidence"/>
  </rdf:Description>
  <rdf:Description rdf:about="http://www.w3.org/2002/07/owl#Class">
    <ns1:hasMember rdf:resource="Evidence"/>
  </rdf:Description>
  <rdf:Description rdf:about="http://www.w3.org/2002/07/owl#ObjectProperty">
    <ns1:hasMember rdf:resource="hasEvidence"/>
    <ns1:hasMember rdf:resource="hasFormat"/>
  </rdf:Description>
  <owl:Class rdf:about="Evidence">
    <rdf:type>
      <rdf:Description rdf:about="http://www.w3.org/2000/01/rdf-schema#Class">
        <ns1:hasMember rdf:resource="Evidence"/>
      </rdf:Description>
    </rdf:type>
    <rdfs:label xml:lang="en">Evidence</rdfs:label>
    <rdfs:comment xml:lang="en">A resource used as an evidence for a statement</rdfs:comment>
    <skos:example xml:lang="en">A drawing can be an evidence.</skos:example>
    <rdfs:isDefinedBy rdf:resource="evidence"/>
    <dct:title xml:lang="en">Evidence</dct:title>
    <dct:description xml:lang="en">A resource used as an evidence for a statement</dct:description>
  </owl:Class>
  <prov:Agent rdf:about="http://maxime-lefrancois.info/me#"/>
</rdf:RDF>
