@prefix aec3po: <https://w3id.org/lbd/aec3po/> .
@prefix cc: <http://creativecommons.org/ns#> .
@prefix dct: <http://purl.org/dc/terms/> .
@prefix dul: <http://www.ontologydesignpatterns.org/ont/dul/DUL.owl#> .
@prefix owl: <http://www.w3.org/2002/07/owl#> .
@prefix rdfs: <http://www.w3.org/2000/01/rdf-schema#> .
@prefix skos: <http://www.w3.org/2004/02/skos/core#> .
@prefix vann: <http://purl.org/vocab/vann/> .
@prefix xsd: <http://www.w3.org/2001/XMLSchema#> .

aec3po:evidence a owl:Ontology ;
    cc:license <https://creativecommons.org/licenses/by/4.0/> ;
    dct:contributor <http://maxime-lefrancois.info/me#> ;
    dct:description """The AEC3PO Evidence module describes the evidence that an actor in the compliance and permitting process needs to provide in order to prove that the requirements derived from a Statement have been met."""@en ;
    dct:description <Evidence.png> ;
    dct:title "AEC3PO: evidence"@en ;
    vann:preferredNamespacePrefix "aec3po" ;
    vann:preferredNamespaceUri "https://w3id.org/lbd/aec3po/" ;
    owl:imports aec3po:statement .

aec3po:Evidence a owl:Class ;
 rdfs:label "Evidence"@en ;
 rdfs:comment "A resource used as an evidence for a statement"@en ;
 skos:example "A drawing can be an evidence."@en ;
 rdfs:isDefinedBy aec3po:evidence .

aec3po:hasEvidence a owl:ObjectProperty;
 rdfs:comment "Links a statement to a piece of evidence for that statement (assertion, statement, or claim)."@en ;
 skos:note "Unstable. Need evidence of how this property is intended to be used"@en ;
 rdfs:domain aec3po:Statement ;
 rdfs:isDefinedBy aec3po:statement .

 aec3po:hasFormat a owl:ObjectProperty;
    rdfs:comment "Defines the format of an evidence, which is of type dct:format."@en ;
    skos:example "an image, a drawing or a model can be an evidence."@en ;
    rdfs:domain aec3po:Statement ;
    rdfs:range dct:format;
    rdfs:isDefinedBy aec3po:evidence .

