<?xml version="1.0" encoding="utf-8"?>
<rdf:RDF xml:base="https://w3id.org/lbd/aec3po/"
  xmlns:rdfs="http://www.w3.org/2000/01/rdf-schema#"
  xmlns:ns1="https://w3id.org/profile/ontdoc/"
  xmlns:rdf="http://www.w3.org/1999/02/22-rdf-syntax-ns#"
  xmlns:dct="http://purl.org/dc/terms/"
  xmlns:cc="http://creativecommons.org/ns#"
  xmlns:owl="http://www.w3.org/2002/07/owl#"
  xmlns:skos="http://www.w3.org/2004/02/skos/core#"
  xmlns:prov="http://www.w3.org/ns/prov#"
  xmlns:vann="http://purl.org/vocab/vann/"
>
  <owl:ObjectProperty rdf:about="hasQuantityKind">
    <rdfs:label xml:lang="en">has quantity kind</rdfs:label>
    <rdfs:comment xml:lang="en">Links a property to its quantity kind</rdfs:comment>
    <rdfs:domain rdf:resource="Property"/>
    <rdfs:range rdf:resource="QuantityKind"/>
    <rdfs:isDefinedBy>
      <owl:Ontology rdf:about="feature_of_interest">
        <cc:license rdf:resource="https://creativecommons.org/licenses/by/4.0/"/>
        <dct:contributor rdf:resource="http://maxime-lefrancois.info/me#"/>
        <dct:description xml:lang="en">The AEC3PO Feature of Interest module describes an entity (feature) of a site, building, or piece of infrastructure that is of interest. Typically, this will be a building component that needs to be compliant to regulations, or be documented in the permitting process. .</dct:description>
        <dct:modified rdf:datatype="http://www.w3.org/2001/XMLSchema#date">2023-05-25</dct:modified>
        <dct:modified rdf:datatype="http://www.w3.org/2001/XMLSchema#date">2024-02-28</dct:modified>
        <dct:title xml:lang="en">AEC3PO: Feature of Interest</dct:title>
        <owl:imports rdf:resource="quantity_kinds"/>
        <vann:preferredNamespacePrefix>aec3po</vann:preferredNamespacePrefix>
        <vann:preferredNamespaceUri>https://w3id.org/lbd/aec3po/</vann:preferredNamespaceUri>
        <dct:created rdf:datatype="http://www.w3.org/2001/XMLSchema#date">2023-05-25</dct:created>
      </owl:Ontology>
    </rdfs:isDefinedBy>
    <skos:example xml:lang="en">A space area property to the property kind "area".</skos:example>
    <dct:title xml:lang="en">has quantity kind</dct:title>
    <dct:description xml:lang="en">Links a property to its quantity kind</dct:description>
  </owl:ObjectProperty>
  <rdf:Description rdf:about="http://www.w3.org/2000/01/rdf-schema#Class">
    <ns1:hasMember rdf:resource="FeatureOfInterest"/>
    <ns1:hasMember rdf:resource="Property"/>
    <ns1:hasMember rdf:resource="QuantityKind"/>
  </rdf:Description>
  <owl:Class rdf:about="FeatureOfInterest">
    <rdf:type rdf:resource="http://www.w3.org/2000/01/rdf-schema#Class"/>
    <rdfs:label xml:lang="en">Feature Of Interest</rdfs:label>
    <rdfs:comment xml:lang="en">The object whose conformance against checks is verified.</rdfs:comment>
    <rdfs:isDefinedBy rdf:resource="feature_of_interest"/>
    <rdfs:subClassOf>
      <rdf:Description rdf:about="http://www.ontologydesignpatterns.org/ont/dul/DUL.owl#Object">
        <ns1:superClassOf rdf:resource="FeatureOfInterest"/>
      </rdf:Description>
    </rdfs:subClassOf>
    <rdfs:subClassOf>
      <rdf:Description rdf:about="https://saref.etsi.org/core/FeatureOfInterest">
        <ns1:superClassOf rdf:resource="FeatureOfInterest"/>
      </rdf:Description>
    </rdfs:subClassOf>
    <skos:example xml:lang="en">A building, a building space, a building element, the set of columns in a building, ...</skos:example>
    <skos:note xml:lang="en">It is expected that classes in other ontologies are used to multi-type instances of FeatureOfInterest.
  For example a feature of interest may also be:
  - a bot:Zone or a bot:Element
  - a ifc:IfcRamp, a ifc:IfcSurfaceFeature</skos:note>
    <dct:title xml:lang="en">Feature Of Interest</dct:title>
    <dct:description xml:lang="en">The object whose conformance against checks is verified.</dct:description>
    <ns1:inDomainOf>
      <owl:ObjectProperty rdf:about="hasProperty">
        <rdfs:label xml:lang="en">has Property</rdfs:label>
        <rdfs:comment xml:lang="en">Links a feature of interest to one of its aspect that is intrinsic to and cannot exist without it.</rdfs:comment>
        <rdfs:domain rdf:resource="FeatureOfInterest"/>
        <rdfs:isDefinedBy rdf:resource="feature_of_interest"/>
        <rdfs:range rdf:resource="Property"/>
        <skos:example xml:lang="en">Links a space to the area property of that space, a wall to the U-value property of that wall...</skos:example>
        <dct:title xml:lang="en">has Property</dct:title>
        <dct:description xml:lang="en">Links a feature of interest to one of its aspect that is intrinsic to and cannot exist without it.</dct:description>
      </owl:ObjectProperty>
    </ns1:inDomainOf>
  </owl:Class>
  <rdf:Description rdf:about="http://www.w3.org/2002/07/owl#Class">
    <ns1:hasMember rdf:resource="FeatureOfInterest"/>
    <ns1:hasMember rdf:resource="Property"/>
    <ns1:hasMember rdf:resource="QuantityKind"/>
  </rdf:Description>
  <owl:Class rdf:about="Property">
    <rdf:type rdf:resource="http://www.w3.org/2000/01/rdf-schema#Class"/>
    <rdfs:label xml:lang="en">Property</rdfs:label>
    <rdfs:comment xml:lang="en">An aspect of a feature of interest that is intrinsic to and cannot exist without the feature of interest.</rdfs:comment>
    <rdfs:isDefinedBy rdf:resource="feature_of_interest"/>
    <rdfs:subClassOf>
      <rdf:Description rdf:about="http://www.ontologydesignpatterns.org/ont/dul/DUL.owl#Quality">
        <ns1:superClassOf rdf:resource="Property"/>
      </rdf:Description>
    </rdfs:subClassOf>
    <skos:example xml:lang="en">The height of a building, the area of a space, the U-value of a wall</skos:example>
    <dct:title xml:lang="en">Property</dct:title>
    <dct:description xml:lang="en">An aspect of a feature of interest that is intrinsic to and cannot exist without the feature of interest.</dct:description>
    <ns1:inDomainOf rdf:resource="hasQuantityKind"/>
    <ns1:inRangeOf rdf:resource="hasProperty"/>
  </owl:Class>
  <owl:Class rdf:about="QuantityKind">
    <rdf:type rdf:resource="http://www.w3.org/2000/01/rdf-schema#Class"/>
    <rdfs:label xml:lang="en">Quantity Kind</rdfs:label>
    <rdfs:comment xml:lang="en">A kind of quantity.</rdfs:comment>
    <rdfs:isDefinedBy rdf:resource="feature_of_interest"/>
    <skos:example xml:lang="en">height, area, U-value</skos:example>
    <dct:title xml:lang="en">Quantity Kind</dct:title>
    <dct:description xml:lang="en">A kind of quantity.</dct:description>
    <ns1:inRangeOf rdf:resource="hasQuantityKind"/>
  </owl:Class>
  <prov:Agent rdf:about="http://maxime-lefrancois.info/me#"/>
  <rdf:Description rdf:about="http://www.w3.org/2002/07/owl#ObjectProperty">
    <ns1:hasMember rdf:resource="hasProperty"/>
    <ns1:hasMember rdf:resource="hasQuantityKind"/>
  </rdf:Description>
  <rdf:Description rdf:about="http://www.w3.org/2002/07/owl#Ontology">
    <ns1:hasMember rdf:resource="feature_of_interest"/>
  </rdf:Description>
</rdf:RDF>
