<?xml version="1.0" encoding="utf-8"?>
<rdf:RDF xml:base="https://w3id.org/lbd/aec3po/"
  xmlns:owl="http://www.w3.org/2002/07/owl#"
  xmlns:rdfs="http://www.w3.org/2000/01/rdf-schema#"
  xmlns:cc="http://creativecommons.org/ns#"
  xmlns:dct="http://purl.org/dc/terms/"
  xmlns:vann="http://purl.org/vocab/vann/"
  xmlns:rdf="http://www.w3.org/1999/02/22-rdf-syntax-ns#"
>
  <owl:Class rdf:about="PrivateVerifier">
    <rdfs:label xml:lang="en">Private Verifier</rdfs:label>
    <rdfs:comment xml:lang="en">Private verifier refers to an individual or organisation in the private sector, responsible for independently assessing and verifying compliance with regulatory, safety, quality, and design requirements in a construction project. </rdfs:comment>
    <rdfs:subClassOf rdf:resource="LegalVerifier"/>
    <rdfs:isDefinedBy>
      <owl:Ontology rdf:about="legal_verifier">
        <cc:license rdf:resource="https://creativecommons.org/licenses/by/4.0/"/>
        <dct:contributor rdf:resource="http://maxime-lefrancois.info/me#"/>
        <dct:description xml:lang="en">The AEC3PO Legal Verifier module describes actors of the compliance and permitting process that have the legal capacity to verify that a specific Statement of a compliance document has been met in a satisfactory manner.</dct:description>
        <dct:description rdf:resource="file:///home/runner/work/aec3po/aec3po/src/diagrams/legal_verifier.png"/>
        <dct:modified rdf:datatype="http://www.w3.org/2001/XMLSchema#date">2023-08-31</dct:modified>
        <dct:modified rdf:datatype="http://www.w3.org/2001/XMLSchema#date">2025-04-22</dct:modified>
        <dct:title xml:lang="en">AEC3PO: legal verifier</dct:title>
        <vann:preferredNamespacePrefix>aec3po</vann:preferredNamespacePrefix>
        <vann:preferredNamespaceUri>https://w3id.org/lbd/aec3po/</vann:preferredNamespaceUri>
        <dct:created rdf:datatype="http://www.w3.org/2001/XMLSchema#date">2023-08-31</dct:created>
      </owl:Ontology>
    </rdfs:isDefinedBy>
  </owl:Class>
  <owl:Class rdf:about="StateVerifier">
    <rdfs:label xml:lang="en">State Verifier</rdfs:label>
    <rdfs:comment xml:lang="en">State verifier refers to an individual or organisation in the greater State sector, responsible for assessing and verifying compliance with regulations, legal requirements, and building codes in a construction project. </rdfs:comment>
    <rdfs:subClassOf rdf:resource="LegalVerifier"/>
    <rdfs:isDefinedBy rdf:resource="legal_verifier"/>
  </owl:Class>
  <owl:Class rdf:about="LegalVerifier">
    <rdfs:label xml:lang="en">Legal Verifier</rdfs:label>
    <rdfs:subClassOf rdf:resource="http://xmlns.com/foaf/0.1/Agent"/>
    <rdfs:subClassOf>
      <rdf:Description rdf:nodeID="n7261e10b18c34890bee605e0572b4eaab1">
        <owl:onProperty rdf:resource="forDocument"/>
        <owl:allValuesFrom rdf:resource="Document"/>
      </rdf:Description>
    </rdfs:subClassOf>
    <rdfs:comment xml:lang="en">An entity that has the legal capacity to verify compliance with this regulation.</rdfs:comment>
    <rdfs:isDefinedBy rdf:resource="legal_verifier"/>
  </owl:Class>
</rdf:RDF>
