<?xml version="1.0" encoding="utf-8"?>
<rdf:RDF xml:base="https://w3id.org/lbd/aec3po/"
  xmlns:dct="http://purl.org/dc/terms/"
  xmlns:vann="http://purl.org/vocab/vann/"
  xmlns:rdfs="http://www.w3.org/2000/01/rdf-schema#"
  xmlns:owl="http://www.w3.org/2002/07/owl#"
  xmlns:rdf="http://www.w3.org/1999/02/22-rdf-syntax-ns#"
  xmlns:cc="http://creativecommons.org/ns#"
>
  <owl:ObjectProperty rdf:about="locationCoverage">
    <rdfs:label xml:lang="en">location coverage</rdfs:label>
    <rdfs:comment xml:lang="en">The spatialCoverage indicates the place(s) or the administrative areas which are the focus of the BIM model.</rdfs:comment>
    <rdfs:domain rdf:resource="https://schema.org/Model"/>
    <rdfs:range>
      <owl:Class rdf:nodeID="n8560b7bf7add47f8831e1aca8337c2b4b1">
        <owl:unionOf rdf:parseType="Collection">
          <rdf:Description rdf:about="https://schema.org/Place"/>
          <rdf:Description rdf:about="AdministrativeArea"/>
        </owl:unionOf>
      </owl:Class>
    </rdfs:range>
    <owl:equivalentProperty rdf:resource="https://schema.org/spatialCoverage"/>
  </owl:ObjectProperty>
  <owl:ObjectProperty rdf:about="hasDimension">
    <rdfs:label xml:lang="en">has dimension</rdfs:label>
    <rdfs:comment xml:lang="en">is used to represent the physical dimensions or measurements of an object, entity, or element within the BIM model. </rdfs:comment>
    <rdfs:domain rdf:resource="Model"/>
    <rdfs:range rdf:resource="Dimension"/>
  </owl:ObjectProperty>
  <owl:Class rdf:about="Element">
    <rdfs:label xml:lang="en">Element</rdfs:label>
    <rdfs:subClassOf rdf:resource="Model"/>
    <rdfs:comment>Specific attributes of individual elements, such as doors, windows, walls, etc.</rdfs:comment>
    <rdfs:isDefinedBy>
      <owl:Ontology rdf:about="model">
        <cc:license rdf:resource="https://creativecommons.org/licenses/by/4.0/"/>
        <dct:contributor rdf:resource="amna"/>
        <dct:description xml:lang="en">The AEC3PO model module describes a model representing part or the entirety of a site, building, or piece of infrastructure. Typically, this will be in the form of a Building Information Model.</dct:description>
        <dct:modified rdf:datatype="http://www.w3.org/2001/XMLSchema#date">2023-08-15</dct:modified>
        <dct:modified rdf:datatype="http://www.w3.org/2001/XMLSchema#date">2024-02-28</dct:modified>
        <dct:title xml:lang="en">AEC3PO:Model</dct:title>
        <owl:imports rdf:resource="evidence"/>
        <vann:preferredNamespacePrefix>aec3po</vann:preferredNamespacePrefix>
        <vann:preferredNamespaceUri>https://w3id.org/lbd/aec3po/</vann:preferredNamespaceUri>
        <dct:created rdf:datatype="http://www.w3.org/2001/XMLSchema#date">2023-08-16</dct:created>
      </owl:Ontology>
    </rdfs:isDefinedBy>
  </owl:Class>
  <owl:ObjectProperty rdf:about="location">
    <rdfs:label xml:lang="en">location</rdfs:label>
    <rdfs:comment xml:lang="en">The physical or geographic location of the building or structure represented in the BIM model.</rdfs:comment>
    <rdfs:domain rdf:resource="https://schema.org/Model"/>
    <rdfs:range rdf:resource="https://schema.org/Place"/>
    <owl:equivalentProperty rdf:resource="https://schema.org/spatial"/>
  </owl:ObjectProperty>
  <owl:DatatypeProperty rdf:about="material">
    <rdfs:label xml:lang="en">material</rdfs:label>
    <rdfs:comment xml:lang="en">The materials used for different parts of the building, such as walls, floors, and roofs.</rdfs:comment>
    <rdfs:domain rdf:resource="https://schema.org/Model"/>
    <rdfs:range rdf:resource="http://www.w3.org/2001/XMLSchema#string"/>
    <owl:equivalentProperty rdf:resource="https://schema.org/material"/>
  </owl:DatatypeProperty>
  <owl:ObjectProperty rdf:about="hasBuildingPhase">
    <rdfs:label xml:lang="en">has building phase</rdfs:label>
    <rdfs:comment xml:lang="en">describes the relationship between a construction-related entity and the phase of the building process it is associated with. (Inspired by the BIM shared ontology)</rdfs:comment>
    <rdfs:domain rdf:resource="Model"/>
    <rdfs:range rdf:resource="Phase"/>
  </owl:ObjectProperty>
  <owl:DatatypeProperty rdf:about="name">
    <rdfs:label xml:lang="en">name</rdfs:label>
    <rdfs:comment xml:lang="en">The name or the identifier of the BIM model.</rdfs:comment>
    <rdfs:domain rdf:resource="https://schema.org/Model"/>
    <rdfs:range rdf:resource="http://www.w3.org/2001/XMLSchema#string"/>
    <owl:inverseOf rdf:resource="https://schema.org/subjectOf"/>
    <owl:equivalentProperty rdf:resource="https://schema.org/about"/>
  </owl:DatatypeProperty>
  <owl:ObjectProperty rdf:about="hasElementPhase">
    <rdfs:label xml:lang="en">has element phase</rdfs:label>
    <rdfs:comment xml:lang="en">is used to establish a relationship between a construction element or component and the specific phase of the building process in which that element is relevant or applicable. (Inspired by the BIM shared ontology)</rdfs:comment>
    <rdfs:domain rdf:resource="Model"/>
    <rdfs:range rdf:resource="Phase"/>
  </owl:ObjectProperty>
  <owl:ObjectProperty rdf:about="hasClassification">
    <rdfs:label xml:lang="en">has dimension</rdfs:label>
    <rdfs:comment xml:lang="en">is used to link building components, elements, or other entities to a classification scheme that provides a standardised way of categorising and organising them.. </rdfs:comment>
    <rdfs:domain rdf:resource="Model"/>
    <rdfs:range rdf:resource="Classification"/>
  </owl:ObjectProperty>
  <owl:DatatypeProperty rdf:about="description">
    <rdfs:label xml:lang="en">description</rdfs:label>
    <rdfs:comment xml:lang="en">A textual description providing additional details about the BIM model.</rdfs:comment>
    <rdfs:domain rdf:resource="https://schema.org/Model"/>
    <rdfs:range rdf:resource="http://www.w3.org/2001/XMLSchema#string"/>
    <owl:equivalentProperty rdf:resource="https://schema.org/abstract"/>
  </owl:DatatypeProperty>
  <owl:Class rdf:about="Dimension">
    <rdfs:label xml:lang="en">Dimension</rdfs:label>
    <rdfs:subClassOf rdf:resource="Model"/>
    <rdfs:comment>Measurements and sizes of various building components and elements.</rdfs:comment>
    <rdfs:isDefinedBy rdf:resource="model"/>
  </owl:Class>
  <owl:Class rdf:about="Phase">
    <rdfs:label xml:lang="en">Phase</rdfs:label>
    <rdfs:subClassOf rdf:resource="Model"/>
    <rdfs:comment>A construction or renovation phase the building model may represent. Inspired by the BIM Shared Ontology (https://www.sciencedirect.com/science/article/pii/S0926580517302364)</rdfs:comment>
    <rdfs:isDefinedBy rdf:resource="model"/>
  </owl:Class>
  <owl:Class rdf:about="Classification">
    <rdfs:label xml:lang="en">Classification</rdfs:label>
    <rdfs:subClassOf rdf:resource="Model"/>
    <rdfs:comment>Classification systems or codes used to categorise and organise building components.</rdfs:comment>
    <rdfs:isDefinedBy rdf:resource="model"/>
  </owl:Class>
  <owl:Class rdf:about="Model">
    <rdfs:label xml:lang="en">Model</rdfs:label>
    <rdfs:comment>A BIM model is a digital representation of a building or infrastructure project that includes both graphical and non-graphical information.</rdfs:comment>
    <rdfs:isDefinedBy rdf:resource="model"/>
  </owl:Class>
</rdf:RDF>
