<?xml version="1.0" encoding="utf-8"?>
<rdf:RDF xml:base="https://w3id.org/lbd/aec3po/"
  xmlns:owl="http://www.w3.org/2002/07/owl#"
  xmlns:rdfs="http://www.w3.org/2000/01/rdf-schema#"
  xmlns:dct="http://purl.org/dc/terms/"
  xmlns:skos="http://www.w3.org/2004/02/skos/core#"
  xmlns:rdf="http://www.w3.org/1999/02/22-rdf-syntax-ns#"
  xmlns:cc="http://creativecommons.org/ns#"
  xmlns:vann="http://purl.org/vocab/vann/"
>
  <owl:ObjectProperty rdf:about="appliesTo">
    <rdfs:label xml:lang="en">applies to</rdfs:label>
    <rdfs:comment xml:lang="en">Links a check statement to the expression of a thing it applies to, as per the Requirement Application Selection and Exception (RASE) methodology.</rdfs:comment>
    <skos:note xml:lang="en">Usually, the Applies/Application statements are highlighted in green.</skos:note>
    <rdfs:subPropertyOf rdf:resource="hasSubdivision"/>
    <rdfs:domain rdf:resource="CheckStatement"/>
    <rdfs:range rdf:resource="ApplicationStatement"/>
    <rdfs:isDefinedBy>
      <owl:Ontology rdf:about="rase_statement">
        <cc:license rdf:resource="https://creativecommons.org/licenses/by/4.0/"/>
        <dct:contributor rdf:resource="http://maxime-lefrancois.info/me#"/>
        <dct:description xml:lang="en">The AEC3PO RASE Statement module describes statements decomposed following the Requirement Application Selection and Exception (RASE) methodology.</dct:description>
        <dct:description rdf:resource="file:///home/runner/work/aec3po/aec3po/src/diagrams/rase_statement.png"/>
        <dct:title xml:lang="en">AEC3PO: RASE statement</dct:title>
        <vann:preferredNamespacePrefix>aec3po</vann:preferredNamespacePrefix>
        <vann:preferredNamespaceUri>https://w3id.org/lbd/aec3po/</vann:preferredNamespaceUri>
        <owl:imports rdf:resource="statement"/>
        <dct:created rdf:datatype="http://www.w3.org/2001/XMLSchema#date">2023-09-07</dct:created>
        <dct:modified rdf:datatype="http://www.w3.org/2001/XMLSchema#date">2025-04-22</dct:modified>
      </owl:Ontology>
    </rdfs:isDefinedBy>
  </owl:ObjectProperty>
  <owl:ObjectProperty rdf:about="selects">
    <rdfs:label xml:lang="en">selects</rdfs:label>
    <rdfs:comment xml:lang="en">Links a check statement to the expression of a thing that is selected by the check, as per the Requirement Application Selection and Exception (RASE) methodology.</rdfs:comment>
    <skos:note xml:lang="en">Usually, the Select/Selection statements are highlighted in purple.</skos:note>
    <rdfs:subPropertyOf rdf:resource="hasSubdivision"/>
    <rdfs:domain rdf:resource="CheckStatement"/>
    <rdfs:range rdf:resource="RequirementStatement"/>
    <rdfs:isDefinedBy rdf:resource="rase_statement"/>
  </owl:ObjectProperty>
  <owl:ObjectProperty rdf:about="requires">
    <rdfs:label xml:lang="en">requires</rdfs:label>
    <rdfs:comment xml:lang="en">Links a check statement to the expression of a thing that is required by the check, as per the Requirement Application Selection and Exception (RASE) methodology.</rdfs:comment>
    <skos:note xml:lang="en">Usually, the Required/Requirement statements are highlighted in blue.</skos:note>
    <rdfs:subPropertyOf rdf:resource="hasSubdivision"/>
    <rdfs:domain rdf:resource="CheckStatement"/>
    <rdfs:range rdf:resource="RequirementStatement"/>
    <rdfs:isDefinedBy rdf:resource="rase_statement"/>
  </owl:ObjectProperty>
  <owl:AllDifferent rdf:nodeID="n8976c6a81c234939a554a997756f909ab1">
    <owl:members rdf:parseType="Collection">
      <rdf:Description rdf:about="ApplicationStatement"/>
      <rdf:Description rdf:about="SelectionStatement"/>
      <rdf:Description rdf:about="RequirementStatement"/>
      <rdf:Description rdf:about="ExceptionStatement"/>
    </owl:members>
  </owl:AllDifferent>
  <owl:ObjectProperty rdf:about="except">
    <rdfs:label xml:lang="en">except</rdfs:label>
    <rdfs:comment xml:lang="en">Links a check statement to the expression of a thing that is excepted by the check, as per the Requirement Application Selection and Exception (RASE) methodology.</rdfs:comment>
    <skos:note xml:lang="en">Usually, the Excepted/Exception statements are highlighted in yellow.</skos:note>
    <rdfs:subPropertyOf rdf:resource="hasSubdivision"/>
    <rdfs:domain rdf:resource="CheckStatement"/>
    <rdfs:range rdf:resource="ExceptionStatement"/>
    <rdfs:isDefinedBy rdf:resource="rase_statement"/>
  </owl:ObjectProperty>
  <owl:Class rdf:about="SelectionStatement">
    <rdfs:label xml:lang="en">Selection Statement</rdfs:label>
    <rdfs:comment xml:lang="en">Represents the Selection tag in the semantic mark-up Requirements Applications Selections and Exceptions (RASE) methodology.</rdfs:comment>
    <skos:note xml:lang="en">Usually, the Select/Selection statements are highlighted in purple.</skos:note>
    <rdfs:subClassOf rdf:resource="Statement"/>
    <rdfs:isDefinedBy rdf:resource="rase_statement"/>
  </owl:Class>
  <owl:Class rdf:about="RequirementStatement">
    <rdfs:label xml:lang="en">Requirement Statement</rdfs:label>
    <rdfs:comment xml:lang="en">Represents the Requirement tag in the semantic mark-up Requirement Application Selection and Exception (RASE) methodology.</rdfs:comment>
    <skos:note xml:lang="en">Usually, the Required/Requirement statements are highlighted in blue.</skos:note>
    <rdfs:subClassOf rdf:resource="Statement"/>
    <rdfs:isDefinedBy rdf:resource="rase_statement"/>
  </owl:Class>
  <owl:Class rdf:about="ApplicationStatement">
    <rdfs:label xml:lang="en">ApplicationStatement</rdfs:label>
    <rdfs:comment xml:lang="en">Represents the Applications tag in the semantic mark-up Requirement Application Selection and Exception (RASE) methodology.</rdfs:comment>
    <skos:note xml:lang="en">Usually, the Applies/Application statements are highlighted in green.</skos:note>
    <rdfs:subClassOf rdf:resource="Statement"/>
    <rdfs:isDefinedBy rdf:resource="rase_statement"/>
  </owl:Class>
  <owl:Class rdf:about="ExceptionStatement">
    <rdfs:label xml:lang="en">Exception Statement</rdfs:label>
    <rdfs:comment xml:lang="en">Represents the Exception tag in the semantic mark-up Requirement Application Selection and Exception (RASE) methodology.</rdfs:comment>
    <skos:note xml:lang="en">Usually, the Excepted/Exception statements are highlighted in yellow.</skos:note>
    <rdfs:subClassOf rdf:resource="Statement"/>
    <rdfs:isDefinedBy rdf:resource="rase_statement"/>
  </owl:Class>
</rdf:RDF>
