@base <https://w3id.org/lbd/aec3po/> .
@prefix aec3po: <https://w3id.org/lbd/aec3po/> .
@prefix cc: <http://creativecommons.org/ns#> .
@prefix dct: <http://purl.org/dc/terms/> .
@prefix owl: <http://www.w3.org/2002/07/owl#> .
@prefix rdf: <http://www.w3.org/1999/02/22-rdf-syntax-ns#> .
@prefix rdfs: <http://www.w3.org/2000/01/rdf-schema#> .
@prefix skos: <http://www.w3.org/2004/02/skos/core#> .
@prefix vann: <http://purl.org/vocab/vann/> .
@prefix xsd: <http://www.w3.org/2001/XMLSchema#> .

<appliesTo> a owl:ObjectProperty ;
    rdfs:label "applies to"@en ;
    rdfs:comment "Links a check statement to the expression of a thing it applies to, as per the Requirement Application Selection and Exception (RASE) methodology."@en ;
    rdfs:domain <CheckStatement> ;
    rdfs:isDefinedBy <rase_statement> ;
    rdfs:range <ApplicationStatement> ;
    rdfs:subPropertyOf <hasSubdivision> ;
    skos:note "Usually, the Applies/Application statements are highlighted in green."@en .

<except> a owl:ObjectProperty ;
    rdfs:label "except"@en ;
    rdfs:comment "Links a check statement to the expression of a thing that is excepted by the check, as per the Requirement Application Selection and Exception (RASE) methodology."@en ;
    rdfs:domain <CheckStatement> ;
    rdfs:isDefinedBy <rase_statement> ;
    rdfs:range <ExceptionStatement> ;
    rdfs:subPropertyOf <hasSubdivision> ;
    skos:note "Usually, the Excepted/Exception statements are highlighted in yellow."@en .

<requires> a owl:ObjectProperty ;
    rdfs:label "requires"@en ;
    rdfs:comment "Links a check statement to the expression of a thing that is required by the check, as per the Requirement Application Selection and Exception (RASE) methodology."@en ;
    rdfs:domain <CheckStatement> ;
    rdfs:isDefinedBy <rase_statement> ;
    rdfs:range <RequirementStatement> ;
    rdfs:subPropertyOf <hasSubdivision> ;
    skos:note "Usually, the Required/Requirement statements are highlighted in blue."@en .

<selects> a owl:ObjectProperty ;
    rdfs:label "selects"@en ;
    rdfs:comment "Links a check statement to the expression of a thing that is selected by the check, as per the Requirement Application Selection and Exception (RASE) methodology."@en ;
    rdfs:domain <CheckStatement> ;
    rdfs:isDefinedBy <rase_statement> ;
    rdfs:range <RequirementStatement> ;
    rdfs:subPropertyOf <hasSubdivision> ;
    skos:note "Usually, the Select/Selection statements are highlighted in purple."@en .

<SelectionStatement> a owl:Class ;
    rdfs:label "Selection Statement"@en ;
    rdfs:comment "Represents the Selection tag in the semantic mark-up Requirements Applications Selections and Exceptions (RASE) methodology."@en ;
    rdfs:isDefinedBy <rase_statement> ;
    rdfs:subClassOf <Statement> ;
    skos:note "Usually, the Select/Selection statements are highlighted in purple."@en .

<ApplicationStatement> a owl:Class ;
    rdfs:label "ApplicationStatement"@en ;
    rdfs:comment "Represents the Applications tag in the semantic mark-up Requirement Application Selection and Exception (RASE) methodology."@en ;
    rdfs:isDefinedBy <rase_statement> ;
    rdfs:subClassOf <Statement> ;
    skos:note "Usually, the Applies/Application statements are highlighted in green."@en .

<ExceptionStatement> a owl:Class ;
    rdfs:label "Exception Statement"@en ;
    rdfs:comment "Represents the Exception tag in the semantic mark-up Requirement Application Selection and Exception (RASE) methodology."@en ;
    rdfs:isDefinedBy <rase_statement> ;
    rdfs:subClassOf <Statement> ;
    skos:note "Usually, the Excepted/Exception statements are highlighted in yellow."@en .

<RequirementStatement> a owl:Class ;
    rdfs:label "Requirement Statement"@en ;
    rdfs:comment "Represents the Requirement tag in the semantic mark-up Requirement Application Selection and Exception (RASE) methodology."@en ;
    rdfs:isDefinedBy <rase_statement> ;
    rdfs:subClassOf <Statement> ;
    skos:note "Usually, the Required/Requirement statements are highlighted in blue."@en .

<rase_statement> a owl:Ontology ;
    cc:license <https://creativecommons.org/licenses/by/4.0/> ;
    dct:contributor <http://maxime-lefrancois.info/me#> ;
    dct:created "2023-09-07"^^xsd:date ;
    dct:description <file:///home/runner/work/aec3po/aec3po/src/diagrams/rase_statement.png>,
        "The AEC3PO RASE Statement module describes statements decomposed following the Requirement Application Selection and Exception (RASE) methodology."@en ;
    dct:modified "2025-04-22"^^xsd:date ;
    dct:title "AEC3PO: RASE statement"@en ;
    vann:preferredNamespacePrefix "aec3po" ;
    vann:preferredNamespaceUri "https://w3id.org/lbd/aec3po/" ;
    owl:imports <statement> .

[] a owl:AllDifferent ;
    owl:members ( <ApplicationStatement> <SelectionStatement> <RequirementStatement> <ExceptionStatement> ) .

