<?xml version="1.0" encoding="utf-8"?>
<rdf:RDF xml:base="https://w3id.org/lbd/aec3po/"
  xmlns:owl="http://www.w3.org/2002/07/owl#"
  xmlns:rdfs="http://www.w3.org/2000/01/rdf-schema#"
  xmlns:dct="http://purl.org/dc/terms/"
  xmlns:skos="http://www.w3.org/2004/02/skos/core#"
  xmlns:rdf="http://www.w3.org/1999/02/22-rdf-syntax-ns#"
  xmlns:cc="http://creativecommons.org/ns#"
  xmlns:vann="http://purl.org/vocab/vann/"
>
  <owl:ObjectProperty rdf:about="hasInlinePart">
    <rdfs:label xml:lang="en">hasInlinePart</rdfs:label>
    <rdfs:comment xml:lang="en">Links a statement to an inline subdivision of that statement.</rdfs:comment>
    <rdfs:subPropertyOf rdf:resource="http://purl.org/dc/terms/hasPart"/>
    <rdfs:seeAlso rdf:resource="https://github.com/Accord-Project/aec3po/issues/43"/>
    <rdfs:isDefinedBy>
      <owl:Ontology rdf:about="statement">
        <cc:license rdf:resource="https://creativecommons.org/licenses/by/4.0/"/>
        <dct:contributor rdf:resource="http://maxime-lefrancois.info/me#"/>
        <dct:description xml:lang="en">The AEC3PO Statement module describes a statement, of any kind, found in a document.</dct:description>
        <dct:description rdf:resource="file:///home/runner/work/aec3po/aec3po/src/diagrams/statement.png"/>
        <dct:title xml:lang="en">AEC3PO: statement</dct:title>
        <vann:preferredNamespacePrefix>aec3po</vann:preferredNamespacePrefix>
        <vann:preferredNamespaceUri>https://w3id.org/lbd/aec3po/</vann:preferredNamespaceUri>
        <owl:imports rdf:resource="document"/>
        <dct:created rdf:datatype="http://www.w3.org/2001/XMLSchema#date">2023-08-31</dct:created>
        <dct:modified rdf:datatype="http://www.w3.org/2001/XMLSchema#date">2025-04-22</dct:modified>
      </owl:Ontology>
    </rdfs:isDefinedBy>
  </owl:ObjectProperty>
  <owl:Class rdf:about="NumericalCheckStatement">
    <rdfs:label xml:lang="en">Numerical Check Statement</rdfs:label>
    <rdfs:comment>A type of check that involves checking one numerical property against another, i.e. x &lt; y or similar.</rdfs:comment>
    <rdfs:subClassOf rdf:resource="CheckStatement"/>
    <rdfs:seeAlso rdf:resource="https://github.com/Accord-Project/aec3po/issues/57"/>
    <rdfs:isDefinedBy rdf:resource="statement"/>
  </owl:Class>
  <owl:ObjectProperty rdf:about="hasDefinition">
    <rdfs:label xml:lang="en">has definition</rdfs:label>
    <rdfs:comment xml:lang="en">Links a definition statement to the definition of the term</rdfs:comment>
    <rdfs:domain rdf:resource="DefinitionStatement"/>
    <rdfs:range rdf:resource="DocumentSubdivision"/>
    <rdfs:isDefinedBy rdf:resource="statement"/>
  </owl:ObjectProperty>
  <owl:ObjectProperty rdf:about="definitionOf">
    <rdfs:label xml:lang="en">definition of</rdfs:label>
    <rdfs:comment xml:lang="en">Links a definition statement to the term that is defined</rdfs:comment>
    <rdfs:domain rdf:resource="DefinitionStatement"/>
    <rdfs:range rdf:resource="DocumentSubdivision"/>
    <rdfs:isDefinedBy rdf:resource="statement"/>
  </owl:ObjectProperty>
  <owl:Class rdf:about="CategoryCheckStatement">
    <rdfs:label xml:lang="en">Category Check Statement</rdfs:label>
    <rdfs:comment xml:lang="en">Category check statement refers to a type of statement or requirement that focuses on verifying compliance with specific categories of regulations, standards, or guidelines within the construction industry. Category check statements are used to assess whether a construction project aligns with predefined categories of criteria, such as safety, environmental impact, energy efficiency, accessibility, and more.</rdfs:comment>
    <rdfs:seeAlso rdf:resource="https://github.com/Accord-Project/aec3po/issues/56"/>
    <rdfs:subClassOf rdf:resource="CheckStatement"/>
    <rdfs:isDefinedBy rdf:resource="statement"/>
  </owl:Class>
  <owl:ObjectProperty rdf:about="hasEvaluator">
    <rdfs:label xml:lang="en">has evaluator</rdfs:label>
    <rdfs:comment xml:lang="en">Links a human evaluated statement to the subdivision that expresses who shall verify this check</rdfs:comment>
    <rdfs:domain rdf:resource="HumanEvaluatedCheckStatement"/>
    <rdfs:range rdf:resource="Statement"/>
    <rdfs:isDefinedBy rdf:resource="statement"/>
  </owl:ObjectProperty>
  <owl:Class rdf:about="OrCheckStatement">
    <rdfs:label xml:lang="en">Or Check Statement</rdfs:label>
    <rdfs:comment xml:lang="en">Check verified if and only if at least one of its sub-checks is verified.</rdfs:comment>
    <rdfs:subClassOf>
      <owl:Restriction rdf:nodeID="n8c2369ae7da6414f9d10098dc93d1560b2">
        <owl:minCardinality rdf:datatype="http://www.w3.org/2001/XMLSchema#integer">1</owl:minCardinality>
        <owl:onProperty rdf:resource="hasSubdivision"/>
      </owl:Restriction>
    </rdfs:subClassOf>
    <rdfs:subClassOf rdf:resource="ChecklistStatement"/>
    <rdfs:isDefinedBy rdf:resource="statement"/>
  </owl:Class>
  <owl:Class rdf:about="AndCheckStatement">
    <rdfs:label xml:lang="en">And Check Statement</rdfs:label>
    <rdfs:comment xml:lang="en">Check verified if and only if all of its sub-checks are verified.</rdfs:comment>
    <rdfs:subClassOf>
      <owl:Restriction rdf:nodeID="n8c2369ae7da6414f9d10098dc93d1560b1">
        <owl:minCardinality rdf:datatype="http://www.w3.org/2001/XMLSchema#integer">1</owl:minCardinality>
        <owl:onProperty rdf:resource="hasSubdivision"/>
      </owl:Restriction>
    </rdfs:subClassOf>
    <rdfs:subClassOf rdf:resource="ChecklistStatement"/>
    <rdfs:isDefinedBy rdf:resource="statement"/>
  </owl:Class>
  <owl:Class rdf:about="NotCheckStatement">
    <rdfs:label xml:lang="en">Not Check Statement</rdfs:label>
    <rdfs:comment xml:lang="en">Check verified if and only if the sub-check is not verified.</rdfs:comment>
    <rdfs:subClassOf>
      <owl:Restriction rdf:nodeID="n8c2369ae7da6414f9d10098dc93d1560b3">
        <owl:cardinality rdf:datatype="http://www.w3.org/2001/XMLSchema#integer">1</owl:cardinality>
        <owl:onProperty rdf:resource="hasSubdivision"/>
      </owl:Restriction>
    </rdfs:subClassOf>
    <rdfs:isDefinedBy rdf:resource="statement"/>
  </owl:Class>
  <owl:Class rdf:about="BooleanCheckStatement">
    <rdfs:label xml:lang="en">Boolean Check Statement</rdfs:label>
    <rdfs:comment xml:lang="en">A type of check that checks the existence of an element (property) related to a feature of interest.</rdfs:comment>
    <rdfs:seeAlso rdf:resource="https://github.com/Accord-Project/aec3po/issues/58"/>
    <rdfs:subClassOf rdf:resource="CheckStatement"/>
    <rdfs:isDefinedBy rdf:resource="statement"/>
  </owl:Class>
  <owl:Class rdf:about="CertificateCheckStatement">
    <rdfs:label xml:lang="en">Certificate Check Statement</rdfs:label>
    <rdfs:comment xml:lang="en">Certificate check statement refers to a type of statement or requirement that focuses on verifying and validating the authenticity and compliance of certificates related to construction projects</rdfs:comment>
    <rdfs:subClassOf rdf:resource="CheckStatement"/>
    <rdfs:seeAlso rdf:resource="https://github.com/Accord-Project/aec3po/issues/59"/>
    <rdfs:isDefinedBy rdf:resource="statement"/>
  </owl:Class>
  <owl:ObjectProperty rdf:about="hasEvidence">
    <rdfs:label xml:lang="en">hasEvidence</rdfs:label>
    <rdfs:comment xml:lang="en">Links a statement to a piece of evidence for that statement (assertion, statement, or claim).</rdfs:comment>
    <skos:note xml:lang="en">Unstable. Need evidence of how this property is intended to be used</skos:note>
    <rdfs:domain rdf:resource="Statement"/>
    <rdfs:isDefinedBy rdf:resource="statement"/>
  </owl:ObjectProperty>
  <owl:Class rdf:about="ChecklistStatement">
    <rdfs:label xml:lang="en">Checklist Statement</rdfs:label>
    <rdfs:comment xml:lang="en">Checklist statement is a type of check statement that represents a list of checks that need to be verified.</rdfs:comment>
    <rdfs:subClassOf rdf:resource="CheckStatement"/>
    <rdfs:isDefinedBy rdf:resource="statement"/>
  </owl:Class>
  <owl:Class rdf:about="Statement">
    <rdfs:label xml:lang="en">Statement</rdfs:label>
    <rdfs:comment xml:lang="en">Something stated in a building compliance-related document</rdfs:comment>
    <skos:example xml:lang="en">Any solar protection solutions in the building shall be taken into account in the calculation of solar energy gains for the building.</skos:example>
    <rdfs:subClassOf rdf:resource="DocumentSubdivision"/>
    <rdfs:isDefinedBy rdf:resource="statement"/>
  </owl:Class>
  <owl:Class rdf:about="DefinitionStatement">
    <rdfs:label xml:lang="en">Definition Statement</rdfs:label>
    <rdfs:comment xml:lang="en">A type of statement that provides a formal and precise definition for a specific concept or term, scoped to this document.</rdfs:comment>
    <rdfs:subClassOf rdf:resource="Statement"/>
    <rdfs:isDefinedBy rdf:resource="statement"/>
  </owl:Class>
  <owl:Class rdf:about="HumanEvaluatedCheckStatement">
    <rdfs:label xml:lang="en">Human Evaluated Check Statement</rdfs:label>
    <rdfs:comment xml:lang="en">A type of check statement that is evaluated by a human.</rdfs:comment>
    <skos:note xml:lang="en">Those are primarily for issues of perception</skos:note>
    <skos:example xml:lang="en">"is aesthetically appropriate"</skos:example>
    <rdfs:seeAlso rdf:resource="https://github.com/Accord-Project/aec3po/issues/60"/>
    <rdfs:subClassOf rdf:resource="CheckStatement"/>
    <rdfs:isDefinedBy rdf:resource="statement"/>
  </owl:Class>
  <owl:Class rdf:about="CheckStatement">
    <rdfs:label xml:lang="en">Check Statement</rdfs:label>
    <rdfs:comment xml:lang="en">refers to a type of statement that is used to specify conditions, criteria, or rules for evaluating the compliance, correctness, or validity of certain properties, features, or aspects of a system, process, or domain.</rdfs:comment>
    <rdfs:subClassOf rdf:resource="Statement"/>
    <rdfs:isDefinedBy rdf:resource="statement"/>
  </owl:Class>
</rdf:RDF>
