<?xml version="1.0" encoding="utf-8"?>
<rdf:RDF xml:base="https://w3id.org/lbd/aec3po/"
  xmlns:rdfs="http://www.w3.org/2000/01/rdf-schema#"
  xmlns:owl="http://www.w3.org/2002/07/owl#"
  xmlns:rdf="http://www.w3.org/1999/02/22-rdf-syntax-ns#"
  xmlns:cc="http://creativecommons.org/ns#"
  xmlns:vann="http://purl.org/vocab/vann/"
  xmlns:dct="http://purl.org/dc/terms/"
>
  <owl:DatatypeProperty rdf:about="caption">
    <rdfs:label xml:lang="en">caption</rdfs:label>
    <rdfs:comment xml:lang="en">The caption of a table, image, etc. </rdfs:comment>
    <rdfs:domain>
      <owl:Class rdf:nodeID="n90b1d94a3d3444edb6c83f593f9aaa9bb12">
        <owl:unionOf rdf:parseType="Collection">
          <rdf:Description rdf:about="Table"/>
          <rdf:Description rdf:about="Image"/>
        </owl:unionOf>
      </owl:Class>
    </rdfs:domain>
    <rdfs:isDefinedBy>
      <owl:Ontology rdf:about="table">
        <cc:license rdf:resource="https://creativecommons.org/licenses/by/4.0/"/>
        <dct:contributor rdf:resource="edlira"/>
        <dct:description xml:lang="en">The AEC3PO Table module describes tables as representations of data in rows and columns. Tables are described by captions.</dct:description>
        <dct:modified rdf:datatype="http://www.w3.org/2001/XMLSchema#date">2023-05-26</dct:modified>
        <dct:modified rdf:datatype="http://www.w3.org/2001/XMLSchema#date">2023-11-01</dct:modified>
        <dct:title xml:lang="en">AEC3PO: Table</dct:title>
        <owl:imports rdf:resource="document"/>
        <vann:preferredNamespacePrefix>aec3po</vann:preferredNamespacePrefix>
        <vann:preferredNamespaceUri>https://w3id.org/lbd/aec3po/</vann:preferredNamespaceUri>
        <dct:created rdf:datatype="http://www.w3.org/2001/XMLSchema#date">2023-05-26</dct:created>
      </owl:Ontology>
    </rdfs:isDefinedBy>
  </owl:DatatypeProperty>
  <owl:ObjectProperty rdf:about="isContainedIn">
    <rdfs:label xml:lang="en">is contained by</rdfs:label>
    <rdfs:comment xml:lang="en">A table contains row, columns and other elements.</rdfs:comment>
    <rdfs:range>
      <owl:Class rdf:nodeID="n90b1d94a3d3444edb6c83f593f9aaa9bb6">
        <owl:unionOf rdf:parseType="Collection">
          <rdf:Description rdf:about="Table"/>
          <rdf:Description rdf:about="Image"/>
          <rdf:Description rdf:about="Row"/>
          <rdf:Description rdf:about="Column"/>
          <rdf:Description rdf:about="Cell"/>
        </owl:unionOf>
      </owl:Class>
    </rdfs:range>
    <rdfs:isDefinedBy rdf:resource="table"/>
  </owl:ObjectProperty>
  <owl:ObjectProperty rdf:about="contains">
    <rdfs:label xml:lang="en">Contains</rdfs:label>
    <rdfs:comment xml:lang="en">A container contains a table and its caption. A table contains row, columns and other elements.</rdfs:comment>
    <rdfs:domain>
      <owl:Class rdf:nodeID="n90b1d94a3d3444edb6c83f593f9aaa9bb1">
        <owl:unionOf rdf:parseType="Collection">
          <rdf:Description rdf:about="Table"/>
          <rdf:Description rdf:about="Image"/>
          <rdf:Description rdf:about="Row"/>
          <rdf:Description rdf:about="Column"/>
        </owl:unionOf>
      </owl:Class>
    </rdfs:domain>
    <rdfs:isDefinedBy rdf:resource="table"/>
  </owl:ObjectProperty>
  <owl:Class rdf:about="Container">
    <rdfs:subClassOf rdf:resource="DocumentSubdivision"/>
    <rdfs:label xml:lang="en">Container</rdfs:label>
    <rdfs:comment>A rectangular shape within a document containing and object such as table, image, equation and their respective caption. (Inspired by DoCo ontology)</rdfs:comment>
    <rdfs:isDefinedBy rdf:resource="table"/>
  </owl:Class>
  <owl:Class rdf:about="Cell">
    <rdfs:label xml:lang="en">Cell</rdfs:label>
    <rdfs:subClassOf rdf:resource="Table"/>
    <rdfs:comment>A cell in a table. Cells are contained in rows and columns</rdfs:comment>
    <rdfs:isDefinedBy rdf:resource="table"/>
  </owl:Class>
  <owl:Class rdf:about="Column">
    <rdfs:label xml:lang="en">Column</rdfs:label>
    <rdfs:subClassOf rdf:resource="Table"/>
    <rdfs:comment>A column in a table.</rdfs:comment>
    <rdfs:isDefinedBy rdf:resource="table"/>
  </owl:Class>
  <owl:Class rdf:about="Row">
    <rdfs:label xml:lang="en">Row</rdfs:label>
    <rdfs:subClassOf rdf:resource="Table"/>
    <rdfs:comment>A row in a table.</rdfs:comment>
    <rdfs:isDefinedBy rdf:resource="table"/>
  </owl:Class>
  <owl:Class rdf:about="Table">
    <rdfs:label xml:lang="en">Table</rdfs:label>
    <rdfs:comment>A table is a form of representing information or data in rows and columns. Tables are described by captions.</rdfs:comment>
    <rdfs:isDefinedBy rdf:resource="table"/>
  </owl:Class>
</rdf:RDF>
