@base <https://w3id.org/lbd/aec3po/> .
@prefix aec3po: <https://w3id.org/lbd/aec3po/> .
@prefix cc: <http://creativecommons.org/ns#> .
@prefix dct: <http://purl.org/dc/terms/> .
@prefix ns1: <https://w3id.org/profile/ontdoc/> .
@prefix owl: <http://www.w3.org/2002/07/owl#> .
@prefix prov: <http://www.w3.org/ns/prov#> .
@prefix rdf: <http://www.w3.org/1999/02/22-rdf-syntax-ns#> .
@prefix rdfs: <http://www.w3.org/2000/01/rdf-schema#> .
@prefix vann: <http://purl.org/vocab/vann/> .
@prefix xsd: <http://www.w3.org/2001/XMLSchema#> .

_:nd64d291a23fd441387594d3a290fbdc6b1 a rdfs:Class,
        owl:Class ;
    owl:unionOf ( <Table> <Image> <Row> <Column> ) ;
    ns1:inDomainOf <contains> .

_:nd64d291a23fd441387594d3a290fbdc6b12 a rdfs:Class,
        owl:Class ;
    owl:unionOf ( <Table> <Image> ) ;
    ns1:inDomainOf <caption> .

_:nd64d291a23fd441387594d3a290fbdc6b6 a rdfs:Class,
        owl:Class ;
    owl:unionOf ( <Table> <Image> <Row> <Column> <Cell> ) ;
    ns1:inRangeOf <isContainedIn> .

<Cell> a rdfs:Class,
        owl:Class ;
    rdfs:label "Cell"@en ;
    dct:description "A cell in a table. Cells are contained in rows and columns" ;
    dct:title "Cell"@en ;
    rdfs:comment "A cell in a table. Cells are contained in rows and columns" ;
    rdfs:isDefinedBy <table> ;
    rdfs:subClassOf <Table> .

<Column> a rdfs:Class,
        owl:Class ;
    rdfs:label "Column"@en ;
    dct:description "A column in a table." ;
    dct:title "Column"@en ;
    rdfs:comment "A column in a table." ;
    rdfs:isDefinedBy <table> ;
    rdfs:subClassOf <Table> .

<Container> a rdfs:Class,
        owl:Class ;
    rdfs:label "Container"@en ;
    dct:description "A rectangular shape within a document containing and object such as table, image, equation and their respective caption. (Inspired by DoCo ontology)" ;
    dct:title "Container"@en ;
    rdfs:comment "A rectangular shape within a document containing and object such as table, image, equation and their respective caption. (Inspired by DoCo ontology)" ;
    rdfs:isDefinedBy <table> ;
    rdfs:subClassOf <DocumentSubdivision> .

<Row> a rdfs:Class,
        owl:Class ;
    rdfs:label "Row"@en ;
    dct:description "A row in a table." ;
    dct:title "Row"@en ;
    rdfs:comment "A row in a table." ;
    rdfs:isDefinedBy <table> ;
    rdfs:subClassOf <Table> .

<Table> a rdfs:Class,
        owl:Class ;
    rdfs:label "Table"@en ;
    dct:description "A table is a form of representing information or data in rows and columns. Tables are described by captions." ;
    dct:title "Table"@en ;
    rdfs:comment "A table is a form of representing information or data in rows and columns. Tables are described by captions." ;
    rdfs:isDefinedBy <table> ;
    ns1:superClassOf <Cell>,
        <Column>,
        <Row> .

owl:DatatypeProperty ns1:hasMember <caption> .

owl:Ontology ns1:hasMember <table> .

<DocumentSubdivision> ns1:superClassOf <Container> .

<edlira> a prov:Agent .

owl:ObjectProperty ns1:hasMember <contains>,
        <isContainedIn> .

<caption> a owl:DatatypeProperty ;
    rdfs:label "caption"@en ;
    dct:description "The caption of a table, image, etc. "@en ;
    dct:title "caption"@en ;
    rdfs:comment "The caption of a table, image, etc. "@en ;
    rdfs:domain _:nd64d291a23fd441387594d3a290fbdc6b12 ;
    rdfs:isDefinedBy <table> .

<contains> a owl:ObjectProperty ;
    rdfs:label "Contains"@en ;
    dct:description "A container contains a table and its caption. A table contains row, columns and other elements."@en ;
    dct:title "Contains"@en ;
    rdfs:comment "A container contains a table and its caption. A table contains row, columns and other elements."@en ;
    rdfs:domain _:nd64d291a23fd441387594d3a290fbdc6b1 ;
    rdfs:isDefinedBy <table> .

<isContainedIn> a owl:ObjectProperty ;
    rdfs:label "is contained by"@en ;
    dct:description "A table contains row, columns and other elements."@en ;
    dct:title "is contained by"@en ;
    rdfs:comment "A table contains row, columns and other elements."@en ;
    rdfs:isDefinedBy <table> ;
    rdfs:range _:nd64d291a23fd441387594d3a290fbdc6b6 .

rdfs:Class ns1:hasMember _:nd64d291a23fd441387594d3a290fbdc6b1,
        _:nd64d291a23fd441387594d3a290fbdc6b12,
        _:nd64d291a23fd441387594d3a290fbdc6b6,
        <Cell>,
        <Column>,
        <Container>,
        <Row>,
        <Table> .

owl:Class ns1:hasMember _:nd64d291a23fd441387594d3a290fbdc6b1,
        _:nd64d291a23fd441387594d3a290fbdc6b12,
        _:nd64d291a23fd441387594d3a290fbdc6b6,
        <Cell>,
        <Column>,
        <Container>,
        <Row>,
        <Table> .

<table> a owl:Ontology ;
    cc:license <https://creativecommons.org/licenses/by/4.0/> ;
    dct:contributor <edlira> ;
    dct:created "2023-05-26"^^xsd:date ;
    dct:description "The AEC3PO Table module describes tables as representations of data in rows and columns. Tables are described by captions."@en ;
    dct:modified "2023-05-26"^^xsd:date,
        "2023-11-01"^^xsd:date ;
    dct:title "AEC3PO: Table"@en ;
    vann:preferredNamespacePrefix "aec3po" ;
    vann:preferredNamespaceUri "https://w3id.org/lbd/aec3po/" ;
    owl:imports <document> .

