@prefix aec3po: <https://w3id.org/lbd/aec3po/> .
@prefix cc: <http://creativecommons.org/ns#> .
@prefix dct: <http://purl.org/dc/terms/> .
@prefix eli: <http://data.europa.eu/eli/ontology#> .
@prefix owl: <http://www.w3.org/2002/07/owl#> .
@prefix rdfs: <http://www.w3.org/2000/01/rdf-schema#> .
@prefix skos: <http://www.w3.org/2004/02/skos/core#> .
@prefix vann: <http://purl.org/vocab/vann/> .
@prefix xsd: <http://www.w3.org/2001/XMLSchema#> .

aec3po:administrative_areas a owl:Ontology ;
    cc:license <https://creativecommons.org/licenses/by/4.0/> ;
    dct:contributor <http://maxime-lefrancois.info/me#> ;
    dct:description "Definition of an administrative areas concept scheme for AEC3PO."@en ;
    dct:modified "2023-05-25"^^xsd:date ;
    dct:title "AEC3PO: Administrative Areas"@en ;
    vann:preferredNamespacePrefix "aec3po" ;
    vann:preferredNamespaceUri "https://w3id.org/lbd/aec3po/" .

aec3po:AdministrativeArea a owl:Class ;
    rdfs:label "Administrative Area"@en ;
    rdfs:comment "Formally defined as the set of skos:Concept either in concept scheme aec3po:AdministrativeAreaNomenclature or in concept scheme http://publications.europa.eu/mdr/authority/atu (Administrative Territorial Unit nomenclature published of the EU Publications Office)."@en ;
    rdfs:isDefinedBy aec3po:administrative_areas ;
    rdfs:seeAlso <https://op.europa.eu/en/web/eu-vocabularies/concept-scheme/-/resource?uri=http://publications.europa.eu/resource/authority/atu> ;
    rdfs:subClassOf skos:Concept ;
    owl:equivalentClass eli:AdministrativeArea ;
    owl:equivalentClass [ owl:intersectionOf ( skos:Concept [ a owl:Restriction ;
                        owl:hasValue aec3po:AdministrativeAreaNomenclature ;
                        owl:onProperty skos:inScheme ] ) ] .

aec3po:AdministrativeAreaNomenclature a skos:ConceptScheme ;
    rdfs:label "Administrative Area nomenclature"@en ;
    rdfs:isDefinedBy aec3po:administrative_areas ;
    skos:definition """A set of values for the administrative areas.
  aec3po includes a set of values for this nomenclature.
  These values are :
  - England
  - Estonia
  - Finland
  - France
  - Germany
  - Italy
  - Spain"""@en ;
    skos:hasTopConcept aec3po:England,
    aec3po:Estonia,
    aec3po:Finland,
    aec3po:France,
    aec3po:Germany,
    aec3po:Italy,
    aec3po:Spain .

aec3po:forAdministrativeArea a owl:ObjectProperty ;
    rdfs:label "for administrative area"@en ;
    rdfs:comment """The administrative area for which something applies.
  A set of values is defined by aec3po in the corresponding concept scheme."""@en ;
    rdfs:isDefinedBy aec3po:administrative_areas ;
    rdfs:range aec3po:AdministrativeArea .

aec3po:England a owl:NamedIndividual, skos:Concept , aec3po:AdministrativeArea ;
    rdfs:isDefinedBy aec3po:administrative_areas ;
    skos:definition "England"@en ;
    skos:inScheme aec3po:AdministrativeAreaNomenclature ;
    skos:prefLabel "England"@en ;
    skos:topConceptOf aec3po:AdministrativeAreaNomenclature .

aec3po:Estonia a owl:NamedIndividual, skos:Concept , aec3po:AdministrativeArea ;
    rdfs:isDefinedBy aec3po:administrative_areas ;
    skos:definition "Estonia"@en ;
    skos:inScheme aec3po:AdministrativeAreaNomenclature ;
    skos:prefLabel "Estonia"@en ;
    skos:topConceptOf aec3po:AdministrativeAreaNomenclature .

aec3po:Finland a owl:NamedIndividual, skos:Concept , aec3po:AdministrativeArea ;
    rdfs:isDefinedBy aec3po:administrative_areas ;
    skos:definition "Finland"@en ;
    skos:inScheme aec3po:AdministrativeAreaNomenclature ;
    skos:prefLabel "Finland"@en ;
    skos:topConceptOf aec3po:AdministrativeAreaNomenclature .

aec3po:France a owl:NamedIndividual, skos:Concept , aec3po:AdministrativeArea ;
    rdfs:isDefinedBy aec3po:administrative_areas ;
    skos:definition "France"@en ;
    skos:inScheme aec3po:AdministrativeAreaNomenclature ;
    skos:prefLabel "France"@en ;
    skos:topConceptOf aec3po:AdministrativeAreaNomenclature .

aec3po:Germany a owl:NamedIndividual, skos:Concept , aec3po:AdministrativeArea ;
    rdfs:isDefinedBy aec3po:administrative_areas ;
    skos:definition "Germany"@en ;
    skos:inScheme aec3po:AdministrativeAreaNomenclature ;
    skos:prefLabel "Germany"@en ;
    skos:topConceptOf aec3po:AdministrativeAreaNomenclature .

aec3po:Italy a owl:NamedIndividual, skos:Concept , aec3po:AdministrativeArea ;
    rdfs:isDefinedBy aec3po:administrative_areas ;
    skos:definition "Italy"@en ;
    skos:inScheme aec3po:AdministrativeAreaNomenclature ;
    skos:prefLabel "Italy"@en ;
    skos:topConceptOf aec3po:AdministrativeAreaNomenclature .

aec3po:Spain a owl:NamedIndividual, skos:Concept , aec3po:AdministrativeArea ;
    rdfs:isDefinedBy aec3po:administrative_areas ;
    skos:definition "Spain"@en ;
    skos:inScheme aec3po:AdministrativeAreaNomenclature ;
    skos:prefLabel "Spain"@en ;
    skos:topConceptOf aec3po:AdministrativeAreaNomenclature .
