<?xml version="1.0" encoding="utf-8"?>
<rdf:RDF xml:base="https://w3id.org/lbd/aec3po/"
  xmlns:rdf="http://www.w3.org/1999/02/22-rdf-syntax-ns#"
  xmlns:rdfs="http://www.w3.org/2000/01/rdf-schema#"
  xmlns:owl="http://www.w3.org/2002/07/owl#"
  xmlns:cc="http://creativecommons.org/ns#"
  xmlns:skos="http://www.w3.org/2004/02/skos/core#"
  xmlns:vann="http://purl.org/vocab/vann/"
  xmlns:ns1="https://w3id.org/profile/ontdoc/"
  xmlns:prov="http://www.w3.org/ns/prov#"
  xmlns:dct="http://purl.org/dc/terms/"
  xmlns:aec3po="https://w3id.org/lbd/aec3po/"
>
  <owl:NamedIndividual rdf:about="Germany">
    <rdf:type>
      <rdf:Description rdf:about="http://www.w3.org/2004/02/skos/core#Concept">
        <ns1:superClassOf rdf:resource="AdministrativeArea"/>
        <ns1:hasMember rdf:resource="England"/>
        <ns1:hasMember rdf:resource="Estonia"/>
        <ns1:hasMember rdf:resource="Finland"/>
        <ns1:hasMember rdf:resource="France"/>
        <ns1:hasMember rdf:resource="Germany"/>
        <ns1:hasMember rdf:resource="Italy"/>
        <ns1:hasMember rdf:resource="Spain"/>
      </rdf:Description>
    </rdf:type>
    <rdf:type rdf:resource="AdministrativeArea"/>
    <rdfs:isDefinedBy>
      <owl:Ontology rdf:about="administrative_areas">
        <cc:license rdf:resource="https://creativecommons.org/licenses/by/4.0/"/>
        <dct:contributor rdf:resource="http://maxime-lefrancois.info/me#"/>
        <dct:description xml:lang="en">Definition of an administrative areas concept scheme for AEC3PO.</dct:description>
        <dct:modified rdf:datatype="http://www.w3.org/2001/XMLSchema#date">2023-05-25</dct:modified>
        <dct:modified rdf:datatype="http://www.w3.org/2001/XMLSchema#date">2023-08-31</dct:modified>
        <dct:title xml:lang="en">AEC3PO: Administrative Areas</dct:title>
        <vann:preferredNamespacePrefix>aec3po</vann:preferredNamespacePrefix>
        <vann:preferredNamespaceUri>https://w3id.org/lbd/aec3po/</vann:preferredNamespaceUri>
        <dct:created rdf:datatype="http://www.w3.org/2001/XMLSchema#date">2023-05-25</dct:created>
      </owl:Ontology>
    </rdfs:isDefinedBy>
    <skos:definition xml:lang="en">Germany</skos:definition>
    <skos:inScheme>
      <skos:ConceptScheme rdf:about="AdministrativeAreaNomenclature">
        <rdfs:label xml:lang="en">Administrative Area nomenclature</rdfs:label>
        <rdfs:isDefinedBy rdf:resource="administrative_areas"/>
        <skos:definition xml:lang="en">A set of values for the administrative areas.
  aec3po includes a set of values for this nomenclature.
  These values are :
  - England
  - Estonia
  - Finland
  - France
  - Germany
  - Italy
  - Spain</skos:definition>
        <skos:hasTopConcept rdf:resource="England"/>
        <skos:hasTopConcept rdf:resource="Estonia"/>
        <skos:hasTopConcept rdf:resource="Finland"/>
        <skos:hasTopConcept rdf:resource="France"/>
        <skos:hasTopConcept rdf:resource="Germany"/>
        <skos:hasTopConcept rdf:resource="Italy"/>
        <skos:hasTopConcept rdf:resource="Spain"/>
        <dct:title xml:lang="en">Administrative Area nomenclature</dct:title>
        <dct:description xml:lang="en">A set of values for the administrative areas.
  aec3po includes a set of values for this nomenclature.
  These values are :
  - England
  - Estonia
  - Finland
  - France
  - Germany
  - Italy
  - Spain</dct:description>
      </skos:ConceptScheme>
    </skos:inScheme>
    <skos:prefLabel xml:lang="en">Germany</skos:prefLabel>
    <skos:topConceptOf rdf:resource="AdministrativeAreaNomenclature"/>
    <dct:title xml:lang="en">Germany</dct:title>
    <dct:description xml:lang="en">Germany</dct:description>
  </owl:NamedIndividual>
  <owl:NamedIndividual rdf:about="Finland">
    <rdf:type rdf:resource="http://www.w3.org/2004/02/skos/core#Concept"/>
    <rdf:type rdf:resource="AdministrativeArea"/>
    <rdfs:isDefinedBy rdf:resource="administrative_areas"/>
    <skos:definition xml:lang="en">Finland</skos:definition>
    <skos:inScheme rdf:resource="AdministrativeAreaNomenclature"/>
    <skos:prefLabel xml:lang="en">Finland</skos:prefLabel>
    <skos:topConceptOf rdf:resource="AdministrativeAreaNomenclature"/>
    <dct:title xml:lang="en">Finland</dct:title>
    <dct:description xml:lang="en">Finland</dct:description>
  </owl:NamedIndividual>
  <owl:NamedIndividual rdf:about="England">
    <rdf:type rdf:resource="http://www.w3.org/2004/02/skos/core#Concept"/>
    <rdf:type rdf:resource="AdministrativeArea"/>
    <rdfs:isDefinedBy rdf:resource="administrative_areas"/>
    <skos:definition xml:lang="en">England</skos:definition>
    <skos:inScheme rdf:resource="AdministrativeAreaNomenclature"/>
    <skos:prefLabel xml:lang="en">England</skos:prefLabel>
    <skos:topConceptOf rdf:resource="AdministrativeAreaNomenclature"/>
    <dct:title xml:lang="en">England</dct:title>
    <dct:description xml:lang="en">England</dct:description>
  </owl:NamedIndividual>
  <owl:ObjectProperty rdf:about="forAdministrativeArea">
    <rdfs:label xml:lang="en">for administrative area</rdfs:label>
    <rdfs:comment xml:lang="en">The administrative area for which something applies.
  A set of values is defined by aec3po in the corresponding concept scheme.</rdfs:comment>
    <rdfs:isDefinedBy rdf:resource="administrative_areas"/>
    <rdfs:range rdf:resource="AdministrativeArea"/>
    <dct:title xml:lang="en">for administrative area</dct:title>
    <dct:description xml:lang="en">The administrative area for which something applies.
  A set of values is defined by aec3po in the corresponding concept scheme.</dct:description>
  </owl:ObjectProperty>
  <owl:Class rdf:about="AdministrativeArea">
    <rdf:type>
      <rdf:Description rdf:about="http://www.w3.org/2000/01/rdf-schema#Class">
        <ns1:hasMember rdf:resource="AdministrativeArea"/>
      </rdf:Description>
    </rdf:type>
    <rdfs:label xml:lang="en">Administrative Area</rdfs:label>
    <rdfs:comment xml:lang="en">Formally defined as the set of skos:Concept either in concept scheme aec3po:AdministrativeAreaNomenclature or in concept scheme http://publications.europa.eu/mdr/authority/atu (Administrative Territorial Unit nomenclature published of the EU Publications Office).</rdfs:comment>
    <rdfs:isDefinedBy rdf:resource="administrative_areas"/>
    <rdfs:seeAlso rdf:resource="https://op.europa.eu/en/web/eu-vocabularies/concept-scheme/-/resource?uri=http://publications.europa.eu/resource/authority/atu"/>
    <rdfs:subClassOf rdf:resource="http://www.w3.org/2004/02/skos/core#Concept"/>
    <owl:equivalentClass rdf:resource="http://data.europa.eu/eli/ontology#AdministrativeArea"/>
    <owl:equivalentClass>
      <owl:Class rdf:nodeID="n1c2b1af9d3a74c7689cadace53e1fa38b1">
        <owl:intersectionOf rdf:parseType="Collection">
          <rdf:Description rdf:about="http://www.w3.org/2004/02/skos/core#Concept"/>
          <owl:Restriction rdf:nodeID="n1c2b1af9d3a74c7689cadace53e1fa38b2">
            <owl:hasValue rdf:resource="AdministrativeAreaNomenclature"/>
            <owl:onProperty rdf:resource="http://www.w3.org/2004/02/skos/core#inScheme"/>
          </owl:Restriction>
        </owl:intersectionOf>
      </owl:Class>
    </owl:equivalentClass>
    <dct:title xml:lang="en">Administrative Area</dct:title>
    <dct:description xml:lang="en">Formally defined as the set of skos:Concept either in concept scheme aec3po:AdministrativeAreaNomenclature or in concept scheme http://publications.europa.eu/mdr/authority/atu (Administrative Territorial Unit nomenclature published of the EU Publications Office).</dct:description>
    <ns1:inRangeOf rdf:resource="forAdministrativeArea"/>
    <ns1:hasMember rdf:resource="England"/>
    <ns1:hasMember>
      <owl:NamedIndividual rdf:about="Estonia">
        <rdf:type rdf:resource="http://www.w3.org/2004/02/skos/core#Concept"/>
        <rdf:type rdf:resource="AdministrativeArea"/>
        <rdfs:isDefinedBy rdf:resource="administrative_areas"/>
        <skos:definition xml:lang="en">Estonia</skos:definition>
        <skos:inScheme rdf:resource="AdministrativeAreaNomenclature"/>
        <skos:prefLabel xml:lang="en">Estonia</skos:prefLabel>
        <skos:topConceptOf rdf:resource="AdministrativeAreaNomenclature"/>
        <dct:title xml:lang="en">Estonia</dct:title>
        <dct:description xml:lang="en">Estonia</dct:description>
      </owl:NamedIndividual>
    </ns1:hasMember>
    <ns1:hasMember rdf:resource="Finland"/>
    <ns1:hasMember>
      <owl:NamedIndividual rdf:about="France">
        <rdf:type rdf:resource="http://www.w3.org/2004/02/skos/core#Concept"/>
        <rdf:type rdf:resource="AdministrativeArea"/>
        <rdfs:isDefinedBy rdf:resource="administrative_areas"/>
        <skos:definition xml:lang="en">France</skos:definition>
        <skos:inScheme rdf:resource="AdministrativeAreaNomenclature"/>
        <skos:prefLabel xml:lang="en">France</skos:prefLabel>
        <skos:topConceptOf rdf:resource="AdministrativeAreaNomenclature"/>
        <dct:title xml:lang="en">France</dct:title>
        <dct:description xml:lang="en">France</dct:description>
      </owl:NamedIndividual>
    </ns1:hasMember>
    <ns1:hasMember rdf:resource="Germany"/>
    <ns1:hasMember>
      <owl:NamedIndividual rdf:about="Italy">
        <rdf:type rdf:resource="http://www.w3.org/2004/02/skos/core#Concept"/>
        <rdf:type rdf:resource="AdministrativeArea"/>
        <rdfs:isDefinedBy rdf:resource="administrative_areas"/>
        <skos:definition xml:lang="en">Italy</skos:definition>
        <skos:inScheme rdf:resource="AdministrativeAreaNomenclature"/>
        <skos:prefLabel xml:lang="en">Italy</skos:prefLabel>
        <skos:topConceptOf rdf:resource="AdministrativeAreaNomenclature"/>
        <dct:title xml:lang="en">Italy</dct:title>
        <dct:description xml:lang="en">Italy</dct:description>
      </owl:NamedIndividual>
    </ns1:hasMember>
    <ns1:hasMember>
      <owl:NamedIndividual rdf:about="Spain">
        <rdf:type rdf:resource="http://www.w3.org/2004/02/skos/core#Concept"/>
        <rdf:type rdf:resource="AdministrativeArea"/>
        <rdfs:isDefinedBy rdf:resource="administrative_areas"/>
        <skos:definition xml:lang="en">Spain</skos:definition>
        <skos:inScheme rdf:resource="AdministrativeAreaNomenclature"/>
        <skos:prefLabel xml:lang="en">Spain</skos:prefLabel>
        <skos:topConceptOf rdf:resource="AdministrativeAreaNomenclature"/>
        <dct:title xml:lang="en">Spain</dct:title>
        <dct:description xml:lang="en">Spain</dct:description>
      </owl:NamedIndividual>
    </ns1:hasMember>
  </owl:Class>
  <rdf:Description rdf:about="http://www.w3.org/2002/07/owl#ObjectProperty">
    <ns1:hasMember rdf:resource="forAdministrativeArea"/>
  </rdf:Description>
  <rdf:Description rdf:about="http://www.w3.org/2002/07/owl#NamedIndividual">
    <ns1:hasMember rdf:resource="England"/>
    <ns1:hasMember rdf:resource="Estonia"/>
    <ns1:hasMember rdf:resource="Finland"/>
    <ns1:hasMember rdf:resource="France"/>
    <ns1:hasMember rdf:resource="Germany"/>
    <ns1:hasMember rdf:resource="Italy"/>
    <ns1:hasMember rdf:resource="Spain"/>
  </rdf:Description>
  <rdf:Description rdf:about="http://www.w3.org/2002/07/owl#Ontology">
    <ns1:hasMember rdf:resource="administrative_areas"/>
  </rdf:Description>
  <rdf:Description rdf:about="http://www.w3.org/2002/07/owl#Restriction">
    <ns1:hasMember rdf:nodeID="n1c2b1af9d3a74c7689cadace53e1fa38b2"/>
  </rdf:Description>
  <rdf:Description rdf:about="http://www.w3.org/2002/07/owl#Class">
    <ns1:hasMember rdf:resource="AdministrativeArea"/>
    <ns1:hasMember rdf:nodeID="n1c2b1af9d3a74c7689cadace53e1fa38b1"/>
  </rdf:Description>
  <prov:Agent rdf:about="http://maxime-lefrancois.info/me#"/>
  <rdf:Description rdf:about="http://www.w3.org/2004/02/skos/core#ConceptScheme">
    <ns1:hasMember rdf:resource="AdministrativeAreaNomenclature"/>
  </rdf:Description>
</rdf:RDF>
