@prefix aec3po: <https://w3id.org/lbd/aec3po/> .
@prefix cc: <http://creativecommons.org/ns#> .
@prefix dct: <http://purl.org/dc/terms/> .
@prefix eli: <http://data.europa.eu/eli/ontology#> .
@prefix owl: <http://www.w3.org/2002/07/owl#> .
@prefix rdf: <http://www.w3.org/1999/02/22-rdf-syntax-ns#> .
@prefix rdfs: <http://www.w3.org/2000/01/rdf-schema#> .
@prefix skos: <http://www.w3.org/2004/02/skos/core#> .
@prefix vann: <http://purl.org/vocab/vann/> .
@prefix xsd: <http://www.w3.org/2001/XMLSchema#> .

aec3po:building_structure a owl:Ontology ;
    cc:license <https://creativecommons.org/licenses/by/4.0/> ;
    dct:contributor <http://maxime-lefrancois.info/me#>,
        aec3po:etc ;
    dct:description "Definition of a building structure concept scheme for the Construction Compliance Checking and Permitting ontology."@en ;
    dct:modified "2023-04-26"^^xsd:date ;
    dct:title "Construction Compliance Checking and Permitting Ontology: Building Structure"@en ;
    vann:preferredNamespacePrefix "aec3po" ;
    vann:preferredNamespaceUri aec3po: .

aec3po:forBuildingStructure a owl:ObjectProperty ;
    rdfs:label "for building structure"@en ;
    rdfs:comment """The building structure for which a specific check, verifier, or check result applies.
  A set of values is defined by aec3po in the corresponding concept scheme."""@en ;
    rdfs:range aec3po:BuildingStructure ;
    rdfs:subPropertyOf aec3po:forDesign .

aec3po:hasBuildingStructure a owl:FunctionalProperty,
        owl:ObjectProperty ;
    rdfs:label "has building structure"@en ;
    rdfs:comment """The building structure design of a feature of interest or a property of that feature of interest.
  A set of values is defined by aec3po in the corresponding concept scheme."""@en ;
    rdfs:range aec3po:BuildingStructure ;
    rdfs:subPropertyOf aec3po:hasDesign .

aec3po:BuildingStructure-steel a skos:Concept,
        aec3po:BuildingStructure ;
    skos:definition "Building has steel structure."@en ;
    skos:inScheme aec3po:BuildingStructureTable ;
    skos:prefLabel "steel"@en ;
    skos:topConceptOf aec3po:BuildingStructureTable .

aec3po:BuildingStructure-timber a skos:Concept,
        aec3po:BuildingStructure ;
    skos:definition "Building has timber structure."@en ;
    skos:inScheme aec3po:BuildingStructureTable ;
    skos:prefLabel "timber"@en ;
    skos:topConceptOf aec3po:BuildingStructureTable .

aec3po:BuildingStructure a owl:Class ;
    rdfs:label "building structure"@en ;
    rdfs:comment "Formally defined as the set of skos:Concept in concept scheme aec3po:BuildingStructureTable"@en ;
    rdfs:subClassOf skos:Concept,
        aec3po:Design ;
    owl:equivalentClass [ owl:intersectionOf ( skos:Concept [ a owl:Restriction ;
                        owl:hasValue eli:BuildingStructureTable ;
                        owl:onProperty skos:inScheme ] ) ] .

aec3po:BuildingStructureTable a skos:ConceptScheme ;
    rdfs:label "Building structure table"@en ;
    skos:definition """A set of values for the building structure design.
  aec3po includes a set of values for this table.
  These values are :
  - steel : steel building;
  - timber : timber building."""@en ;
    skos:hasTopConcept aec3po:BuildingStructure-steel,
        aec3po:BuildingStructure-timber .

