@base <https://w3id.org/lbd/aec3po/> .
@prefix aec3po: <https://w3id.org/lbd/aec3po/> .
@prefix cc: <http://creativecommons.org/ns#> .
@prefix dct: <http://purl.org/dc/terms/> .
@prefix ns1: <https://w3id.org/profile/ontdoc/> .
@prefix owl: <http://www.w3.org/2002/07/owl#> .
@prefix prov: <http://www.w3.org/ns/prov#> .
@prefix rdf: <http://www.w3.org/1999/02/22-rdf-syntax-ns#> .
@prefix rdfs: <http://www.w3.org/2000/01/rdf-schema#> .
@prefix skos: <http://www.w3.org/2004/02/skos/core#> .
@prefix vann: <http://purl.org/vocab/vann/> .
@prefix xsd: <http://www.w3.org/2001/XMLSchema#> .

<BuildingUsage> a rdfs:Class,
        owl:Class ;
    rdfs:label "building usage"@en ;
    dct:description "Formally defined as the set of skos:Concept in concept scheme aec3po:BuildingUsageNomenclature"@en ;
    dct:title "building usage"@en ;
    rdfs:comment "Formally defined as the set of skos:Concept in concept scheme aec3po:BuildingUsageNomenclature"@en ;
    rdfs:isDefinedBy <building_usage> ;
    rdfs:subClassOf skos:Concept,
        <Design> ;
    owl:equivalentClass _:n4d77ab9eb246491dbeff4306152dbb17b1 ;
    ns1:hasMember <BuildingUsage-commercial>,
        <BuildingUsage-cultural>,
        <BuildingUsage-residential> ;
    ns1:inRangeOf <forBuildingUsage>,
        <hasBuildingUsage> .

<http://maxime-lefrancois.info/me#> a prov:Agent .

rdfs:Class ns1:hasMember <BuildingUsage> .

owl:FunctionalProperty ns1:hasMember <hasBuildingUsage> .

owl:Ontology ns1:hasMember <building_usage> .

owl:Restriction ns1:hasMember _:n4d77ab9eb246491dbeff4306152dbb17b2 .

skos:ConceptScheme ns1:hasMember <BuildingUsageNomenclature> .

<Design> ns1:superClassOf <BuildingUsage> .

<forDesign> ns1:superPropertyOf <forBuildingUsage> .

<hasDesign> ns1:superPropertyOf <hasBuildingUsage> .

owl:Class ns1:hasMember _:n4d77ab9eb246491dbeff4306152dbb17b1,
        <BuildingUsage> .

owl:ObjectProperty ns1:hasMember <forBuildingUsage>,
        <hasBuildingUsage> .

owl:NamedIndividual ns1:hasMember <BuildingUsage-commercial>,
        <BuildingUsage-cultural>,
        <BuildingUsage-residential> .

<BuildingUsage-cultural> a owl:NamedIndividual,
        skos:Concept,
        <BuildingUsage> ;
    dct:description "Building has cultural usage."@en ;
    dct:title "cultural"@en ;
    rdfs:isDefinedBy <building_usage> ;
    skos:definition "Building has cultural usage."@en ;
    skos:inScheme <BuildingUsageNomenclature> ;
    skos:prefLabel "cultural"@en ;
    skos:topConceptOf <BuildingUsageNomenclature> .

<forBuildingUsage> a owl:ObjectProperty ;
    rdfs:label "for building usage"@en ;
    dct:description """The building usage for which a specific check, verifier, or check result applies.
  A set of values is defined by aec3po in the corresponding concept scheme."""@en ;
    dct:title "for building usage"@en ;
    rdfs:comment """The building usage for which a specific check, verifier, or check result applies.
  A set of values is defined by aec3po in the corresponding concept scheme."""@en ;
    rdfs:isDefinedBy <building_usage> ;
    rdfs:range <BuildingUsage> ;
    rdfs:subPropertyOf <forDesign> .

<BuildingUsage-commercial> a owl:NamedIndividual,
        skos:Concept,
        <BuildingUsage> ;
    dct:description "Building has commercial usage."@en ;
    dct:title "commercial"@en ;
    rdfs:isDefinedBy <building_usage> ;
    skos:definition "Building has commercial usage."@en ;
    skos:inScheme <BuildingUsageNomenclature> ;
    skos:prefLabel "commercial"@en ;
    skos:topConceptOf <BuildingUsageNomenclature> .

<BuildingUsage-residential> a owl:NamedIndividual,
        skos:Concept,
        <BuildingUsage> ;
    dct:description "Building has residential usage."@en ;
    dct:title "residential"@en ;
    rdfs:isDefinedBy <building_usage> ;
    skos:definition "Building has residential usage."@en ;
    skos:inScheme <BuildingUsageNomenclature> ;
    skos:prefLabel "residential"@en ;
    skos:topConceptOf <BuildingUsageNomenclature> .

<hasBuildingUsage> a owl:FunctionalProperty,
        owl:ObjectProperty ;
    rdfs:label "has building usage"@en ;
    dct:description """The building usage design of a feature of interest or a property of that feature of interest.
  A set of values is defined by aec3po in the corresponding concept scheme."""@en ;
    dct:title "has building usage"@en ;
    rdfs:comment """The building usage design of a feature of interest or a property of that feature of interest.
  A set of values is defined by aec3po in the corresponding concept scheme."""@en ;
    rdfs:isDefinedBy <building_usage> ;
    rdfs:range <BuildingUsage> ;
    rdfs:subPropertyOf <hasDesign> .

skos:Concept ns1:hasMember <BuildingUsage-commercial>,
        <BuildingUsage-cultural>,
        <BuildingUsage-residential> ;
    ns1:superClassOf <BuildingUsage> .

<BuildingUsageNomenclature> a skos:ConceptScheme ;
    rdfs:label "Building usage nomenclature"@en ;
    dct:description """A set of values for the building usage design.
  AEC3PO includes a set of values for this nomenclature.
  These values are :
  - residential : residential building;
  - commercial : commercial building."""@en ;
    dct:title "Building usage nomenclature"@en ;
    rdfs:isDefinedBy <building_usage> ;
    skos:definition """A set of values for the building usage design.
  AEC3PO includes a set of values for this nomenclature.
  These values are :
  - residential : residential building;
  - commercial : commercial building."""@en ;
    skos:hasTopConcept <BuildingUsage-commercial>,
        <BuildingUsage-residential> .

<building_usage> a owl:Ontology ;
    cc:license <https://creativecommons.org/licenses/by/4.0/> ;
    dct:contributor <http://maxime-lefrancois.info/me#> ;
    dct:created "2023-05-25"^^xsd:date ;
    dct:description "Definition of a building usage concept scheme for AEC3PO."@en ;
    dct:modified "2023-04-26"^^xsd:date,
        "2023-08-31"^^xsd:date ;
    dct:title "AEC3PO: Building Usage"@en ;
    vann:preferredNamespacePrefix "aec3po" ;
    vann:preferredNamespaceUri "https://w3id.org/lbd/aec3po/" .

_:n4d77ab9eb246491dbeff4306152dbb17b3 rdf:first skos:Concept ;
    rdf:rest ( _:n4d77ab9eb246491dbeff4306152dbb17b2 ) .

_:n4d77ab9eb246491dbeff4306152dbb17b1 a owl:Class ;
    owl:intersectionOf _:n4d77ab9eb246491dbeff4306152dbb17b3 .

_:n4d77ab9eb246491dbeff4306152dbb17b2 a owl:Restriction ;
    owl:hasValue <BuildingUsageNomenclature> ;
    owl:onProperty skos:inScheme .

