@base <https://w3id.org/lbd/aec3po/> .
@prefix aec3po: <> .
@prefix owl: <http://www.w3.org/2002/07/owl#> .
@prefix rdf: <http://www.w3.org/1999/02/22-rdf-syntax-ns#> .
@prefix xml: <http://www.w3.org/XML/1998/namespace> .
@prefix xsd: <http://www.w3.org/2001/XMLSchema#> .
@prefix rdfs: <http://www.w3.org/2000/01/rdf-schema#> .
@prefix cc: <http://creativecommons.org/ns#> .
@prefix vann: <http://purl.org/vocab/vann/> .
@prefix voaf: <http://purl.org/vocommons/voaf#> .
@prefix foaf: <http://xmlns.com/foaf/0.1/>.
@prefix schema: <http://schema.org/>.
@prefix dct: <http://purl.org/dc/terms/>.
@prefix skos: <http://www.w3.org/2004/02/skos/core#>.
@prefix dul: <http://www.ontologydesignpatterns.org/ont/dul/DUL.owl#>.
@prefix eli: <http://data.europa.eu/eli/ontology#> .
@prefix rdac: <http://www.rdaregistry.info/Elements/c/> .

aec3po:building_usage a owl:Ontology ;
    dct:title "Construction Compliance Checking and Permitting Ontology: Building Usage"@en ;
    dct:description  "Definition of a building usage concept scheme for the Construction Compliance Checking and Permitting ontology."@en ;
    dct:modified "2023-04-26"^^xsd:date ;
    dct:contributor <http://maxime-lefrancois.info/me#> ; 
    dct:contributor <etc> ;
    cc:license <https://creativecommons.org/licenses/by/4.0/> ;
    vann:preferredNamespacePrefix "aec3po" ;
    vann:preferredNamespaceUri <> .


aec3po:BuildingUsage a owl:Class ;
  rdfs:subClassOf aec3po:Design, skos:Concept ;
  rdfs:label "building usage"@en ;
  rdfs:comment "Formally defined as the set of skos:Concept in concept scheme aec3po:BuildingUsageTable"@en ;
  owl:equivalentClass [
    owl:intersectionOf (
     skos:Concept
     [  a owl:Restriction ;
        owl:onProperty skos:inScheme ;
        owl:hasValue eli:BuildingUsageTable .
     ]
   )
  ] .

aec3po:hasBuildingUsage a owl:ObjectProperty, owl:FunctionalProperty ;
  rdfs:subPropertyOf aec3po:hasDesign ;
  rdfs:range aec3po:BuildingUsage ;
  rdfs:label "has building usage"@en ;
  rdfs:comment """The building usage design of a feature of interest or a property of that feature of interest.
  A set of values is defined by aec3po in the corresponding concept scheme."""@en .

aec3po:forBuildingUsage a owl:ObjectProperty ;
  rdfs:subPropertyOf aec3po:forDesign ;
  rdfs:range aec3po:BuildingUsage ;
  rdfs:label "for building usage"@en ;
  rdfs:comment """The building usage for which a specific check, verifier, or check result applies.
  A set of values is defined by aec3po in the corresponding concept scheme."""@en .

aec3po:BuildingUsageTable a skos:ConceptScheme ;
  skos:hasTopConcept aec3po:BuildingUsage-residential, aec3po:BuildingUsage-commercial ;
  rdfs:label "Building usage table"@en ;
  skos:definition """A set of values for the building usage design.
  aec3po includes a set of values for this table.
  These values are :
  - residential : residential building;
  - commercial : commercial building."""@en .

aec3po:BuildingUsage-residential a aec3po:BuildingUsage, skos:Concept ;
  skos:inScheme aec3po:BuildingUsageTable ;
  skos:topConceptOf aec3po:BuildingUsageTable ;
  skos:definition "Building has residential usage."@en ;
  skos:prefLabel "residential"@en .

aec3po:BuildingUsage-commercial a aec3po:BuildingUsage, skos:Concept ;
  skos:inScheme aec3po:BuildingUsageTable ;
  skos:topConceptOf aec3po:BuildingUsageTable ;
  skos:definition "Building has commercial usage."@en ;
  skos:prefLabel "commercial"@en .

