<?xml version="1.0" encoding="utf-8"?>
<rdf:RDF xml:base="https://w3id.org/lbd/aec3po/"
  xmlns:rdfs="http://www.w3.org/2000/01/rdf-schema#"
  xmlns:owl="http://www.w3.org/2002/07/owl#"
  xmlns:skos="http://www.w3.org/2004/02/skos/core#"
  xmlns:dct="http://purl.org/dc/terms/"
  xmlns:vann="http://purl.org/vocab/vann/"
  xmlns:aec3po="https://w3id.org/lbd/aec3po/"
  xmlns:rdf="http://www.w3.org/1999/02/22-rdf-syntax-ns#"
  xmlns:ns1="https://w3id.org/profile/ontdoc/"
  xmlns:prov="http://www.w3.org/ns/prov#"
  xmlns:cc="http://creativecommons.org/ns#"
>
  <owl:NamedIndividual rdf:about="CheckMethodcomparator-eq">
    <rdf:type>
      <rdf:Description rdf:about="http://www.w3.org/2004/02/skos/core#Concept">
        <ns1:superClassOf rdf:resource="CheckMethodComparator"/>
        <ns1:hasMember rdf:resource="CheckMethodcomparator-eq"/>
        <ns1:hasMember rdf:resource="CheckMethodComparator-neq"/>
        <ns1:hasMember rdf:resource="CheckMethodComparator-lt"/>
        <ns1:hasMember rdf:resource="CheckMethodComparator-le"/>
        <ns1:hasMember rdf:resource="CheckMethodComparator-gt"/>
        <ns1:hasMember rdf:resource="CheckMethodComparator-ge"/>
        <ns1:hasMember rdf:resource="CheckMethodcomparator-logicalAND"/>
        <ns1:hasMember rdf:resource="CheckMethodComparator-logicalOR"/>
      </rdf:Description>
    </rdf:type>
    <rdf:type>
      <rdf:Description rdf:about="CheckMethodcomparator">
        <ns1:hasMember rdf:resource="CheckMethodcomparator-eq"/>
      </rdf:Description>
    </rdf:type>
    <rdfs:isDefinedBy>
      <owl:Ontology rdf:about="check_method_comparators">
        <cc:license rdf:resource="https://creativecommons.org/licenses/by/4.0/"/>
        <dct:contributor rdf:resource="amna"/>
        <dct:description xml:lang="en">Definition of comparators scheme for AEC3PO.</dct:description>
        <dct:modified rdf:datatype="http://www.w3.org/2001/XMLSchema#date">2024-01-24</dct:modified>
        <dct:modified rdf:datatype="http://www.w3.org/2001/XMLSchema#date">2025-04-22</dct:modified>
        <dct:title xml:lang="en">AEC3PO: comparators</dct:title>
        <vann:preferredNamespacePrefix>aec3po</vann:preferredNamespacePrefix>
        <vann:preferredNamespaceUri>https://w3id.org/lbd/aec3po/</vann:preferredNamespaceUri>
        <dct:created rdf:datatype="http://www.w3.org/2001/XMLSchema#date">2024-01-24'
'2023-09-25</dct:created>
      </owl:Ontology>
    </rdfs:isDefinedBy>
    <skos:definition xml:lang="en">equal-to comparator.</skos:definition>
    <skos:inScheme>
      <skos:ConceptScheme rdf:about="CheckMethodComparatorNomenclature">
        <rdfs:label xml:lang="en">check method nomenclature</rdfs:label>
        <rdfs:isDefinedBy rdf:resource="check_method_comparators"/>
        <skos:definition xml:lang="en">A set of comparators for the check method.

  AEC3PO includes a set of comparators for this nomenclature.

  These comparators are :

  - _eq : equal-to comparator;
  - comparator_neq : not equal-to comparator.
  - comparator_lt : less-than comparator.
  - comparator_le : less-equal comparator.
  - comparator_gt : greater-than comparator.
  - comparator_ge : greater-equal comparator.
  </skos:definition>
        <skos:hasTopConcept rdf:resource="CheckMethodComparator-eq"/>
        <skos:hasTopConcept rdf:resource="CheckMethodcomparator-neq"/>
        <skos:hasTopConcept rdf:resource="CheckMethodcomparator-lt"/>
        <skos:hasTopConcept rdf:resource="CheckMethodcomparator-le"/>
        <skos:hasTopConcept rdf:resource="CheckMethodcomparator-gt"/>
        <skos:hasTopConcept rdf:resource="CheckMethodcomparator-ge"/>
        <skos:hasTopConcept rdf:resource="CheckMethodcomparator-logicalAND"/>
        <skos:hasTopConcept rdf:resource="CheckMethodcomparator-logicalOR"/>
        <dct:title xml:lang="en">check method nomenclature</dct:title>
        <dct:description xml:lang="en">A set of comparators for the check method.

  AEC3PO includes a set of comparators for this nomenclature.

  These comparators are :

  - _eq : equal-to comparator;
  - comparator_neq : not equal-to comparator.
  - comparator_lt : less-than comparator.
  - comparator_le : less-equal comparator.
  - comparator_gt : greater-than comparator.
  - comparator_ge : greater-equal comparator.
  </dct:description>
      </skos:ConceptScheme>
    </skos:inScheme>
    <skos:prefLabel xml:lang="en">equal-to</skos:prefLabel>
    <skos:topConceptOf rdf:resource="CheckMethodComparatorNomenclature"/>
    <dct:title xml:lang="en">equal-to</dct:title>
    <dct:description xml:lang="en">equal-to comparator.</dct:description>
  </owl:NamedIndividual>
  <owl:Class rdf:about="CheckMethodComparator">
    <rdf:type>
      <rdf:Description rdf:about="http://www.w3.org/2000/01/rdf-schema#Class">
        <ns1:hasMember rdf:resource="CheckMethodComparator"/>
      </rdf:Description>
    </rdf:type>
    <rdfs:label xml:lang="en">check method comparator</rdfs:label>
    <rdfs:comment xml:lang="en">Formally defined as the set of skos:Concept in concept scheme aec3po:CheckMethodComparatorNomenclature</rdfs:comment>
    <rdfs:isDefinedBy rdf:resource="check_method_comparators"/>
    <rdfs:subClassOf rdf:resource="http://www.w3.org/2004/02/skos/core#Concept"/>
    <rdfs:subClassOf>
      <rdf:Description rdf:about="CheckMethod">
        <ns1:superClassOf rdf:resource="CheckMethodComparator"/>
        <ns1:inRangeOf rdf:resource="hasComparator"/>
      </rdf:Description>
    </rdfs:subClassOf>
    <owl:equivalentClass>
      <owl:Class rdf:nodeID="n054a34c22b134c409ab2a872c59f32eab1">
        <owl:intersectionOf rdf:parseType="Collection">
          <rdf:Description rdf:about="http://www.w3.org/2004/02/skos/core#Concept"/>
          <owl:Restriction rdf:nodeID="n054a34c22b134c409ab2a872c59f32eab2">
            <owl:hasValue rdf:resource="CheckMethodComparatorNomenclature"/>
            <owl:onProperty rdf:resource="http://www.w3.org/2004/02/skos/core#inScheme"/>
          </owl:Restriction>
        </owl:intersectionOf>
      </owl:Class>
    </owl:equivalentClass>
    <dct:title xml:lang="en">check method comparator</dct:title>
    <dct:description xml:lang="en">Formally defined as the set of skos:Concept in concept scheme aec3po:CheckMethodComparatorNomenclature</dct:description>
    <ns1:hasMember>
      <owl:NamedIndividual rdf:about="CheckMethodComparator-neq">
        <rdf:type rdf:resource="http://www.w3.org/2004/02/skos/core#Concept"/>
        <rdf:type rdf:resource="CheckMethodComparator"/>
        <rdfs:isDefinedBy rdf:resource="check_method_comparators"/>
        <skos:definition xml:lang="en">not equal-to comparator.</skos:definition>
        <skos:inScheme rdf:resource="CheckMethodComparatorNomenclature"/>
        <skos:prefLabel xml:lang="en">not equal-to</skos:prefLabel>
        <skos:topConceptOf rdf:resource="CheckMethodComparatorNomenclature"/>
        <dct:title xml:lang="en">not equal-to</dct:title>
        <dct:description xml:lang="en">not equal-to comparator.</dct:description>
      </owl:NamedIndividual>
    </ns1:hasMember>
    <ns1:hasMember>
      <owl:NamedIndividual rdf:about="CheckMethodComparator-lt">
        <rdf:type rdf:resource="http://www.w3.org/2004/02/skos/core#Concept"/>
        <rdf:type rdf:resource="CheckMethodComparator"/>
        <rdfs:isDefinedBy rdf:resource="check_method_comparators"/>
        <skos:definition xml:lang="en">less-than comparator.</skos:definition>
        <skos:inScheme rdf:resource="CheckMethodComparatorNomenclature"/>
        <skos:prefLabel xml:lang="en">less than</skos:prefLabel>
        <skos:topConceptOf rdf:resource="CheckMethodComparatorNomenclature"/>
        <dct:title xml:lang="en">less than</dct:title>
        <dct:description xml:lang="en">less-than comparator.</dct:description>
      </owl:NamedIndividual>
    </ns1:hasMember>
    <ns1:hasMember>
      <owl:NamedIndividual rdf:about="CheckMethodComparator-le">
        <rdf:type rdf:resource="http://www.w3.org/2004/02/skos/core#Concept"/>
        <rdf:type rdf:resource="CheckMethodComparator"/>
        <rdfs:isDefinedBy rdf:resource="check_method_comparators"/>
        <skos:definition xml:lang="en">less-equal comparator.</skos:definition>
        <skos:inScheme rdf:resource="CheckMethodComparatorNomenclature"/>
        <skos:prefLabel xml:lang="en">less equal</skos:prefLabel>
        <skos:topConceptOf rdf:resource="CheckMethodComparatorNomenclature"/>
        <dct:title xml:lang="en">less equal</dct:title>
        <dct:description xml:lang="en">less-equal comparator.</dct:description>
      </owl:NamedIndividual>
    </ns1:hasMember>
    <ns1:hasMember>
      <owl:NamedIndividual rdf:about="CheckMethodComparator-gt">
        <rdf:type rdf:resource="http://www.w3.org/2004/02/skos/core#Concept"/>
        <rdf:type rdf:resource="CheckMethodComparator"/>
        <rdfs:isDefinedBy rdf:resource="check_method_comparators"/>
        <skos:definition xml:lang="en">greater-than comparator.</skos:definition>
        <skos:inScheme rdf:resource="CheckMethodComparatorNomenclature"/>
        <skos:prefLabel xml:lang="en">greater than</skos:prefLabel>
        <skos:topConceptOf rdf:resource="CheckMethodComparatorNomenclature"/>
        <dct:title xml:lang="en">greater than</dct:title>
        <dct:description xml:lang="en">greater-than comparator.</dct:description>
      </owl:NamedIndividual>
    </ns1:hasMember>
    <ns1:hasMember>
      <owl:NamedIndividual rdf:about="CheckMethodComparator-ge">
        <rdf:type rdf:resource="http://www.w3.org/2004/02/skos/core#Concept"/>
        <rdf:type rdf:resource="CheckMethodComparator"/>
        <rdfs:isDefinedBy rdf:resource="check_method_comparators"/>
        <skos:definition xml:lang="en">greater-equal comparator.</skos:definition>
        <skos:inScheme rdf:resource="CheckMethodComparatorNomenclature"/>
        <skos:prefLabel xml:lang="en">greater equal</skos:prefLabel>
        <skos:topConceptOf rdf:resource="CheckMethodComparatorNomenclature"/>
        <dct:title xml:lang="en">greater equal</dct:title>
        <dct:description xml:lang="en">greater-equal comparator.</dct:description>
      </owl:NamedIndividual>
    </ns1:hasMember>
    <ns1:hasMember>
      <owl:NamedIndividual rdf:about="CheckMethodcomparator-logicalAND">
        <rdf:type rdf:resource="http://www.w3.org/2004/02/skos/core#Concept"/>
        <rdf:type rdf:resource="CheckMethodComparator"/>
        <rdfs:isDefinedBy rdf:resource="check_method_comparators"/>
        <skos:definition xml:lang="en">logical AND comparator.</skos:definition>
        <skos:inScheme rdf:resource="CheckMethodComparatorNomenclature"/>
        <skos:prefLabel xml:lang="en">logicalAND</skos:prefLabel>
        <skos:topConceptOf rdf:resource="CheckMethodComparatorNomenclature"/>
        <dct:title xml:lang="en">logicalAND</dct:title>
        <dct:description xml:lang="en">logical AND comparator.</dct:description>
      </owl:NamedIndividual>
    </ns1:hasMember>
    <ns1:hasMember>
      <owl:NamedIndividual rdf:about="CheckMethodComparator-logicalOR">
        <rdf:type rdf:resource="http://www.w3.org/2004/02/skos/core#Concept"/>
        <rdf:type rdf:resource="CheckMethodComparator"/>
        <rdfs:isDefinedBy rdf:resource="check_method_comparators"/>
        <skos:definition xml:lang="en">logical OR comparator.</skos:definition>
        <skos:inScheme rdf:resource="CheckMethodComparatorNomenclature"/>
        <skos:prefLabel xml:lang="en">logicalOR</skos:prefLabel>
        <skos:topConceptOf rdf:resource="CheckMethodComparatorNomenclature"/>
        <dct:title xml:lang="en">logicalOR</dct:title>
        <dct:description xml:lang="en">logical OR comparator.</dct:description>
      </owl:NamedIndividual>
    </ns1:hasMember>
  </owl:Class>
  <rdf:Description rdf:about="http://www.w3.org/2002/07/owl#Ontology">
    <ns1:hasMember rdf:resource="check_method_comparators"/>
  </rdf:Description>
  <owl:FunctionalProperty rdf:about="hasComparator">
    <rdf:type>
      <rdf:Description rdf:about="http://www.w3.org/2002/07/owl#ObjectProperty">
        <ns1:hasMember rdf:resource="hasComparator"/>
      </rdf:Description>
    </rdf:type>
    <rdfs:label xml:lang="en">has comparator</rdfs:label>
    <rdfs:comment xml:lang="en">The comparator of a feature of interest or a property of that is needed by the check method.
  A set of comparators is defined by aec3po in the corresponding concept scheme.</rdfs:comment>
    <rdfs:isDefinedBy rdf:resource="check_method_comparators"/>
    <rdfs:range rdf:resource="CheckMethod"/>
    <rdfs:subPropertyOf>
      <rdf:Description rdf:about="hasDesign">
        <ns1:superPropertyOf rdf:resource="hasComparator"/>
      </rdf:Description>
    </rdfs:subPropertyOf>
    <dct:title xml:lang="en">has comparator</dct:title>
    <dct:description xml:lang="en">The comparator of a feature of interest or a property of that is needed by the check method.
  A set of comparators is defined by aec3po in the corresponding concept scheme.</dct:description>
  </owl:FunctionalProperty>
  <rdf:Description rdf:about="http://www.w3.org/2002/07/owl#FunctionalProperty">
    <ns1:hasMember rdf:resource="hasComparator"/>
  </rdf:Description>
  <rdf:Description rdf:about="http://www.w3.org/2004/02/skos/core#ConceptScheme">
    <ns1:hasMember rdf:resource="CheckMethodComparatorNomenclature"/>
  </rdf:Description>
  <prov:Agent rdf:about="amna"/>
  <rdf:Description rdf:about="http://www.w3.org/2002/07/owl#NamedIndividual">
    <ns1:hasMember rdf:resource="CheckMethodcomparator-eq"/>
    <ns1:hasMember rdf:resource="CheckMethodComparator-neq"/>
    <ns1:hasMember rdf:resource="CheckMethodComparator-lt"/>
    <ns1:hasMember rdf:resource="CheckMethodComparator-le"/>
    <ns1:hasMember rdf:resource="CheckMethodComparator-gt"/>
    <ns1:hasMember rdf:resource="CheckMethodComparator-ge"/>
    <ns1:hasMember rdf:resource="CheckMethodcomparator-logicalAND"/>
    <ns1:hasMember rdf:resource="CheckMethodComparator-logicalOR"/>
  </rdf:Description>
  <rdf:Description rdf:about="http://www.w3.org/2002/07/owl#Class">
    <ns1:hasMember rdf:resource="CheckMethodComparator"/>
    <ns1:hasMember rdf:nodeID="n054a34c22b134c409ab2a872c59f32eab1"/>
  </rdf:Description>
  <rdf:Description rdf:about="http://www.w3.org/2002/07/owl#Restriction">
    <ns1:hasMember rdf:nodeID="n054a34c22b134c409ab2a872c59f32eab2"/>
  </rdf:Description>
</rdf:RDF>
