@base <https://w3id.org/lbd/aec3po/> .
@prefix aec3po: <https://w3id.org/lbd/aec3po/> .
@prefix cc: <http://creativecommons.org/ns#> .
@prefix dct: <http://purl.org/dc/terms/> .
@prefix ns1: <https://w3id.org/profile/ontdoc/> .
@prefix owl: <http://www.w3.org/2002/07/owl#> .
@prefix prov: <http://www.w3.org/ns/prov#> .
@prefix rdf: <http://www.w3.org/1999/02/22-rdf-syntax-ns#> .
@prefix rdfs: <http://www.w3.org/2000/01/rdf-schema#> .
@prefix skos: <http://www.w3.org/2004/02/skos/core#> .
@prefix vann: <http://purl.org/vocab/vann/> .
@prefix xsd: <http://www.w3.org/2001/XMLSchema#> .

<CheckMethodOperator> a rdfs:Class,
        owl:Class ;
    rdfs:label "check method operator"@en ;
    dct:description "Formally defined as the set of skos:Concept in concept scheme aec3po:CheckMethodOperatorNomenclature"@en ;
    dct:title "check method operator"@en ;
    rdfs:comment "Formally defined as the set of skos:Concept in concept scheme aec3po:CheckMethodOperatorNomenclature"@en ;
    rdfs:isDefinedBy <check_method_operators> ;
    rdfs:subClassOf skos:Concept,
        <CheckMethod> ;
    owl:equivalentClass _:ne52e7b893d57409bb4747ea36f44d160b1 ;
    ns1:hasMember <CheckMethodOperator-addition>,
        <CheckMethodOperator-division>,
        <CheckMethodOperator-exists>,
        <CheckMethodOperator-forall>,
        <CheckMethodOperator-multiplication>,
        <CheckMethodOperator-notExists>,
        <CheckMethodOperator-subtraction> .

rdfs:Class ns1:hasMember <CheckMethodOperator> .

owl:FunctionalProperty ns1:hasMember <hasOperator> .

owl:ObjectProperty ns1:hasMember <hasOperator> .

owl:Ontology ns1:hasMember <check_method_operators> .

owl:Restriction ns1:hasMember _:ne52e7b893d57409bb4747ea36f44d160b2 .

skos:ConceptScheme ns1:hasMember <CheckMethodOperatorNomenclature> .

<amna> a prov:Agent .

<hasDesign> ns1:superPropertyOf <hasOperator> .

owl:Class ns1:hasMember _:ne52e7b893d57409bb4747ea36f44d160b1,
        <CheckMethodOperator> .

<CheckMethod> ns1:inRangeOf <hasOperator> ;
    ns1:superClassOf <CheckMethodOperator> .

<CheckMethodOperator-addition> a owl:NamedIndividual,
        skos:Concept,
        <CheckMethodOperator> ;
    dct:description "addition operator."@en ;
    dct:title "addition"@en ;
    rdfs:isDefinedBy <check_method_operators> ;
    skos:definition "addition operator."@en ;
    skos:inScheme <CheckMethodOperatorNomenclature> ;
    skos:prefLabel "addition"@en ;
    skos:topConceptOf <CheckMethodOperatorNomenclature> .

<CheckMethodOperator-division> a owl:NamedIndividual,
        skos:Concept,
        <CheckMethodOperator> ;
    dct:description "division Operator."@en ;
    dct:title "division"@en ;
    rdfs:isDefinedBy <check_method_operators> ;
    skos:definition "division Operator."@en ;
    skos:inScheme <CheckMethodOperatorNomenclature> ;
    skos:prefLabel "division"@en ;
    skos:topConceptOf <CheckMethodOperatorNomenclature> .

<CheckMethodOperator-exists> a owl:NamedIndividual,
        skos:Concept,
        <CheckMethodOperator> ;
    dct:description "exists operator."@en ;
    dct:title "exists"@en ;
    rdfs:isDefinedBy <check_method_operators> ;
    skos:definition "exists operator."@en ;
    skos:inScheme <CheckMethodOperatorNomenclature> ;
    skos:prefLabel "exists"@en ;
    skos:topConceptOf <CheckMethodOperatorNomenclature> .

<CheckMethodOperator-forall> a owl:NamedIndividual,
        skos:Concept,
        <CheckMethodOperator> ;
    dct:description "forall operator."@en ;
    dct:title "forall"@en ;
    rdfs:isDefinedBy <check_method_operators> ;
    skos:definition "forall operator."@en ;
    skos:inScheme <CheckMethodOperatorNomenclature> ;
    skos:prefLabel "forall"@en ;
    skos:topConceptOf <CheckMethodOperatorNomenclature> .

<CheckMethodOperator-multiplication> a owl:NamedIndividual,
        skos:Concept,
        <CheckMethodOperator> ;
    dct:description "multiplication Operator."@en ;
    dct:title "multiplication"@en ;
    rdfs:isDefinedBy <check_method_operators> ;
    skos:definition "multiplication Operator."@en ;
    skos:inScheme <CheckMethodOperatorNomenclature> ;
    skos:prefLabel "multiplication"@en ;
    skos:topConceptOf <CheckMethodOperatorNomenclature> .

<CheckMethodOperator-notExists> a owl:NamedIndividual,
        skos:Concept,
        <CheckMethodOperator> ;
    dct:description "not exists operator."@en ;
    dct:title "not exists"@en ;
    rdfs:isDefinedBy <check_method_operators> ;
    skos:definition "not exists operator."@en ;
    skos:inScheme <CheckMethodOperatorNomenclature> ;
    skos:prefLabel "not exists"@en ;
    skos:topConceptOf <CheckMethodOperatorNomenclature> .

<CheckMethodOperator-subtraction> a owl:NamedIndividual,
        skos:Concept,
        <CheckMethodOperator> ;
    dct:description "subtraction operator."@en ;
    dct:title "subtraction"@en ;
    rdfs:isDefinedBy <check_method_operators> ;
    skos:definition "subtraction operator."@en ;
    skos:inScheme <CheckMethodOperatorNomenclature> ;
    skos:prefLabel "subtraction"@en ;
    skos:topConceptOf <CheckMethodOperatorNomenclature> .

<hasOperator> a owl:FunctionalProperty,
        owl:ObjectProperty ;
    rdfs:label "has operator"@en ;
    dct:description """The operator of a feature of interest or a property of that is needed by the check method.
  A set of operators is defined by aec3po in the corresponding concept scheme."""@en ;
    dct:title "has operator"@en ;
    rdfs:comment """The operator of a feature of interest or a property of that is needed by the check method.
  A set of operators is defined by aec3po in the corresponding concept scheme."""@en ;
    rdfs:isDefinedBy <check_method_Operators> ;
    rdfs:range <CheckMethod> ;
    rdfs:subPropertyOf <hasDesign> .

owl:NamedIndividual ns1:hasMember <CheckMethodOperator-addition>,
        <CheckMethodOperator-division>,
        <CheckMethodOperator-exists>,
        <CheckMethodOperator-forall>,
        <CheckMethodOperator-multiplication>,
        <CheckMethodOperator-notExists>,
        <CheckMethodOperator-subtraction> .

skos:Concept ns1:hasMember <CheckMethodOperator-addition>,
        <CheckMethodOperator-division>,
        <CheckMethodOperator-exists>,
        <CheckMethodOperator-forall>,
        <CheckMethodOperator-multiplication>,
        <CheckMethodOperator-notExists>,
        <CheckMethodOperator-subtraction> ;
    ns1:superClassOf <CheckMethodOperator> .

<check_method_operators> a owl:Ontology ;
    cc:license <https://creativecommons.org/licenses/by/4.0/> ;
    dct:contributor <amna> ;
    dct:created "2024-01-22"^^xsd:date ;
    dct:description "Definition of operators scheme for AEC3PO."@en ;
    dct:modified "2023-09-25"^^xsd:date,
        "2024-01-24"^^xsd:date ;
    dct:title "AEC3PO: Operators"@en ;
    vann:preferredNamespacePrefix "aec3po" ;
    vann:preferredNamespaceUri "https://w3id.org/lbd/aec3po/" .

<CheckMethodOperatorNomenclature> a skos:ConceptScheme ;
    rdfs:label "check method nomenclature"@en ;
    dct:description """A set of operators for the check method.
  AEC3PO includes a set of operators for this nomenclature.
  These operators are :
  - operator_exists : exists operator.
  - operator_notExists : not-exists operator.
  - operator_forall : forall operator."""@en ;
    dct:title "check method nomenclature"@en ;
    rdfs:isDefinedBy <check_method_operators> ;
    skos:definition """A set of operators for the check method.
  AEC3PO includes a set of operators for this nomenclature.
  These operators are :
  - operator_exists : exists operator.
  - operator_notExists : not-exists operator.
  - operator_forall : forall operator."""@en ;
    skos:hasTopConcept <CheckMethodOperator-addition>,
        <CheckMethodOperator-division>,
        <CheckMethodOperator-exists>,
        <CheckMethodOperator-forall>,
        <CheckMethodOperator-multiplication>,
        <CheckMethodOperator-notExists>,
        <CheckMethodOperator-subtraction> .

_:ne52e7b893d57409bb4747ea36f44d160b3 rdf:first skos:Concept ;
    rdf:rest ( _:ne52e7b893d57409bb4747ea36f44d160b2 ) .

_:ne52e7b893d57409bb4747ea36f44d160b1 a owl:Class ;
    owl:intersectionOf _:ne52e7b893d57409bb4747ea36f44d160b3 .

_:ne52e7b893d57409bb4747ea36f44d160b2 a owl:Restriction ;
    owl:hasValue <CheckMethodOperatorNomenclature> ;
    owl:onProperty skos:inScheme .

