@base <https://w3id.org/lbd/aec3po/> .
@prefix aec3po: <https://w3id.org/lbd/aec3po/> .
@prefix cc: <http://creativecommons.org/ns#> .
@prefix dct: <http://purl.org/dc/terms/> .
@prefix ns1: <https://w3id.org/profile/ontdoc/> .
@prefix owl: <http://www.w3.org/2002/07/owl#> .
@prefix prov: <http://www.w3.org/ns/prov#> .
@prefix rdf: <http://www.w3.org/1999/02/22-rdf-syntax-ns#> .
@prefix rdfs: <http://www.w3.org/2000/01/rdf-schema#> .
@prefix skos: <http://www.w3.org/2004/02/skos/core#> .
@prefix vann: <http://purl.org/vocab/vann/> .
@prefix xsd: <http://www.w3.org/2001/XMLSchema#> .

<Discipline> a rdfs:Class,
        owl:Class ;
    rdfs:label "Discipline"@en ;
    dct:description "The AEC discipline to which something pertains." ;
    dct:title "Discipline"@en ;
    rdfs:comment "The AEC discipline to which something pertains." ;
    rdfs:isDefinedBy <discipline> ;
    rdfs:subClassOf skos:Concept ;
    owl:equivalentClass _:n672c126a241a4d71b4a11c7a517dbb3eb1 ;
    ns1:hasMember <Discipline-architecture>,
        <Discipline-buildingServices>,
        <Discipline-construction>,
        <Discipline-planning>,
        <Discipline-structuralEngineering> ;
    ns1:inRangeOf <hasDiscipline> .

<http://maxime-lefrancois.info/me#> a prov:Agent .

rdfs:Class ns1:hasMember <Discipline> .

owl:ObjectProperty ns1:hasMember <hasDiscipline> .

owl:Ontology ns1:hasMember <discipline> .

owl:Restriction ns1:hasMember _:n672c126a241a4d71b4a11c7a517dbb3eb2 .

skos:ConceptScheme ns1:hasMember <DisciplineNomenclature> .

owl:Class ns1:hasMember _:n672c126a241a4d71b4a11c7a517dbb3eb1,
        <Discipline> .

<hasDiscipline> a owl:ObjectProperty ;
    rdfs:label "has discipline"@en ;
    dct:description "Links an entity (procedure, statement, verifier, ...) to the discipline to which it pertains."@en ;
    dct:title "has discipline"@en ;
    rdfs:comment "Links an entity (procedure, statement, verifier, ...) to the discipline to which it pertains."@en ;
    rdfs:isDefinedBy <discipline> ;
    rdfs:range <Discipline> .

<Discipline-architecture> a owl:NamedIndividual,
        skos:Concept,
        <Discipline> ;
    dct:description "The Architecture discipline."@en ;
    dct:title "architecture"@en ;
    rdfs:isDefinedBy <discipline> ;
    skos:definition "The Architecture discipline."@en ;
    skos:inScheme <DisciplineNomenclature> ;
    skos:prefLabel "architecture"@en ;
    skos:topConceptOf <DisciplineNomenclature> .

<Discipline-buildingServices> a owl:NamedIndividual,
        skos:Concept,
        <Discipline> ;
    dct:description "The Building Services discipline."@en ;
    dct:title "building services"@en ;
    rdfs:isDefinedBy <discipline> ;
    skos:definition "The Building Services discipline."@en ;
    skos:inScheme <DisciplineNomenclature> ;
    skos:prefLabel "building services"@en ;
    skos:topConceptOf <DisciplineNomenclature> .

<Discipline-construction> a owl:NamedIndividual,
        skos:Concept,
        <Discipline> ;
    dct:description "The Construction discipline."@en ;
    dct:title "construction"@en ;
    rdfs:isDefinedBy <discipline> ;
    skos:definition "The Construction discipline."@en ;
    skos:inScheme <DisciplineNomenclature> ;
    skos:prefLabel "construction"@en ;
    skos:topConceptOf <DisciplineNomenclature> .

<Discipline-planning> a owl:NamedIndividual,
        skos:Concept,
        <Discipline> ;
    dct:description "The Planning discipline."@en ;
    dct:title "planning"@en ;
    rdfs:isDefinedBy <discipline> ;
    skos:definition "The Planning discipline."@en ;
    skos:inScheme <DisciplineNomenclature> ;
    skos:prefLabel "planning"@en ;
    skos:topConceptOf <DisciplineNomenclature> .

<Discipline-structuralEngineering> a owl:NamedIndividual,
        skos:Concept,
        <Discipline> ;
    dct:description "The Structural Engineering discipline."@en ;
    dct:title "structural engineering"@en ;
    rdfs:isDefinedBy <discipline> ;
    skos:definition "The Structural Engineering discipline."@en ;
    skos:inScheme <DisciplineNomenclature> ;
    skos:prefLabel "structural engineering"@en ;
    skos:topConceptOf <DisciplineNomenclature> .

owl:NamedIndividual ns1:hasMember <Discipline-architecture>,
        <Discipline-buildingServices>,
        <Discipline-construction>,
        <Discipline-planning>,
        <Discipline-structuralEngineering> .

skos:Concept ns1:hasMember <Discipline-architecture>,
        <Discipline-buildingServices>,
        <Discipline-construction>,
        <Discipline-planning>,
        <Discipline-structuralEngineering> ;
    ns1:superClassOf <Discipline> .

<discipline> a owl:Ontology ;
    cc:license <https://creativecommons.org/licenses/by/4.0/> ;
    dct:contributor <http://maxime-lefrancois.info/me#> ;
    dct:created "2023-05-25"^^xsd:date ;
    dct:description "Definition of a disciplines concept scheme for AEC3PO."@en ;
    dct:modified "2023-05-25"^^xsd:date,
        "2023-08-31"^^xsd:date ;
    dct:title "AEC3PO: Disciplines"@en ;
    vann:preferredNamespacePrefix "aec3po" ;
    vann:preferredNamespaceUri "https://w3id.org/lbd/aec3po/" .

<DisciplineNomenclature> a skos:ConceptScheme ;
    rdfs:label "Discipline nomenclature"@en ;
    dct:description """A set of values for disciplines.
  AEC3PO includes a set of values for this nomenclature.
  These values are :
  - architecture;
  - construction;
  - structural engineering;
  - building services;
  - planning."""@en ;
    dct:title "Discipline nomenclature"@en ;
    rdfs:isDefinedBy <discipline> ;
    skos:definition """A set of values for disciplines.
  AEC3PO includes a set of values for this nomenclature.
  These values are :
  - architecture;
  - construction;
  - structural engineering;
  - building services;
  - planning."""@en ;
    skos:hasTopConcept <Discipline-architecture>,
        <Discipline-buildingServices>,
        <Discipline-construction>,
        <Discipline-planning>,
        <Discipline-structuralEngineering> .

_:n672c126a241a4d71b4a11c7a517dbb3eb3 rdf:first skos:Concept ;
    rdf:rest ( _:n672c126a241a4d71b4a11c7a517dbb3eb2 ) .

_:n672c126a241a4d71b4a11c7a517dbb3eb1 a owl:Class ;
    owl:intersectionOf _:n672c126a241a4d71b4a11c7a517dbb3eb3 .

_:n672c126a241a4d71b4a11c7a517dbb3eb2 a owl:Restriction ;
    owl:hasValue <DisciplineNomenclature> ;
    owl:onProperty skos:inScheme .

