@prefix aec3po: <https://w3id.org/lbd/aec3po/> .
@prefix dul: <http://www.ontologydesignpatterns.org/ont/dul/DUL.owl#> .
@prefix owl: <http://www.w3.org/2002/07/owl#> .
@prefix rdfs: <http://www.w3.org/2000/01/rdf-schema#> .

aec3po:Document a owl:Class ;
    rdfs:label "Document"@en ;
    rdfs:comment "A document is a written, drawn, presented, or memorialized representation of thought. (Source: Wikipedia)"@en ;
    rdfs:subClassOf aec3po:Medium .

aec3po:Drawing a owl:Class ;
    rdfs:label "Drawing"@en ;
    rdfs:comment "Drawing is a form of visual art in which an artist uses instruments to mark paper or other two-dimensional surface. (Source: Wikipedia)"@en ;
    rdfs:subClassOf aec3po:Medium .

aec3po:Image a owl:Class ;
    rdfs:label "Image"@en ;
    rdfs:comment "An image is a visual representation of something. It can be two-dimensional, three-dimensional, or somehow otherwise feed into the visual system to convey information. (Source: Wikipedia)"@en ;
    rdfs:subClassOf aec3po:Medium .

aec3po:Model a owl:Class ;
    rdfs:label "Model"@en ;
    rdfs:comment "A design model of a building."@en ;
    rdfs:subClassOf aec3po:Medium .

aec3po:hasMedium a owl:ObjectProperty ;
    rdfs:label "has medium"@en ;
    rdfs:comment "Links an entity (procedure, statement, verifier, ...) to the medium it uses." ;
    rdfs:range aec3po:Medium .

aec3po:hasRequiredMedium a owl:ObjectProperty ;
    rdfs:label "has required medium"@en ;
    rdfs:comment "Links " ;
    rdfs:range aec3po:Medium .

aec3po:Medium a owl:Class ;
    rdfs:label "Medium"@en ;
    rdfs:comment "A piece of information, such as a law, a norm, a drawing, a model."@en ;
    rdfs:subClassOf dul:InformationObject .

