@base <https://w3id.org/lbd/aec3po/> .
@prefix aec3po: <https://w3id.org/lbd/aec3po/> .
@prefix cc: <http://creativecommons.org/ns#> .
@prefix dct: <http://purl.org/dc/terms/> .
@prefix dicl: <https://w3id.org/digitalconstruction/0.5/Lifecycle#> .
@prefix ns1: <https://w3id.org/profile/ontdoc/> .
@prefix owl: <http://www.w3.org/2002/07/owl#> .
@prefix prov: <http://www.w3.org/ns/prov#> .
@prefix rdf: <http://www.w3.org/1999/02/22-rdf-syntax-ns#> .
@prefix rdfs: <http://www.w3.org/2000/01/rdf-schema#> .
@prefix skos: <http://www.w3.org/2004/02/skos/core#> .
@prefix vann: <http://purl.org/vocab/vann/> .
@prefix xsd: <http://www.w3.org/2001/XMLSchema#> .

<PermittingStage> a rdfs:Class,
        owl:Class ;
    rdfs:label "Permitting Stage"@en ;
    dct:description "The class of permitting stages."@en ;
    dct:title "Permitting Stage"@en ;
    rdfs:comment "The class of permitting stages."@en ;
    rdfs:isDefinedBy <permitting_stage> ;
    rdfs:subClassOf skos:Concept ;
    owl:equivalentClass _:ne5dc1f8852344c34af89b3454b75ae4bb1 ;
    ns1:hasMember <UK_Building_Control_Submission>,
        <UK_Planning_Permission> ;
    ns1:inRangeOf <hasPermittingStage> .

<http://maxime-lefrancois.info/me#> a prov:Agent .

rdfs:Class ns1:hasMember <PermittingStage> .

owl:ObjectProperty ns1:hasMember <hasPermittingStage> .

owl:Ontology ns1:hasMember <permitting_stage> .

owl:Restriction ns1:hasMember _:ne5dc1f8852344c34af89b3454b75ae4bb2 .

skos:ConceptScheme ns1:hasMember <PermittingStageNomenclature> .

owl:Class ns1:hasMember _:ne5dc1f8852344c34af89b3454b75ae4bb1,
        <PermittingStage> .

owl:NamedIndividual ns1:hasMember <UK_Building_Control_Submission>,
        <UK_Planning_Permission> .

<hasPermittingStage> a owl:ObjectProperty ;
    rdfs:label "has permitting stage"@en ;
    dct:description "Links an entity to the permitting stage this entity pertains"@en ;
    dct:title "has permitting stage"@en ;
    rdfs:comment "Links an entity to the permitting stage this entity pertains"@en ;
    rdfs:isDefinedBy <permitting_stage> ;
    rdfs:range <PermittingStage> ;
    owl:equivalentProperty dicl:hasStage .

skos:Concept ns1:hasMember <UK_Building_Control_Submission>,
        <UK_Planning_Permission> ;
    ns1:superClassOf <PermittingStage> .

<UK_Building_Control_Submission> a owl:NamedIndividual,
        skos:Concept,
        <PermittingStage> ;
    dct:description "The UK Building Control Submission permitting stage."@en ;
    dct:title "building control submission"@en ;
    rdfs:isDefinedBy <permitting_stage> ;
    skos:definition "The UK Building Control Submission permitting stage."@en ;
    skos:inScheme <PermittingStageNomenclature> ;
    skos:prefLabel "building control submission"@en ;
    skos:topConceptOf <PermittingStageNomenclature> ;
    <forAdministrativeArea> <England> .

<UK_Planning_Permission> a owl:NamedIndividual,
        skos:Concept,
        <PermittingStage> ;
    dct:description "The UK Planning Permission permitting stage."@en ;
    dct:title "planning permission"@en ;
    rdfs:isDefinedBy <permitting_stage> ;
    skos:definition "The UK Planning Permission permitting stage."@en ;
    skos:inScheme <PermittingStageNomenclature> ;
    skos:prefLabel "planning permission"@en ;
    skos:topConceptOf <PermittingStageNomenclature> ;
    <forAdministrativeArea> <England> .

<PermittingStageNomenclature> a skos:ConceptScheme ;
    rdfs:label "Permitting stage nomenclature"@en ;
    dct:description """A set of values for permitting stages.
  AEC3PO includes a set of values for this nomenclature.
  These values are :
  - UK_Building_Control_Submission;
  - UK_Planning_Permission."""@en ;
    dct:title "Permitting stage nomenclature"@en ;
    rdfs:isDefinedBy <permitting_stage> ;
    skos:definition """A set of values for permitting stages.
  AEC3PO includes a set of values for this nomenclature.
  These values are :
  - UK_Building_Control_Submission;
  - UK_Planning_Permission."""@en ;
    skos:hasTopConcept <UK_Building_Control_Submission>,
        <UK_Planning_Permission> .

<permitting_stage> a owl:Ontology ;
    cc:license <https://creativecommons.org/licenses/by/4.0/> ;
    dct:contributor <http://maxime-lefrancois.info/me#> ;
    dct:created "2023-05-25"^^xsd:date ;
    dct:description "Definition of a permitting stage concept scheme for AEC3PO."@en ;
    dct:modified "2023-05-25"^^xsd:date,
        "2023-08-31"^^xsd:date ;
    dct:title "AEC3PO: Permitting Stage"@en ;
    vann:preferredNamespacePrefix "aec3po" ;
    vann:preferredNamespaceUri "https://w3id.org/lbd/aec3po/" ;
    owl:imports <administrative_areas> .

_:ne5dc1f8852344c34af89b3454b75ae4bb3 rdf:first skos:Concept ;
    rdf:rest ( _:ne5dc1f8852344c34af89b3454b75ae4bb2 ) .

_:ne5dc1f8852344c34af89b3454b75ae4bb1 a owl:Class ;
    owl:intersectionOf _:ne5dc1f8852344c34af89b3454b75ae4bb3 .

_:ne5dc1f8852344c34af89b3454b75ae4bb2 a owl:Restriction ;
    owl:hasValue <PermittingStageNomenclature> ;
    owl:onProperty skos:inScheme .

