@prefix aec3po: <https://w3id.org/lbd/aec3po/> .
@prefix cc: <http://creativecommons.org/ns#> .
@prefix dct: <http://purl.org/dc/terms/> .
@prefix owl: <http://www.w3.org/2002/07/owl#> .
@prefix rdf: <http://www.w3.org/1999/02/22-rdf-syntax-ns#> .
@prefix rdfs: <http://www.w3.org/2000/01/rdf-schema#> .
@prefix skos: <http://www.w3.org/2004/02/skos/core#> .
@prefix vann: <http://purl.org/vocab/vann/> .
@prefix xsd: <http://www.w3.org/2001/XMLSchema#> .

aec3po:check_method_comparators a owl:Ontology ;
    cc:license <https://creativecommons.org/licenses/by/4.0/> ;
    dct:contributor aec3po:amna ;
    dct:description "Definition of comparators scheme for AEC3PO."@en ;
    dct:modified "2023-09-25"^^xsd:date ;
    dct:title "AEC3PO: Comparators"@en ;
    vann:preferredNamespacePrefix "aec3po" ;
    vann:preferredNamespaceUri "https://w3id.org/lbd/aec3po/" .
    
aec3po:CheckMethodComparator a owl:Class ;
    rdfs:label "check method comparator"@en ;
    rdfs:comment "Formally defined as the set of skos:Concept in concept scheme aec3po:CheckMethodComparatorNomenclature"@en ;
    rdfs:isDefinedBy aec3po:check_method_comparators ;
    rdfs:subClassOf skos:Concept,
        aec3po:CheckMethod ;
    owl:equivalentClass [ owl:intersectionOf ( skos:Concept [ a owl:Restriction ;
                        owl:hasValue aec3po:CheckMethodComparatorNomenclature ;
                        owl:onProperty skos:inScheme ] ) ] .

aec3po:CheckMethodComparatorNomenclature a skos:ConceptScheme ;
    rdfs:label "check method nomenclature"@en ;
    rdfs:isDefinedBy aec3po:check_method_comparators ;
    skos:definition """A set of comparators for the check method.
  AEC3PO includes a set of comparators for this nomenclature.
  These comparators are :
  - comparator_eq : equal-to comparator;
  - comparator_neq : not equal-to comparator.
  - comparator_lt : less-than comparator.
  - comparator_le : less-equal comparator.
  - comparator_gt : greater-than comparator.
  - comparator_ge : greater-equal comparator.
  - comparator_exists : exists comparator.
  - comparator_notExists : not-exists comparator.
  - comparator_forall : forall comparator."""@en ;
    skos:hasTopConcept aec3po:CheckMethodComparator-eq, 
        aec3po:CheckMethodComparator-neq, 
        aec3po:CheckMethodComparator-lt, 
        aec3po:CheckMethodComparator-le, 
        aec3po:CheckMethodComparator-gt,
        aec3po:CheckMethodComparator-ge,
        aec3po:CheckMethodComparator-exists,
        aec3po:CheckMethodComparator-notExists,
        aec3po:CheckMethodComparator-forall.

aec3po:CheckMethodComparator-eq a owl:NamedIndividual, skos:Concept,
        aec3po:CheckMethodComparator ;
    rdfs:isDefinedBy aec3po:check_method_comparators ;
    skos:definition "equal-to comparator."@en ;
    skos:inScheme aec3po:CheckMethodComparatorNomenclature ;
    skos:prefLabel "equal-to"@en ;
    skos:topConceptOf aec3po:CheckMethodComparatorNomenclature .

aec3po:CheckMethodComparator-neq a owl:NamedIndividual, skos:Concept,
        aec3po:CheckMethodComparator ;
    rdfs:isDefinedBy aec3po:check_method_comparators ;
    skos:definition "not equal-to comparator."@en ;
    skos:inScheme aec3po:CheckMethodComparatorNomenclature ;
    skos:prefLabel "not equal-to"@en ;
    skos:topConceptOf aec3po:CheckMethodComparatorNomenclature .

aec3po:CheckMethodComparator-lt a owl:NamedIndividual, skos:Concept,
        aec3po:CheckMethodComparator ;
    rdfs:isDefinedBy aec3po:check_method_comparators ;
    skos:definition "less-than comparator."@en ;
    skos:inScheme aec3po:CheckMethodComparatorNomenclature ;
    skos:prefLabel "less than"@en ;
    skos:topConceptOf aec3po:CheckMethodComparatorNomenclature .

aec3po:CheckMethodComparator-le a owl:NamedIndividual, skos:Concept,
        aec3po:CheckMethodComparator ;
    rdfs:isDefinedBy aec3po:check_method_comparators ;
    skos:definition "less-equal comparator."@en ;
    skos:inScheme aec3po:CheckMethodComparatorNomenclature ;
    skos:prefLabel "less equal"@en ;
    skos:topConceptOf aec3po:CheckMethodComparatorNomenclature .

aec3po:CheckMethodComparator-gt a owl:NamedIndividual, skos:Concept,
        aec3po:CheckMethodComparator ;
    rdfs:isDefinedBy aec3po:check_method_comparators ;
    skos:definition "greater-than comparator."@en ;
    skos:inScheme aec3po:CheckMethodComparatorNomenclature ;
    skos:prefLabel "greater than"@en ;
    skos:topConceptOf aec3po:CheckMethodComparatorNomenclature .

aec3po:CheckMethodComparator-ge a owl:NamedIndividual, skos:Concept,
        aec3po:CheckMethodComparator ;
    rdfs:isDefinedBy aec3po:check_method_comparators ;
    skos:definition "greater-equal comparator."@en ;
    skos:inScheme aec3po:CheckMethodComparatorNomenclature ;
    skos:prefLabel "greater equal"@en ;
    skos:topConceptOf aec3po:CheckMethodComparatorNomenclature .

aec3po:CheckMethodComparator-exists a owl:NamedIndividual, skos:Concept,
        aec3po:CheckMethodComparator ;
    rdfs:isDefinedBy aec3po:check_method_comparators ;
    skos:definition "exists comparator."@en ;
    skos:inScheme aec3po:CheckMethodComparatorNomenclature ;
    skos:prefLabel "exists"@en ;
    skos:topConceptOf aec3po:CheckMethodComparatorNomenclature .

aec3po:CheckMethodComparator-notExists a owl:NamedIndividual, skos:Concept,
        aec3po:CheckMethodComparator ;
    rdfs:isDefinedBy aec3po:check_method_comparators ;
    skos:definition "not exists comparator."@en ;
    skos:inScheme aec3po:CheckMethodComparatorNomenclature ;
    skos:prefLabel "not exists"@en ;
    skos:topConceptOf aec3po:CheckMethodComparatorNomenclature .

aec3po:CheckMethodComparator-forall a owl:NamedIndividual, skos:Concept,
        aec3po:CheckMethodComparator ;
    rdfs:isDefinedBy aec3po:check_method_comparators ;
    skos:definition "forall comparator."@en ;
    skos:inScheme aec3po:CheckMethodComparatorNomenclature ;
    skos:prefLabel "forall"@en ;
    skos:topConceptOf aec3po:CheckMethodComparatorNomenclature .

aec3po:hasComparator a owl:FunctionalProperty,
        owl:ObjectProperty ;
    rdfs:label "has comparator"@en ;
    rdfs:comment """The comparator/operator of a feature of interest or a property of that is needed by the check method.
  A set of comparators is defined by aec3po in the corresponding concept scheme."""@en ;
    rdfs:isDefinedBy aec3po:check_method_comparators ;
    rdfs:range aec3po:CheckMethod ;
    rdfs:subPropertyOf aec3po:hasDesign .
