@prefix aec3po: <https://w3id.org/lbd/aec3po/> .
@prefix cc: <http://creativecommons.org/ns#> .
@prefix dct: <http://purl.org/dc/terms/> .
@prefix dul: <http://www.ontologydesignpatterns.org/ont/dul/DUL.owl#> .
@prefix owl: <http://www.w3.org/2002/07/owl#> .
@prefix rdfs: <http://www.w3.org/2000/01/rdf-schema#> .
@prefix vann: <http://purl.org/vocab/vann/> .
@prefix xsd: <http://www.w3.org/2001/XMLSchema#> .

aec3po:Document a owl:Class ;
    rdfs:label "Document"@en ;
    rdfs:comment "A document is a written, drawn, presented, or memorialized representation of thought. (Source: Wikipedia)"@en ;
    rdfs:isDefinedBy aec3po:mediums ;
    rdfs:subClassOf aec3po:Medium .

aec3po:Drawing a owl:Class ;
    rdfs:label "Drawing"@en ;
    rdfs:comment "Drawing is a form of visual art in which an artist uses instruments to mark paper or other two-dimensional surface. (Source: Wikipedia)"@en ;
    rdfs:isDefinedBy aec3po:mediums ;
    rdfs:subClassOf aec3po:Medium .

aec3po:Image a owl:Class ;
    rdfs:label "Image"@en ;
    rdfs:comment "An image is a visual representation of something. It can be two-dimensional, three-dimensional, or somehow otherwise feed into the visual system to convey information. (Source: Wikipedia)"@en ;
    rdfs:isDefinedBy aec3po:mediums ;
    rdfs:subClassOf aec3po:Medium .

aec3po:Model a owl:Class ;
    rdfs:label "Model"@en ;
    rdfs:comment "A design model of a building."@en ;
    rdfs:isDefinedBy aec3po:mediums ;
    rdfs:subClassOf aec3po:Medium .

aec3po:hasRequiredMedium a owl:ObjectProperty ;
    rdfs:label "has required medium"@en ;
    rdfs:comment "Links " ;
    rdfs:isDefinedBy aec3po:mediums ;
    rdfs:range aec3po:Medium ;
    rdfs:subPropertyOf aec3po:hasMedium .

aec3po:hasMedium a owl:ObjectProperty ;
    rdfs:label "has medium"@en ;
    rdfs:comment "Links an entity (procedure, statement, verifier, ...) to the medium it uses." ;
    rdfs:isDefinedBy aec3po:mediums ;
    rdfs:range aec3po:Medium .

aec3po:Medium a owl:Class ;
    rdfs:label "Medium"@en ;
    rdfs:comment "A piece of information, such as a law, a norm, a drawing, a model."@en ;
    rdfs:isDefinedBy aec3po:mediums ;
    rdfs:subClassOf dul:InformationObject .

aec3po:mediums a owl:Ontology ;
    cc:license <https://creativecommons.org/licenses/by/4.0/> ;
    dct:contributor <http://maxime-lefrancois.info/me#> ;
    dct:description "Definition of a set of classes for Mediums for AEC3PO."@en ;
    dct:modified "2023-05-25"^^xsd:date ;
    dct:title "AEC3PO: Mediums"@en ;
    vann:preferredNamespacePrefix "aec3po" ;
    vann:preferredNamespaceUri aec3po: .

