@prefix aec3po: <https://w3id.org/lbd/aec3po/> .
@prefix cc: <http://creativecommons.org/ns#> .
@prefix dct: <http://purl.org/dc/terms/> .
@prefix dul: <http://www.ontologydesignpatterns.org/ont/dul/DUL.owl#> .
@prefix eli: <http://data.europa.eu/eli/ontology#> .
@prefix owl: <http://www.w3.org/2002/07/owl#> .
@prefix quantitykind: <http://qudt.org/vocab/quantitykind/> .
@prefix rdf: <http://www.w3.org/1999/02/22-rdf-syntax-ns#> .
@prefix rdfs: <http://www.w3.org/2000/01/rdf-schema#> .
@prefix skos: <http://www.w3.org/2004/02/skos/core#> .
@prefix vann: <http://purl.org/vocab/vann/> .
@prefix xsd: <http://www.w3.org/2001/XMLSchema#> .
@prefix og: <https://ogp.me/> .

aec3po:Statement a owl:Class ;
    rdfs:label "Statement"@en ;
    rdfs:comment "refers clarifies expectations, and outlines standards to be followed by architects, engineers, contractors, builders, and other stakeholders involved in the construction and maintenance of buildings."@en ;
    rdfs:subClassOf aec3po:DocumentSubdivision ;
    skos:example "Any solar protection solutions in the building shall be taken into account in the calculation of solar energy gains for the building."@en .

aec3po:CheckStatement a owl:Class ;
    rdfs:label "Check Statement"@en ;
    rdfs:comment "refers to a type of statement that is used to specify conditions, criteria, or rules for evaluating the compliance, correctness, or validity of certain properties, features, or aspects of a system, process, or domain."@en ;
    rdfs:subClassOf aec3po:Statement .

aec3po:ChecklistStatement a owl:Class ;
 rdfs:comment "Checklist statement is a type of statement that represents a list of checks that need to be verified."@en ;
    rdfs:subClassOf aec3po:Statement .

aec3po:AndCheck a owl:Class ;
    rdfs:label "And Check"@en ;
    rdfs:comment "Check verified if and only if all of its sub-checks are verified."@en ;
    rdfs:subClassOf [ a owl:Restriction ;
            owl:minCardinality 1 ;
            owl:onProperty aec3po:hasSubCheck ],
        aec3po:ChecklistStatement .
aec3po:CheckStatement a owl:Class ;
 rdfs:comment "Check statement represents a formal statement or requirement that is used to assess whether a specific condition or criterion has been met in a construction project, design, or process. It generally refers to a textual extract from the building regulations."@en ;
    rdfs:subClassOf aec3po:ChecklistStatement .

aec3po:OrCheck a owl:Class ;
    rdfs:label "Or Check"@en ;
    rdfs:comment "Check verified if and only if at least one of its sub-checks is verified."@en ;
    rdfs:subClassOf [ a owl:Restriction ;
            owl:minCardinality 1 ;
            owl:onProperty aec3po:hasSubCheck ],
        aec3po:ChecklistStatement .

aec3po:CategoryCheckStatement a owl:Class ;
 rdfs:comment "Category check statement refers to a type of statement or requirement that focuses on verifying compliance with specific categories of regulations, standards, or guidelines within the construction industry. Category check statements are used to assess whether a construction project aligns with predefined categories of criteria, such as safety, environmental impact, energy efficiency, accessibility, and more."@en ;
    rdfs:subClassOf aec3po:CheckStatement .

aec3po:CertificateCheckStatement a owl:Class ;
 rdfs:comment "Certificate check statement refers to a type of statement or requirement that focuses on verifying and validating the authenticity and compliance of certificates related to construction projects"@en ;
    rdfs:subClassOf aec3po:CheckStatement .

#NOTE: This should be placed in the Check_Method module
aec3po:ComponentCheck a owl:Class ;
   rdfs:label "Component Check"@en ;
    rdfs:comment "Formally defined as checks for some feature of interest."@en ;
    rdfs:subClassOf aec3po:Check ;
    owl:equivalentClass [ a owl:Class ;
            owl:intersectionOf ( aec3po:Check [ a owl:Restriction ;
                        owl:allValuesFrom [ a owl:Restriction ;
                                owl:allValuesFrom aec3po:FeatureOfInterest ;
                                owl:onProperty [ owl:inverseOf aec3po:forDesign ] ] ;
                        owl:onProperty aec3po:forDesign ] ) ] .

aec3po:DefinitionStatement a owl:Class ;
 rdfs:comment "A type of statement that provides a formal and precise definition for a specific concept or term."@en ;
    rdfs:subClassOf aec3po:Statement .

aec3po:HumanEvaluatedStatement a owl:Class ;
    rdfs:comment "A type of check that is evaluated by a human. Those are primarily for issues of perception, e.g. \"is aesthetically appropriate\"." ;
    rdfs:subClassOf aec3po:Statement .

aec3po:NumericalCheckStatement a owl:Class ;
    rdfs:comment "A type of check that involves checking one numerical property against another, i.e. x < y or similar." ;
    rdfs:subClassOf aec3po:Statement .

aec3po:BooleanCheckStatement a owl:Class ;
    rdfs:comment "A type of check that checks the existence of an element (property) related to a feature of interest."@en ;
    rdfs:subClassOf aec3po:Statement .

aec3po:DataRequirement a owl:Class;
    rdfs:comment "Data-informed by a Statement which is required in order to perform a check to demonstrate compliance checking." .
      
aec3po:IDS a owl:Class ;
    rdfs:subClassOf aec3po:DataRequirement ;
    skos:note "Required data defined in an Information Delivery Format (IDS)." .

#NOTE: This should be removed.
aec3po:NumericalCheck a owl:Class ;
    rdfs:comment "A check that involves checking one numerical property against another, i.e. x < y or similar." ;
    rdfs:subClassOf aec3po:Check .

aec3po:PrivateVerifier a owl:Class ;
    rdfs:label "Private Verifier"@en ;
    rdfs:comment "Private verifier refers to an individual or entity responsible for independently assessing and verifying compliance with regulatory, safety, quality, and design requirements in a construction project. "@en ;
    rdfs:subClassOf aec3po:LegalVerifier .

aec3po:StateVerifier a owl:Class ;
    rdfs:label "State Verifier"@en ;
    rdfs:comment "State verifier refers to an individual or entity responsible for assessing and verifying compliance with state-specific regulations, legal requirements, and building codes in a construction project. "@en ;
    rdfs:subClassOf aec3po:LegalVerifier .

#NOTE: We used the property "hasRequiredData".
aec3po:hasDataRequirement a owl:ObjectProperty;
 rdfs:comment "todo"@en ;
   rdfs:domain aec3po:DataRequirement.

aec3po:PropertyDesign a owl:Class ;
    rdfs:label "property design"@en ;
    rdfs:comment "Designs that assign a value expressed as a literal to some property of a feature of interest."@en ;
    rdfs:subClassOf [ a owl:Restriction ;
            owl:allValuesFrom aec3po:Property ;
            owl:onProperty [ owl:inverseOf aec3po:hasDesign ] ],
        [ a owl:Restriction ;
            owl:cardinality 1 ;
            owl:onProperty aec3po:hasValue ],
        aec3po:Design ;
    skos:note "The value of the literal may be a XSD literal (boolean, integer, decimal, string), it may also use custom datatypes such as cdt:ucum"@en .

aec3po:ClassificationDesign a owl:Class ;
    rdfs:label "classification design"@en ;
    rdfs:comment "Designs that take values in classification schemes, described using SKOS"@en ;
    owl:equivalentClass [ owl:intersectionOf ( skos:Concept [ a owl:Restriction ;
                        owl:onProperty skos:inScheme ;
                        owl:someValuesFrom skos:ConceptScheme ] ) ] ;
    skos:note """classification design are expected to be taken in existing concept schemes. AEC3PO defines some concept schemes such as aec3po:building_structure. Existing concept schemes may also be used such as Ifc classes, or bSDD."""@en .
aec3po:hasComparisonOperator a owl:FunctionalProperty,
        owl:ObjectProperty ;
    rdfs:label "has comparisonOperator"@en ;
    rdfs:comment "The comparisonOperator of a property kind design. A set of values is defined by C3PO in the corresponding concept scheme."@en ;
    rdfs:range aec3po:ComparisonOperator ;
    rdfs:subPropertyOf aec3po:hasDesign .

skos:ConceptScheme a owl:Class .

skos:inScheme a owl:ObjectProperty .

aec3po:LegalVerifier a owl:Class ;
    rdfs:label "Legal Verifier"@en ;
    rdfs:comment "An entity that has the legal capacity to verify compliance with this regulation."@en .

aec3po:forDesign a owl:ObjectProperty ;
    rdfs:label "for design"@en ;
    rdfs:comment "Links a check, verifier, or checking act, to the type of design it applies."@en ;
    rdfs:domain [ a owl:Class ;
            owl:unionOf ( aec3po:Check aec3po:Verifier aec3po:Checking ) ] ;
    rdfs:range aec3po:Design .

#NOTE: domain and range here should be unionof (CheckStatement, CheckMethod)?
aec3po:hasSubCheck a owl:ObjectProperty ;
    rdfs:label "has sub check"@en ;
    rdfs:comment "Links a AndCheck to the set of checks that all need to be verified. Links a OrCheck to the set of checks that at least one must verify."@en ;
    rdfs:domain aec3po:Check ;
    rdfs:range aec3po:Check .

aec3po:hasDesign a owl:ObjectProperty ;
    rdfs:label "has design"@en ;
    rdfs:comment "Links a feature of interest or a property to a description of its design."@en ;
    rdfs:domain [ a owl:Class ;
            owl:unionOf ( aec3po:FeatureOfInterest aec3po:Property ) ] ;
    rdfs:range aec3po:Design .

aec3po:hasContext a owl:Property ;
    rdfs:label "has Context"@en ;
    rdfs:comment "Represents which bSDD context a given ontology concept or property refers."@en ;
    rdfs:domain [ a owl:Class ;
            owl:unionOf ( aec3po:Class aec3po:Property ) ] ;
    rdfs:range og:url .

aec3po:Property a owl:Class ;
    rdfs:label "Property"@en ;
    rdfs:comment "An aspect of a feature of interest that is intrinsic to and cannot exist without the feature of interest."@en ;
    rdfs:subClassOf dul:Quality ;
    skos:example "The height of a building"@en, "the area of a space"@en, "the U-value of a wall"@en .


aec3po:Application a owl:Class ;
    rdfs:label "Application"@en ;
    rdfs:comment "Represents the Applications tag in the semantic mark-up Requirement Application Selection and Exception (RASE) methodology."@en ;
    rdfs:subClassOf aec3po:Statement ;
owl:disjointWith aec3po:Selection, aec3po:Requirement,  aec3po:Exceptions .			

aec3po:Exception a owl:Class ;
    rdfs:label "Exception"@en ;
    rdfs:comment "Represents the Exception tag in the semantic mark-up Requirement Application Selection and Exception (RASE) methodology."@en ;
    rdfs:subClassOf aec3po:Statement ;
    owl:disjointWith  aec3po:Selection, aec3po:Application, aec3po:Requirement .			

aec3po:Requirement a owl:Class ;
    rdfs:label "Requirement"@en ;
    rdfs:comment "Represents the Requirement tag in the semantic mark-up Requirement Application Selection and Exception (RASE) methodology."@en ;
    rdfs:subClassOf aec3po:Statement ;
    owl:disjointWith  aec3po:Selection, aec3po:Application, aec3po:Exception .	

aec3po:Selection a owl:Class ;
    rdfs:label "Selection"@en ;
    rdfs:comment "Represents the Selection tag in the semantic mark-up Requirements Applications Selections and Exceptions (RASE) methodology."@en ;
    rdfs:subClassOf aec3po:Statement ;
    owl:disjointWith   aec3po:Requirement, aec3po:Application, aec3po:Exception .	

#NOTE: We don't have the class Check anymore. Do you mean CheckMethod or CheckStatement?
aec3po:Function a owl:Class ;
rdfs:label "Function"@en ;
rdfs:comment "todo" ;
rdfs:subClassOf aec3po:Check .

skos:Concept a owl:Class .

aec3po:ontology a owl:Ontology ;
    cc:license <https://creativecommons.org/licenses/by/4.0/> ;
    dct:contributor <http://maxime-lefrancois.info/me#>,
        aec3po:edlira,
        aec3po:etc,
        aec3po:pan,
        aec3po:thomas ;
    dct:description "The Architecture, Engineering and Construction Compliance Checking and Permitting ontology (AEC3PO), based on the statements on building compliance-related document and design codes."@en ;
    dct:modified "2023-05-25"^^xsd:date ;
    dct:title "AEC3PO"@en ;
    vann:preferredNamespacePrefix "aec3po" ;
    vann:preferredNamespaceUri aec3po: ;
    skos:note "Main classes and properties in the AEC3PO ontology are aligned to higher level ontologies, such as DUL."@en .

[] a owl:AllDisjointClasses ;
    owl:members ( aec3po:FeatureOfInterest aec3po:Property aec3po:QuantityKind aec3po:DocumentSubdivision aec3po:Check aec3po:Verifier aec3po:Checking ) .

