@prefix aec3po: <https://w3id.org/lbd/aec3po/> .
@prefix cc: <http://creativecommons.org/ns#> .
@prefix dct: <http://purl.org/dc/terms/> .
@prefix dul: <http://www.ontologydesignpatterns.org/ont/dul/DUL.owl#> .
@prefix owl: <http://www.w3.org/2002/07/owl#> .
@prefix rdfs: <http://www.w3.org/2000/01/rdf-schema#> .
@prefix skos: <http://www.w3.org/2004/02/skos/core#> .
@prefix vann: <http://purl.org/vocab/vann/> .
@prefix xsd: <http://www.w3.org/2001/XMLSchema#> .

aec3po:checking_act a owl:Ontology ;
    cc:license <https://creativecommons.org/licenses/by/4.0/> ;
    dct:contributor <http://maxime-lefrancois.info/me#> ;
    dct:description "The AEC3PO Checking Act module describes the act of checking some entities for something and generating a compliance verification report."@en ;
    dct:modified "2023-05-26"^^xsd:date ;
    dct:title "AEC3PO: Checking Act"@en ;
    owl:imports aec3po:check_method , aec3po:compliance_report ;
    vann:preferredNamespacePrefix "aec3po" ;
    vann:preferredNamespaceUri "https://w3id.org/lbd/aec3po/" .

aec3po:CheckingAct a owl:Class ;
    rdfs:label "Checking Act"@en ;
    rdfs:comment """Act of checking some entities for something and generating a compliance verification report. 
    
- Links to the check method that was used, which operationalizes a statement in a document;
- Links to the process verifier that made the checking act;
- Links to the entities that are checked;
- Links to compliance verification report that resulted.

"""@en ;
    rdfs:isDefinedBy aec3po:checking_act ;
    rdfs:subClassOf [ a owl:Restriction ;
            owl:someValuesFrom aec3po:CheckMethod ;
            owl:onProperty aec3po:usedMethod ],
        [ a owl:Restriction ;
            owl:onProperty aec3po:madeBy ;
            owl:someValuesFrom aec3po:ProcessVerifier ],
        [ a owl:Restriction ;
            owl:someValuesFrom owl:Thing ;
            owl:onProperty aec3po:checked ],
        [ a owl:Restriction ;
            owl:someValuesFrom aec3po:ComplianceReport ;
            owl:onProperty aec3po:hasReport ],
        dul:Event .

aec3po:usedMethod a owl:ObjectProperty ;
    rdfs:label "used method"@en ;
    rdfs:comment "Links a checking act to the method it used (a aec3po:CheckMethod)."@en ;
    rdfs:domain aec3po:CheckingAct ;
    rdfs:isDefinedBy aec3po:checking_act ;
    rdfs:range aec3po:CheckMethod .

aec3po:madeBy a owl:ObjectProperty ;
    rdfs:label "made by"@en ;
    rdfs:comment "Links a checking act to the process verifier that made it (a aec3po:ProcessVerifier)."@en ;
    rdfs:domain aec3po:CheckingAct ;
    rdfs:isDefinedBy aec3po:checking_act ;
    rdfs:range aec3po:ProcessVerifier .

aec3po:checks a owl:ObjectProperty ;
    rdfs:label "checks"@en ;
    rdfs:comment "Links a checking act to some entity it checked."@en ;
    rdfs:domain aec3po:CheckingAct ;
    rdfs:isDefinedBy aec3po:checking_act .

aec3po:hasReport a owl:ObjectProperty ;
    rdfs:label "has report"@en ;
    rdfs:comment "Links a checking act to the resulting compliance verification report."@en ;
    rdfs:domain aec3po:CheckingAct ;
    rdfs:isDefinedBy aec3po:checking_act ;
    rdfs:range aec3po:ComplianceReport .

## moved to Compliance_Report Module
#aec3po:ComplianceReport a owl:Class ;
    #rdfs:label "Compliance Verification Report"@en ;
   # rdfs:comment """The class of compliance verification reports resulting from checking acts."""@en ;
   # rdfs:isDefinedBy aec3po:checking_act ;
   # rdfs:subClassOf [ a owl:Restriction ;
          #  owl:onProperty aec3po:conforms ;
           # owl:cardinality 1 ] .

#aec3po:conforms a owl:DatatypeProperty ;
  #  rdfs:label "conforms"@en ;
 #   rdfs:comment "True if the checking act did not produce any validation results, and false otherwise."@en ;
 #   rdfs:domain aec3po:ComplianceReport ;
  #  rdfs:isDefinedBy aec3po:checking_act ;
   # rdfs:range xsd:boolean .

