@prefix aec3po: <https://w3id.org/lbd/aec3po/> .
@prefix cc: <http://creativecommons.org/ns#> .
@prefix dct: <http://purl.org/dc/terms/> .
@prefix dul: <http://www.ontologydesignpatterns.org/ont/dul/DUL.owl#> .
@prefix owl: <http://www.w3.org/2002/07/owl#> .
@prefix rdfs: <http://www.w3.org/2000/01/rdf-schema#> .
@prefix skos: <http://www.w3.org/2004/02/skos/core#> .
@prefix vann: <http://purl.org/vocab/vann/> .
@prefix xsd: <http://www.w3.org/2001/XMLSchema#> .

aec3po:design a owl:Ontology ;
    cc:license <https://creativecommons.org/licenses/by/4.0/> ;
    dct:contributor <http://maxime-lefrancois.info/me#> ;
    dct:description "The AEC3PO Design module describes descriptions of some design of features of interest, in terms of structure, geometry, and function."@en ;
    dct:modified "2023-05-25"^^xsd:date ;
    dct:title "AEC3PO: Design"@en ;
    owl:imports aec3po:quantity_kinds ;
    vann:preferredNamespacePrefix "aec3po" ;
    vann:preferredNamespaceUri "https://w3id.org/lbd/aec3po/" .

aec3po:Design a owl:Class ;
    rdfs:label "Design"@en ;
    rdfs:comment """A Description of some design of a feature of interest, in terms of structure, geometry, and function. 
    May be linked to a feature of interest to describe the design it has, for example using the ClassificationDesign subclass.
    May be linked to a check, verifier, or check result, to describe the kind of design it is for."""@en ;
    rdfs:isDefinedBy aec3po:design ;
    rdfs:subClassOf dul:Design ;
    skos:example """Example: 
- the type of use of a building (Residential / Commercial)
- the type of structural material (steel/ RC / timber)
- the designed height of a building (High-rise, Mid-rise, Low-rise)
- the area of space abc in IFC model xyz is 14 m2"""@en .

aec3po:hasDesign a owl:ObjectProperty ;
    rdfs:label "has design"@en ;
    rdfs:comment "Links a feature of interest or a property to a description of its design."@en ;
    rdfs:domain [ a owl:Class ;
            owl:unionOf ( aec3po:FeatureOfInterest aec3po:Property ) ] ;
    rdfs:range aec3po:Design ;
    rdfs:isDefinedBy aec3po:design .

aec3po:PropertyDesign a owl:Class ;
    rdfs:label "property design"@en ;
    rdfs:comment "Designs that assign a value expressed as a literal to some property of a feature of interest."@en ;
    rdfs:subClassOf [ a owl:Restriction ;
            owl:allValuesFrom aec3po:Property ;
            owl:onProperty [ owl:inverseOf aec3po:hasDesign ] ],
        [ a owl:Restriction ;
            owl:cardinality 1 ;
            owl:onProperty aec3po:hasValue ],
        aec3po:Design ;
    skos:note "The value of the literal may be a XSD literal (boolean, integer, decimal, string), it may also use custom datatypes such as cdt:ucum"@en ;
    rdfs:isDefinedBy aec3po:design .
