@prefix aec3po: <https://w3id.org/lbd/aec3po/> .
@prefix cc: <http://creativecommons.org/ns#> .
@prefix dct: <http://purl.org/dc/terms/> .
@prefix dul: <http://www.ontologydesignpatterns.org/ont/dul/DUL.owl#> .
@prefix owl: <http://www.w3.org/2002/07/owl#> .
@prefix rdfs: <http://www.w3.org/2000/01/rdf-schema#> .
@prefix skos: <http://www.w3.org/2004/02/skos/core#> .
@prefix vann: <http://purl.org/vocab/vann/> .
@prefix xsd: <http://www.w3.org/2001/XMLSchema#> .

aec3po:document a owl:Ontology ;
 cc:license <https://creativecommons.org/licenses/by/4.0/> ;
 dct:contributor <http://maxime-lefrancois.info/me#> ;
 dct:description """The AEC3PO Document module describes a document, of any kind, typically related to compliance and permitting. Documents are split into division and subdivisions, down to individual statements.

Document subdivisions can be described as literals, link to their first part, and to their immediate following subdivision. This enables roundtripping from a document to its AEC3PO description, and back."""@en ;
 dct:description <document.png> ;
 dct:modified "2023-05-25"^^xsd:date ;
 dct:title "AEC3PO: document"@en ;
 vann:preferredNamespacePrefix "aec3po" ;
 vann:preferredNamespaceUri "https://w3id.org/lbd/aec3po/" .

aec3po:Document a owl:Class ;
 rdfs:label "Document"@en ;
 rdfs:comment "A document representing AEC regulations, guidelines, building codes etc."@en ;
 skos:note "a Document is expected to be annotated using properties from the Dublin Core Terms vocabulary."@en ;
 skos:example "Approved Document A, Eurocode, Finish Regulations, etc."@en ;
 rdfs:isDefinedBy aec3po:document .

    aec3po:forDocument a owl:ObjectProperty ;
    rdfs:label "for document"@en ;
    rdfs:comment "links an entity such as a legal verifier to the document it is for."@en ;
    rdfs:range aec3po:Document ;
    rdfs:isDefinedBy aec3po:document ;
    # rdfs:domain aec3po:LegalVerifier ; # entity **such as** a legal verifier
    rdfs:range aec3po:Document .

    aec3po:usesDocument a owl:ObjectProperty ;
    rdfs:label "uses document"@en ;
    rdfs:comment "Links an entity (procedure, statement, verifier, ...) to the document it uses."@en ;
    rdfs:isDefinedBy aec3po:document ;
    rdfs:range aec3po:Document ;
    # rdfs:domain aec3po:LegalVerifier ; # entity **such as** a legal verifier
    rdfs:range aec3po:Document .

    aec3po:requiresDocument a owl:ObjectProperty ;
    rdfs:label "requires document"@en ;
    rdfs:comment "Links an entity (procedure, statement, verifier, ...) to the document it requires."@en ;
    rdfs:isDefinedBy aec3po:document ;
    rdfs:subPropertyOf aec3po:usesDocument ;
    rdfs:range aec3po:Document .

aec3po:DocumentSubdivision a owl:Class ;
 rdfs:label "Document Subdivision"@en ;
 rdfs:comment "Any subdivision of a document, including sections, paragraphs, definitions, words, etc."@en ;
 rdfs:isDefinedBy aec3po:document ;
 rdfs:subClassOf [ a owl:Restriction ; owl:onProperty aec3po:hasSubdivision ; owl:allValuesFrom aec3po:DocumentSubdivision ] ;
 skos:example "Paragraph, section, definition..."@en .

aec3po:DocumentSubdivision_asLiteral a owl:DatatypeProperty ;
 rdfs:label "as literal"@en ;
 rdfs:comment "Links a document subdivision to its literal representation. The literal datatype may be xsd:string, rdf:HTMLLiteral, xsd:base64Binary, or any other relevant datatype."@en ;
 skos:hiddenLabel "text" ; # alias name for JSON-LD and YAML-LD
 rdfs:isDefinedBy aec3po:document ;
 rdfs:domain aec3po:DocumentSubdivision ;
 rdfs:range rdfs:Literal .

aec3po:hasSubdivision a owl:ObjectProperty ;
 rdfs:label "has subdivision"@en ;
 rdfs:comment "links a document part to some of its subdivision"@en ;
 rdfs:domain [ owl:unionOf ( aec3po:Document aec3po:DocumentSubdivision ) ] ;
 rdfs:range aec3po:DocumentSubdivision ;
 rdfs:subPropertyOf dct:hasPart ;
 rdfs:isDefinedBy aec3po:document . 

aec3po:hasNextSubdivision a owl:ObjectProperty , owl:FunctionalProperty ;
 rdfs:label "has next subdivision"@en ;
 rdfs:comment "Links a document subdivision to the document subdivision that immediately follows it, if it exists"@en ;
 rdfs:domain aec3po:DocumentSubdivision ;
 rdfs:range aec3po:DocumentSubdivision ;
 rdfs:isDefinedBy aec3po:document .

aec3po:hasFirstSubdivision a owl:ObjectProperty , owl:FunctionalProperty ;
 rdfs:label "has first subdivision"@en ;
 rdfs:comment "Links a document part to the first of its subdivision"@en ;
 rdfs:domain [ owl:unionOf ( aec3po:Document aec3po:DocumentSubdivision ) ] ;
 rdfs:range aec3po:DocumentSubdivision ;
 rdfs:subPropertyOf aec3po:hasSubdivision ;
 rdfs:isDefinedBy aec3po:document .

aec3po:Drawing a owl:Class ;
 rdfs:label "Drawing"@en ;
 rdfs:comment "Drawing is a form of visual art in which an artist uses instruments to mark paper or other two-dimensional surface. (Source: Wikipedia)"@en ;
 rdfs:subClassOf aec3po:Document ;
 rdfs:isDefinedBy aec3po:document .

aec3po:Image a owl:Class ;
 rdfs:label "Image"@en ;
 rdfs:comment "An image is a visual representation of something. It can be two-dimensional, three-dimensional, or somehow otherwise feed into the visual system to convey information. (Source: Wikipedia)"@en ;
 rdfs:subClassOf aec3po:Document ;
 rdfs:isDefinedBy aec3po:document .
