@prefix aec3po: <https://w3id.org/lbd/aec3po/> .
@prefix cc: <http://creativecommons.org/ns#> .
@prefix dct: <http://purl.org/dc/terms/> .
@prefix dul: <http://www.ontologydesignpatterns.org/ont/dul/DUL.owl#> .
@prefix owl: <http://www.w3.org/2002/07/owl#> .
@prefix rdfs: <http://www.w3.org/2000/01/rdf-schema#> .
@prefix skos: <http://www.w3.org/2004/02/skos/core#> .
@prefix vann: <http://purl.org/vocab/vann/> .
@prefix xsd: <http://www.w3.org/2001/XMLSchema#> .

aec3po:statement a owl:Ontology ;
    cc:license <https://creativecommons.org/licenses/by/4.0/> ;
    dct:contributor <http://maxime-lefrancois.info/me#> ;
    dct:description """The AEC3PO Statement module describes a statement, of any kind, found in a document."""@en ;
    dct:description <diagrams/statement.png> ;
    dct:title "AEC3PO: statement"@en ;
    vann:preferredNamespacePrefix "aec3po" ;
    vann:preferredNamespaceUri "https://w3id.org/lbd/aec3po/" ;
    owl:imports aec3po:document .

aec3po:Statement a owl:Class ;
 rdfs:label "Statement"@en ;
 rdfs:comment "Something stated in a building compliance-related document"@en ;
 skos:example "Any solar protection solutions in the building shall be taken into account in the calculation of solar energy gains for the building."@en ;
 rdfs:subClassOf aec3po:DocumentSubdivision ;
 rdfs:isDefinedBy aec3po:statement .

  aec3po:hasEvidence a owl:ObjectProperty;
    rdfs:label "hasEvidence"@en ;
    rdfs:comment "Links a statement to a piece of evidence for that statement (assertion, statement, or claim)."@en ;
    skos:note "Unstable. Need evidence of how this property is intended to be used"@en ;
    rdfs:domain aec3po:Statement ;
    rdfs:isDefinedBy aec3po:statement .

## Defined in the RASEDecomposedStatement module 
#aec3po:requires a owl:ObjectProperty;
    #rdfs:label "requires"@en ;
    #rdfs:comment "Links a statement to something that needs to be provided or associated with it."@en ;
    #skos:example "A property to perform a calculation, an Information Delivery Specification (IDS) file, a certificate, ..."@en ;
    #skos:note "Unstable. Need evidence of how this property is intended to be used"@en ;
    #rdfs:domain aec3po:Statement ;
    #rdfs:isDefinedBy aec3po:statement .

aec3po:hasInlinePart a owl:ObjectProperty ;
  rdfs:label "hasInlinePart"@en ;
  rdfs:comment "Links a statement to an inline subdivision of that statement."@en;
  rdfs:subPropertyOf dct:hasPart ;
  rdfs:seeAlso <https://github.com/Accord-Project/aec3po/issues/43> ;
  rdfs:isDefinedBy aec3po:statement .

# definitions

aec3po:DefinitionStatement a owl:Class ;
 rdfs:label "Definition Statement"@en ;
 rdfs:comment "A type of statement that provides a formal and precise definition for a specific concept or term, scoped to this document."@en ;
 rdfs:subClassOf aec3po:Statement ;
 rdfs:isDefinedBy aec3po:statement .

    aec3po:definitionOf a owl:ObjectProperty ;
        rdfs:label "definition of"@en ;
        rdfs:comment "Links a definition statement to the term that is defined"@en ;
        rdfs:domain aec3po:DefinitionStatement ;
        rdfs:range aec3po:DocumentSubdivision ;
        rdfs:isDefinedBy aec3po:statement .

    aec3po:hasDefinition a owl:ObjectProperty ;
        rdfs:label "has definition"@en ;
        rdfs:comment "Links a definition statement to the definition of the term"@en ;
        rdfs:domain aec3po:DefinitionStatement ;
        rdfs:range aec3po:DocumentSubdivision ;
        rdfs:isDefinedBy aec3po:statement .

# check statement 

aec3po:CheckStatement a owl:Class ;
 rdfs:label "Check Statement"@en ;
 rdfs:comment "refers to a type of statement that is used to specify conditions, criteria, or rules for evaluating the compliance, correctness, or validity of certain properties, features, or aspects of a system, process, or domain."@en ;
 rdfs:subClassOf aec3po:Statement ;
 rdfs:isDefinedBy aec3po:statement .

aec3po:CategoryCheckStatement a owl:Class ;
 rdfs:label "Category Check Statement"@en ;
 rdfs:comment "Category check statement refers to a type of statement or requirement that focuses on verifying compliance with specific categories of regulations, standards, or guidelines within the construction industry. Category check statements are used to assess whether a construction project aligns with predefined categories of criteria, such as safety, environmental impact, energy efficiency, accessibility, and more."@en ;
 rdfs:seeAlso <https://github.com/Accord-Project/aec3po/issues/56> ;
 rdfs:subClassOf aec3po:CheckStatement ;
 rdfs:isDefinedBy aec3po:statement .

aec3po:CertificateCheckStatement a owl:Class ;
 rdfs:label "Certificate Check Statement"@en ;
 rdfs:comment "Certificate check statement refers to a type of statement or requirement that focuses on verifying and validating the authenticity and compliance of certificates related to construction projects"@en ;
 rdfs:subClassOf aec3po:CheckStatement ;
 rdfs:seeAlso <https://github.com/Accord-Project/aec3po/issues/59> ;
 rdfs:isDefinedBy aec3po:statement .

aec3po:ChecklistStatement a owl:Class ;
 rdfs:label "Checklist Statement"@en ;
 rdfs:comment "Checklist statement is a type of check statement that represents a list of checks that need to be verified."@en ;
 rdfs:subClassOf aec3po:CheckStatement ;
 rdfs:isDefinedBy aec3po:statement .

# human evaluated statement

aec3po:HumanEvaluatedCheckStatement a owl:Class ;
 rdfs:label "Human Evaluated Check Statement"@en ;
 rdfs:comment "A type of check statement that is evaluated by a human."@en ;
 skos:note "Those are primarily for issues of perception"@en ;
 skos:example "\"is aesthetically appropriate\""@en ;
 rdfs:seeAlso <https://github.com/Accord-Project/aec3po/issues/60> ;
 rdfs:subClassOf aec3po:CheckStatement ;
 rdfs:isDefinedBy aec3po:statement .

    aec3po:hasEvaluator a owl:ObjectProperty ;
        rdfs:label "has evaluator"@en ;
        rdfs:comment "Links a human evaluated statement to the subdivision that expresses who shall verify this check"@en ;
        rdfs:domain aec3po:HumanEvaluatedCheckStatement ;
        rdfs:range aec3po:Statement ;
        rdfs:isDefinedBy aec3po:statement .

aec3po:NumericalCheckStatement a owl:Class ;
 rdfs:label "Numerical Check Statement"@en ;
 rdfs:comment "A type of check that involves checking one numerical property against another, i.e. x < y or similar." ;
 rdfs:subClassOf aec3po:CheckStatement ;
 rdfs:seeAlso <https://github.com/Accord-Project/aec3po/issues/57> ;
 rdfs:isDefinedBy aec3po:statement .

aec3po:BooleanCheckStatement a owl:Class ;
 rdfs:label "Boolean Check Statement"@en ;
 rdfs:comment "A type of check that checks the existence of an element (property) related to a feature of interest."@en ;
 rdfs:seeAlso <https://github.com/Accord-Project/aec3po/issues/58> ;
 rdfs:subClassOf aec3po:CheckStatement ;
 rdfs:isDefinedBy aec3po:statement .

aec3po:AndCheckStatement a owl:Class ;
 rdfs:label "And Check Statement"@en ;
 rdfs:comment "Check verified if and only if all of its sub-checks are verified."@en ;
 rdfs:subClassOf [ a owl:Restriction ;
  owl:minCardinality 1 ;
  owl:onProperty aec3po:hasSubdivision ],
 aec3po:ChecklistStatement ;
 rdfs:isDefinedBy aec3po:statement .

aec3po:OrCheckStatement a owl:Class ;
 rdfs:label "Or Check Statement"@en ;
 rdfs:comment "Check verified if and only if at least one of its sub-checks is verified."@en ;
 rdfs:subClassOf [ a owl:Restriction ;
  owl:minCardinality 1 ;
  owl:onProperty aec3po:hasSubdivision ],
 aec3po:ChecklistStatement ;
 rdfs:isDefinedBy aec3po:statement .

aec3po:NotCheckStatement a owl:Class ;
 rdfs:label "Not Check Statement"@en ;
 rdfs:comment "Check verified if and only if the sub-check is not verified."@en ;
 rdfs:subClassOf [ a owl:Restriction ;
  owl:cardinality 1 ;
  owl:onProperty aec3po:hasSubdivision ] ;
 rdfs:isDefinedBy aec3po:statement .

