@prefix aec3po: <https://w3id.org/lbd/aec3po/> .
@prefix cc: <http://creativecommons.org/ns#> .
@prefix dct: <http://purl.org/dc/terms/> .
@prefix dul: <http://www.ontologydesignpatterns.org/ont/dul/DUL.owl#> .
@prefix owl: <http://www.w3.org/2002/07/owl#> .
@prefix rdfs: <http://www.w3.org/2000/01/rdf-schema#> .
@prefix skos: <http://www.w3.org/2004/02/skos/core#> .
@prefix vann: <http://purl.org/vocab/vann/> .
@prefix xsd: <http://www.w3.org/2001/XMLSchema#> .

aec3po:statement a owl:Ontology ;
    cc:license <https://creativecommons.org/licenses/by/4.0/> ;
    dct:contributor <http://maxime-lefrancois.info/me#> ;
    dct:description """The AEC3PO Statement module describes things stated in a building compliance-related document"""@en ;
    dct:description <statement.png> ;
    dct:title "AEC3PO: statement"@en ;
    vann:preferredNamespacePrefix "aec3po" ;
    vann:preferredNamespaceUri "https://w3id.org/lbd/aec3po/" .


aec3po:Statement a owl:Class ;
 rdfs:label "Statement"@en ;
 rdfs:comment "Something stated in a building compliance-related document"@en ;
 rdfs:isDefinedBy aec3po:statement ;
 rdfs:subClassOf aec3po:DocumentSubdivision ;
 skos:example "Any solar protection solutions in the building shall be taken into account in the calculation of solar energy gains for the building."@en .

aec3po:hasEvidence a owl:ObjectProperty;
 rdfs:comment "Links a statement to a piece of evidence for that statement (assertion, statement, or claim)."@en ;
 rdfs:domain aec3po:Statement ;
 rdfs:range aec3po:Statement ;
 rdfs:isDefinedBy aec3po:statement .

aec3po:hasRequiredData a owl:ObjectProperty;
 rdfs:comment "Links a statement to something that needs to be provided or associated with it."@en ;
 skos:example "A property to perform a calculation, an Information Delivery Specification (IDS) file, a certificate, ..."@en ;
 rdfs:domain aec3po:Statement ;
 rdfs:isDefinedBy aec3po:statement .

aec3po:CheckStatement a owl:Class ;
 rdfs:label "Check Statement"@en ;
 rdfs:comment "refers to a type of statement that is used to specify conditions, criteria, or rules for evaluating the compliance, correctness, or validity of certain properties, features, or aspects of a system, process, or domain."@en ;
 rdfs:subClassOf aec3po:Statement ;
 rdfs:isDefinedBy aec3po:statement .

aec3po:CategoryCheckStatement a owl:Class ;
 rdfs:label "Category Check Statement"@en ;
 rdfs:comment "Category check statement refers to a type of statement or requirement that focuses on verifying compliance with specific categories of regulations, standards, or guidelines within the construction industry. Category check statements are used to assess whether a construction project aligns with predefined categories of criteria, such as safety, environmental impact, energy efficiency, accessibility, and more."@en ;
 rdfs:subClassOf aec3po:CheckStatement ;
 rdfs:isDefinedBy aec3po:statement .

aec3po:CertificateCheckStatement a owl:Class ;
 rdfs:label "Certificate Check Statement"@en ;
 rdfs:comment "Certificate check statement refers to a type of statement or requirement that focuses on verifying and validating the authenticity and compliance of certificates related to construction projects"@en ;
 rdfs:subClassOf aec3po:CheckStatement ;
 rdfs:isDefinedBy aec3po:statement .

aec3po:ChecklistStatement a owl:Class ;
 rdfs:label "Checklist Statement"@en ;
 rdfs:comment "Checklist statement is a type of check statement that represents a list of checks that need to be verified."@en ;
 rdfs:subClassOf aec3po:CheckStatement ;
 rdfs:isDefinedBy aec3po:statement .

aec3po:DefinitionStatement a owl:Class ;
 rdfs:label "Definition Statement"@en ;
 rdfs:comment "A type of statement that provides a formal and precise definition for a specific concept or term."@en ;
 rdfs:subClassOf aec3po:Statement ;
 rdfs:isDefinedBy aec3po:statement .

aec3po:HumanEvaluatedStatement a owl:Class ;
 rdfs:label "Human Evaluated Statement"@en ;
 rdfs:comment "A type of check statement that is evaluated by a human."@en ;
 skos:note "Those are primarily for issues of perception"@en ;
 skos:example "\"is aesthetically appropriate\""@en ;
 rdfs:subClassOf aec3po:CheckStatement ;
 rdfs:isDefinedBy aec3po:statement .

aec3po:NumericalCheckStatement a owl:Class ;
 rdfs:label "Numerical Check Statement"@en ;
 rdfs:comment "A type of check that involves checking one numerical property against another, i.e. x < y or similar." ;
 rdfs:subClassOf aec3po:CheckStatement ;
 rdfs:isDefinedBy aec3po:statement .

aec3po:BooleanCheckStatement a owl:Class ;
 rdfs:label "Boolean Check Statement"@en ;
 rdfs:comment "A type of check that checks the existence of an element (property) related to a feature of interest."@en ;
 rdfs:subClassOf aec3po:CheckStatement ;
 rdfs:isDefinedBy aec3po:statement .

aec3po:AndCheck a owl:Class ;
 rdfs:label "And Check"@en ;
 rdfs:comment "Check verified if and only if all of its sub-checks are verified."@en ;
 rdfs:subClassOf [ a owl:Restriction ;
  owl:minCardinality 1 ;
  owl:onProperty aec3po:hasSubCheck ],
 aec3po:ChecklistStatement ;
 rdfs:isDefinedBy aec3po:statement .

aec3po:OrCheck a owl:Class ;
 rdfs:label "Or Check"@en ;
 rdfs:comment "Check verified if and only if at least one of its sub-checks is verified."@en ;
 rdfs:subClassOf [ a owl:Restriction ;
  owl:minCardinality 1 ;
  owl:onProperty aec3po:hasSubCheck ],
 aec3po:ChecklistStatement ;
 rdfs:isDefinedBy aec3po:statement .

aec3po:hasSubCheck a owl:ObjectProperty ;
 rdfs:label "has sub check"@en ;
 rdfs:comment "Links a AndCheck to the set of checks that all need to be verified. Links a OrCheck to the set of checks that at least one must verify."@en ;
 rdfs:domain [ a owl:Class ; owl:unionOf ( aec3po:CheckListStatement aec3po:CheckMethod ) ] ;
 rdfs:range [ a owl:Class ; owl:unionOf ( aec3po:CheckStatement aec3po:CheckMethod ) ] ;
 rdfs:isDefinedBy aec3po:statement .

aec3po:Application a owl:Class ;
 rdfs:label "Application"@en ;
 rdfs:comment "Represents the Applications tag in the semantic mark-up Requirement Application Selection and Exception (RASE) methodology."@en ;
 rdfs:subClassOf aec3po:Statement ;
 rdfs:isDefinedBy aec3po:statement .

aec3po:Exception a owl:Class ;
 rdfs:label "Exception"@en ;
 rdfs:comment "Represents the Exception tag in the semantic mark-up Requirement Application Selection and Exception (RASE) methodology."@en ;
 rdfs:subClassOf aec3po:Statement ;
 rdfs:isDefinedBy aec3po:statement .

aec3po:Requirement a owl:Class ;
 rdfs:label "Requirement"@en ;
 rdfs:comment "Represents the Requirement tag in the semantic mark-up Requirement Application Selection and Exception (RASE) methodology."@en ;
 rdfs:subClassOf aec3po:Statement ;
 rdfs:isDefinedBy aec3po:statement .

aec3po:Selection a owl:Class ;
 rdfs:label "Selection"@en ;
 rdfs:comment "Represents the Selection tag in the semantic mark-up Requirements Applications Selections and Exceptions (RASE) methodology."@en ;
 rdfs:subClassOf aec3po:Statement ;
 rdfs:isDefinedBy aec3po:statement .

[] a owl:AllDifferent ; owl:members ( aec3po:Application aec3po:Selection aec3po:Requirement  aec3po:Exceptions ) .
